src/ITreeSpec/Automation.v
@@ -1,0 +1,2047 @@
+From Stdlib Require Export
+  Datatypes
+  Arith.PeanoNat
+  Arith.Peano_dec
+  Arith.Compare
+  Wf_nat
+  Morphisms
+  Setoid
+  Program.Equality
+  Lists.List
+  Logic.Eqdep_dec
+  Logic.EqdepFacts
+  Eqdep EqdepFacts
+  Logic.ProofIrrelevance.
+
+From ITree Require Import
+  Basics.HeterogeneousRelations
+  Eq.Eqit.
+
+From ITreeSpec Require Import
+  ITreeSpecDefinition
+  ITreeSpecFacts
+  ITreeSpecCombinatorFacts
+  RecSpecFix
+  SpecM
+  MRecSpec
+  SpecMFacts
+  LetRecRefines
+  DefRefines.
+
+From Paco Require Import paco.
+
+Export SigTNotations.
+
+Import SpecMNotations.
+Local Open Scope entree_scope.
+
+(* FIXME: There has to be a better way... *)
+Ltac resum_unfold :=
+  unfold (* SubEvent.v *)
+         resum, resum_ret,
+         ReSum_inl, ReSumRet_inl,
+         ReSum_inr, ReSumRet_inr,
+         (* EnTreeDefinition.v *)
+         SpecEventReSum, SpecEventReSumRet,
+         (* RecSpecFix.v *)
+         ReSum_id, ReSumRet_id,
+         callESpecReSum, callESpecReSumRet,
+         (* SpecM.v *)
+         ReSum_FunStackE_E, ReSumRet_FunStackE_E,
+         ReSum_FunStackE_Error, ReSumRet_FunStackE_Error,
+         ReSum_LRTInput_FunStackE, ReSumRet_LRTInput_FunStackE,
+         ReSum_FrameCall_FunStackE, ReSumRet_FrameCall_FunStackE.
+Ltac encodes_unfold_in H :=
+  unfold (* HeterogeneousRelations.v *)
+         encodes,
+         EncodingSum,
+         (* QuantEnc.v *)
+         EncodingType_QuantEnc, encodes_QuantEnc,
+         (* EnTreeSpecDefinition *)
+         SpecEventEncoding,
+         (* SpecM.v *)
+         EncodingType_LRTInput,
+         EncodingType_FrameCall,
+         EncodingType_ErrorE,
+         EncodingType_FunStackE,
+         EncodingType_EncType in H.
+
+(***
+ *** Definition and basic properties of spec_refines
+ ***)
+
+
+(* FIXME: need rules to add binds to all the unary combinators *)
+
+(** Refinement rules for recursion **)
+
+Definition callSPost {E1 E2 : EncType} {Γ1 Γ2 R1 R2}
+  (RPost : SpecPostRel E1 E2 Γ1 Γ2)
+  (call1 : FrameCallWithRet Γ1 R1) (call2 : FrameCallWithRet Γ2 R2)
+  (r1 : R1) (r2 : R2) : Prop :=
+  RPost
+    (inl (proj1_sig call1)) (inl (proj1_sig call2))
+    (eq_rect _ (fun T => T) r1 _ (eq_sym (proj2_sig call1)))
+    (eq_rect _ (fun T => T) r2 _ (eq_sym (proj2_sig call2))).
+
+Lemma spec_refines_call (E1 E2 : EncType) Γ1 Γ2 R1 R2
+      (RPre : SpecPreRel E1 E2 Γ1 Γ2)
+      (RPost : SpecPostRel E1 E2 Γ1 Γ2)
+      (call1 : FrameCallWithRet Γ1 R1) (call2 : FrameCallWithRet Γ2 R2)
+      (RR : Rel R1 R2) :
+  RPre (inl (proj1_sig call1)) (inl (proj1_sig call2)) ->
+  (forall r1 r2, callSPost RPost call1 call2 r1 r2 -> RR r1 r2) ->
+  spec_refines RPre RPost RR (CallS _ _ _ call1) (CallS _ _ _ call2).
+Proof.
+  intros. apply padded_refines_vis; [ auto | ].
+  intros. apply padded_refines_ret. apply H0.
+  unfold callSPost.
+  rewrite rew_compose. rewrite rew_compose.
+  rewrite <- eq_rect_eq. rewrite <- eq_rect_eq. assumption.
+Qed.
+
+(* The bind of one recursive call refines the bind of another if the recursive
+   calls are in the current RPre and, for all return values for them in RPost,
+   the bind continuations refine each other *)
+Lemma spec_refines_call_bind (E1 E2 : EncType) Γ1 Γ2 R1 R2 T1 T2
+      (RPre : SpecPreRel E1 E2 Γ1 Γ2)
+      (RPost : SpecPostRel E1 E2 Γ1 Γ2)
+      (RR : T1 -> T2 -> Prop)
+      (call1 : FrameCallWithRet Γ1 R1) (call2 : FrameCallWithRet Γ2 R2)
+      (k1 : R1 -> SpecM E1 Γ1 T1)
+      (k2 : R2 -> SpecM E2 Γ2 T2) :
+  RPre (inl (proj1_sig call1)) (inl (proj1_sig call2)) ->
+  (forall r1 r2,
+      callSPost RPost call1 call2 r1 r2 ->
+      spec_refines RPre RPost RR (k1 r1) (k2 r2)) ->
+  spec_refines RPre RPost RR (CallS _ _ _ call1 >>= k1) (CallS _ _ _ call2 >>= k2).
+Proof.
+  intros. eapply padded_refines_bind; try eapply spec_refines_call; eauto.
+Qed.
+
+(* Add a bind to a RetS to a CallS on the left *)
+Lemma spec_refines_call_bind_ret_l (E1 E2 : EncType) Γ1 Γ2 R1 R2
+      (RPre : SpecPreRel E1 E2 Γ1 Γ2)
+      (RPost : SpecPostRel E1 E2 Γ1 Γ2)
+      (call1 : FrameCallWithRet Γ1 R1) t2 (RR : Rel R1 R2) :
+  spec_refines RPre RPost RR (CallS _ _ _ call1 >>= RetS) t2 ->
+  spec_refines RPre RPost RR (CallS _ _ _ call1) t2.
+Proof. intro; rewrite <- (bind_ret_r (CallS _ _ _ _)); eauto. Qed.
+
+(* Add a bind to a RetS to a CallS on the right *)
+Lemma spec_refines_call_bind_ret_r (E1 E2 : EncType) Γ1 Γ2 R1 R2
+      (RPre : SpecPreRel E1 E2 Γ1 Γ2)
+      (RPost : SpecPostRel E1 E2 Γ1 Γ2)
+      t1 (call2 : FrameCallWithRet Γ2 R2) (RR : Rel R1 R2) :
+  spec_refines RPre RPost RR t1 (CallS _ _ _ call2 >>= RetS) ->
+  spec_refines RPre RPost RR t1 (CallS _ _ _ call2).
+Proof. intro H; rewrite <- (bind_ret_r (CallS _ _ _ _)); eauto. Qed.
+
+
+
+
+
+(* Add a precondition relation for a new frame on the FunStack *)
+Definition pushPreRel {E1 E2 : EncType} {Γ1 Γ2}
+           (precond : Rel (FrameCall Γ1) (FrameCall Γ2))
+           (RPre : SpecPreRel E1 E2 Γ1 Γ2) :
+  SpecPreRel E1 E2 Γ1 Γ2 :=
+  fun a1 a2 => match a1,a2 with
+               | inl args1, inl args2 => precond args1 args2
+               | inr ev1, inr ev2 => RPre ev1 ev2
+               | _, _ => False
+               end.
+
+(* Add a postcondition relation for a new frame on the FunStack *)
+Definition pushPostRel {E1 E2 : EncType} {Γ1 Γ2 frame1 frame2}
+           (postcond : PostRel (FrameCall frame1) (FrameCall frame2))
+           (RPost : SpecPostRel E1 E2 Γ1 Γ2) :
+  SpecPostRel E1 E2 (frame1 :: Γ1) (frame2 :: Γ2) :=
+  fun a1 a2 => match a1,a2 with
+               | inl args1, inl args2 => postcond args1 args2
+               | inr ev1, inr ev2 => RPost ev1 ev2
+               | _, _ => fun _ _ => False
+               end.
+
+Lemma spec_refines_multifix (E1 E2 : EncType) Γ1 Γ2 frame1 frame2 
+      (RPre : SpecPreRel E1 E2 Γ1 Γ2) (RPost : SpecPostRel E1 E2 Γ1 Γ2)
+      (bodies1 : FrameTuple E1 (frame1 :: Γ1) frame1)
+      (bodies2 : FrameTuple E2 (frame2 :: Γ2) frame2)
+      (call1 : FrameCall frame1) (call2 : FrameCall frame2)
+      (RR : Rel (encodes call1) (encodes call2))
+      (precond : Rel (FrameCall frame1) (FrameCall frame2))
+      (postcond : PostRel (FrameCall frame1) (FrameCall frame2)) :
+  precond call1 call2 ->
+  (forall r1 r2, postcond call1 call2 r1 r2 -> RR r1 r2) ->
+  (forall call1' call2',
+      precond call1' call2' ->
+      spec_refines (pushPreRel precond RPre) (pushPostRel postcond RPost)
+                   (postcond call1' call2')
+                   (applyFrameTuple _ _ _ bodies1 call1')
+                   (applyFrameTuple _ _ _ bodies2 call2')) ->
+  spec_refines RPre RPost RR
+               (MultiFixS E1 Γ1 frame1 bodies1 call1)
+               (MultiFixS E2 Γ2 frame2 bodies2 call2).
+
+Proof.
+  intros Hcalls HRR Hbody.
+  unfold MultiFixS. 
+  eapply padded_refines_interp_mrec_spec with (RPreInv := precond) (RPostInv := postcond).
+  - intros. apply Hbody in H. eapply padded_refines_monot; try apply H; auto; clear - E1.
+    + intros call1 call2 Hcall. 
+      destruct call1; destruct call2; cbn in *; try contradiction;
+        constructor; auto.
+    + intros call1 call2 r1 r2 H. destruct H; auto.
+  - apply Hbody in Hcalls.
+    eapply padded_refines_monot; try apply Hcalls; auto; clear - E1.
+    + intros call1 call2 Hcall. 
+      destruct call1; destruct call2; cbn in *; try contradiction;
+        constructor; auto.
+    + intros call1 call2 r1 r2 H. destruct H; auto.
+Qed.
+
+(* The bind of one multifix refines the bind of another if: the recursive calls
+   which start the multifixes are related to each other by the supplied
+   precondition; the bodies of the multifixes refine each other and return
+   values that satisfy the supplied postcondition for all calls that satisfy the
+   precondition; and that the bind continuations refine each other for all
+   outputs in the supplied postcondition *)
+Lemma spec_refines_multifix_bind (E1 E2 : EncType) Γ1 Γ2 frame1 frame2 R1 R2
+      (RPre : SpecPreRel E1 E2 Γ1 Γ2) (RPost : SpecPostRel E1 E2 Γ1 Γ2) RR
+      (bodies1 : FrameTuple E1 (frame1 :: Γ1) frame1)
+      (bodies2 : FrameTuple E2 (frame2 :: Γ2) frame2)
+      (call1 : FrameCall frame1) (call2 : FrameCall frame2)
+      (k1 : FrameCallRet frame1 call1 -> SpecM E1 Γ1 R1)
+      (k2 : FrameCallRet frame2 call2 -> SpecM E2 Γ2 R2)
+      (precond : Rel (FrameCall frame1) (FrameCall frame2))
+      (postcond : PostRel (FrameCall frame1) (FrameCall frame2)) :
+  precond call1 call2 ->
+  (forall call1' call2',
+      precond call1' call2' ->
+      spec_refines (pushPreRel precond RPre) (pushPostRel postcond RPost)
+                   (postcond call1' call2')
+                   (applyFrameTuple _ _ _ bodies1 call1')
+                   (applyFrameTuple _ _ _ bodies2 call2')) ->
+  (forall r1 r2,
+      postcond call1 call2 r1 r2 ->
+      spec_refines RPre RPost RR (k1 r1) (k2 r2)) ->
+  spec_refines RPre RPost RR
+               (MultiFixS E1 Γ1 frame1 bodies1 call1 >>= k1)
+               (MultiFixS E2 Γ2 frame2 bodies2 call2 >>= k2).
+Proof.
+  intros.
+  eapply padded_refines_bind; try eapply spec_refines_multifix; eauto.
+Qed.
+
+(* Build a RecFrame with a single, unary function *)
+Definition unary1Frame (A B : Type) : RecFrame :=
+  cons (LRT_Fun A (fun _ => LRT_Ret B)) nil.
+
+Notation unary1Call x := (mkFrameCall (unary1Frame _ _) 0 x).
+
+
+(* The total correctness specification *)
+Definition total_spec {E Γ A B} `{QuantType B}
+           (pre : A -> Prop) (post : A -> B -> Prop) (a : A) : SpecM E Γ B :=
+  AssumeS (pre a);;
+  b <- ExistsS B;;
+  AssertS (post a b);;
+  RetS b.
+
+Definition uncall_unary1Frame {A B} (c : FrameCall (unary1Frame A B)) : A.
+destruct c. cbn in args. destruct n.
+- destruct args as [a ?]. exact a.
+- destruct args as [[] []].
+Defined.
+
+Definition call_unary1Frame {A B} (c : FrameCall (unary1Frame A B)) (b : B) : encodes c.
+destruct c. destruct n. destruct args. cbn. exact b.
+cbn in args. destruct args as [ [] _].
+Defined.
+
+(* The one-step unfolding of total_spec with recursive calls *)
+Definition total_spec_fix_body {E Γ A B} `{QuantType A} `{QuantType B}
+           (pre : A -> Prop) (post : A -> B -> Prop) (rdec : A -> A -> Prop)
+           (a : A) : SpecM E (unary1Frame A B :: Γ) B :=
+  AssumeS (pre a);;
+  n <- ExistsS nat;;
+  trepeat n (a' <- ExistsS A;;
+             AssertS (pre a' /\ rdec a' a);;
+             CallS E Γ _ (mkFrameCall (unary1Frame A B) 0 a'));;
+  b <- ExistsS B;;
+  AssertS (post a b);;
+  RetS b.
+
+(* total_spec defined with recursive calls, primarily written as part of a proof*)
+Definition total_spec_fix {E Γ A B} `{QuantType A} `{QuantType B}
+           (pre : A -> Prop) (post : A -> B -> Prop) (rdec : A -> A -> Prop)
+           (a : A) : SpecM E Γ B.
+  eapply @interp_mrec_spec with (D := (FrameCall (unary1Frame A B)));
+    try  (apply (total_spec_fix_body pre post rdec a)).
+  clear a.
+  intros call. specialize (uncall_unary1Frame call) as a. cbn. 
+  eapply EnTree.bind.
+  exact (total_spec_fix_body pre post rdec (uncall_unary1Frame call)).
+  intros b. exact (Ret (call_unary1Frame call b)).
+Defined.
+
+(* Add a precondition relation for proving total_spec refinement *)
+Definition pushTSPreRel {E1 E2 : EncType} {Γ1 Γ2 frame1 A2 B2}
+           (tsPre : A2 -> Prop)
+           (precond : Rel (FrameCall frame1) (FrameCall (unary1Frame A2 B2)))
+           (RPre : SpecPreRel E1 E2 Γ1 Γ2) :
+  SpecPreRel E1 E2 (frame1 :: Γ1) (unary1Frame A2 B2 :: Γ2) :=
+  fun a1 a2 => match a1,a2 with
+               | inl args1, inl (FrameCallOfArgs _ 0 (existT _ a2 _)) =>
+                 tsPre a2 /\ precond args1 (unary1Call a2)
+               | inr ev1, inr ev2 => RPre ev1 ev2
+               | _, _ => False
+               end.
+
+(* Add a postcondition relation for proving total_spec refinement *)
+Definition pushTSPostRel {E1 E2 : EncType} {Γ1 Γ2 frame1 A2 B2}
+           (tsPost : A2 -> B2 -> Prop)
+           (postcond : PostRel (FrameCall frame1) (FrameCall (unary1Frame A2 B2)))
+           (RPost : SpecPostRel E1 E2 Γ1 Γ2) :
+  SpecPostRel E1 E2 (frame1 :: Γ1) (unary1Frame A2 B2 :: Γ2) :=
+  fun a1 a2 => match a1,a2 return encodes a1 -> encodes a2 -> Prop with
+               | inl args1, inl (FrameCallOfArgs _ 0 (existT _ a2 _)) =>
+                 fun r1 b2 => tsPost a2 b2 /\ postcond args1 (unary1Call a2) r1 b2
+               | inr a1', inr a2' => RPost a1' a2'
+               | _, _ => fun _ _ => False
+               end.
+
+(* Add a postcondition to the return relation for proving total_spec refinement *)
+Definition pushTSRR {frame1 A2 B2}
+           (tsPost : A2 -> B2 -> Prop)
+           (postcond : PostRel (FrameCall frame1) (FrameCall (unary1Frame A2 B2)))
+           (call1 : FrameCall frame1) (a2 : A2) :
+  Rel (FrameCallRet frame1 call1) B2 :=
+  fun r1 r2 => tsPost a2 r2 /\ postcond call1 (unary1Call a2) r1 r2.
+
+Ltac quantr := apply padded_refines_assumer || apply padded_refines_assertr ||
+                     apply interp_mrec_spec_assumer || apply interp_mrec_spec_assertr || 
+                     apply padded_refines_exists_specr || 
+                     apply padded_refines_forall_specr ||
+                     apply interp_mrec_spec_forall_specr ||
+                     apply interp_mrec_spec_exists_specr
+.
+
+Ltac quantl := apply padded_refines_assumel || apply padded_refines_assertl ||
+                     apply interp_mrec_spec_assumel || apply interp_mrec_spec_assertl ||
+                     apply padded_refines_exists_specl || 
+                     apply padded_refines_forall_specl ||
+                     apply interp_mrec_spec_forall_specl ||
+                     apply interp_mrec_spec_exists_specl.
+
+Lemma total_spec_fix_refines_total_spec_aux1:
+  forall (E : EncType) (Γ : FunStack) (A B : Type) (H : QuantType A) (H0 : QuantType B)
+    (pre : A -> Prop) (post : Rel A B) (rdec : Rel A A) (a : A),
+    strict_refines
+     (interp_mrec_spec
+        (fun call : FrameCall (unary1Frame A B) =>
+           EnTree.bind
+             (EnTree.bind (AssumeS (pre (uncall_unary1Frame call)))
+                (fun _ : unit =>
+                    EnTree.bind (ExistsS nat) (fun n : nat =>
+                       EnTree.bind
+                         (trepeat n
+                           (EnTree.bind (ExistsS A)
+                                        (fun a' : A =>
+                                           EnTree.bind (AssertS (pre a' /\ rdec a' (uncall_unary1Frame call)))
+                                                       (fun _ : unit =>
+                                                          CallS E Γ (unary1Frame A B)
+                                                                (FrameCallOfArgs (unary1Frame A B) 0
+                                                                                 (existT (fun _ : A => unit) a' tt))))))
+                         (fun _ : unit =>
+                            EnTree.bind (exists_spec B)
+                                        (fun b : B =>
+                                           EnTree.bind (AssertS (post (uncall_unary1Frame call) b))
+                                                       (fun _ : unit => RetS b)))))) (fun b : B => RetS (call_unary1Frame call b)))
+        (CallS E Γ (unary1Frame A B)
+               (FrameCallOfArgs (unary1Frame A B) 0 (existT (fun _ : A => unit) a tt))))
+     (total_spec_fix pre post rdec a).
+Proof.
+  intros E Γ A B H H0 pre post rdec a. setoid_rewrite interp_mrec_spec_inl at 1.
+  rewrite tau_eutt. match goal with |- strict_refines (interp_mrec_spec ?b _) _ =>
+                                      set b as body end.
+  eapply padded_refines_interp_mrec_spec with (RPreInv := eq) (RPostInv := PostRelEq).
+  - intros. subst. destruct d2.
+    destruct n. 2 : destruct args as [ [] _].
+    destruct args as [a' []]. cbn. cbn. eapply padded_refines_bind with (RR := eq).
+    2 : { intros. apply padded_refines_ret. subst. constructor. }
+    quantr. intros. apply padded_refines_assumel. auto.
+    apply padded_refines_exists_specl. intros.
+    quantr. exists a0. eapply padded_refines_bind with (RR := eq).
+    + eapply padded_refines_monot; try apply strict_refines_refl; intros; subst.
+      destruct x1; constructor; auto. destruct PR. destruct H2. constructor.
+      destruct H2. constructor. auto.
+    + intros. subst. quantl. intros. quantr. exists a1. quantl.
+      intros. quantr. auto. apply padded_refines_ret. auto.
+ - cbn. quantr. intros. (* lets get a better way to rewrite bind_bind *)
+   eapply padded_refines_monot with (RPre1 := eq) (RPost1 := PostRelEq) (RR1 := eq); eauto.
+   + intros. subst. destruct x1; constructor; auto.
+   + intros. destruct e1; dependent destruction PR. dependent destruction H6.
+     constructor. dependent destruction H6. constructor.
+   + repeat apply padded_refines_bind_bind_l. quantl. eexists. eauto.
+     apply padded_refines_ret_bind_l. apply padded_refines_bind_bind_l.
+     eapply padded_refines_bind. apply strict_refines_refl.
+     intros. subst. apply padded_refines_bind_bind_l.
+     eapply padded_refines_bind. apply strict_refines_refl.
+     intros [] [] _. apply padded_refines_bind_bind_l. 
+     quantl. intros. quantr. exists a0. apply padded_refines_bind_bind_l.
+     quantl. intros. quantr. auto. repeat apply padded_refines_ret_bind_l.
+     apply padded_refines_ret. cbv. auto.
+Qed.
+   
+Lemma total_spec_fix_refines_total_spec {E Γ A B} `{QuantType A} `{QuantType B}
+           (pre : A -> Prop) (post : A -> B -> Prop) (rdec : A -> A -> Prop)
+           (a : A) : 
+  well_founded rdec ->
+  strict_refines (total_spec_fix pre post rdec a) (@total_spec E Γ A B _ pre post a).
+Proof.
+  intros Hwf. revert a. apply well_founded_ind with (R := rdec). auto.
+  intros x Hind. unfold total_spec_fix. unfold total_spec_fix_body. cbn.
+  match goal with |- strict_refines (interp_mrec_spec ?b _) _ =>
+                    set b as body end.
+  quantr. intro. quantl. auto. apply interp_mrec_spec_exists_specl. intros n.
+  induction n.
+  - cbn. rewrite bind_ret_l. apply interp_mrec_spec_exists_specl.
+    intros b. quantr. exists b. apply interp_mrec_spec_assertl.
+    intros. quantr. auto. rewrite interp_mrec_spec_ret.
+    apply padded_refines_ret. auto.
+  - cbn. repeat rewrite bind_bind. apply interp_mrec_spec_exists_specl.
+    intros a. rewrite bind_bind. apply interp_mrec_spec_assertl.
+    intros [Hpre Hdec]. rewrite interp_mrec_spec_bind.
+    specialize (Hind a Hdec). 
+    match goal with |- padded_refines eq PostRelEq eq (EnTree.bind ?tf _ ) _ =>
+                      assert (strict_refines tf (total_spec_fix pre post rdec a)) end.
+    apply total_spec_fix_refines_total_spec_aux1.
+    eapply padded_refines_weaken_r
+           with (phi2 := EnTree.bind (total_spec pre post a)  (fun _  =>
+              EnTree.bind (exists_spec B)
+                (fun b : B => EnTree.bind (AssertS (post x b)) (fun _ : unit => RetS b))) )
+    .
+    { eapply padded_refines_bind; eauto. eapply padded_refines_weaken_l; eauto. } 
+    clear - Hwf Hpre Hdec. cbn.
+    apply padded_refines_bind_bind_l. quantl. auto.
+    apply padded_refines_bind_bind_l. quantl. intros b. apply padded_refines_bind_bind_l.
+    quantl. intros. rewrite bind_ret_l. quantl. intros bf.
+    quantl. intros Hbf. quantr. exists bf. quantr. auto. apply padded_refines_ret.
+    auto.
+Qed.
+
+Definition lift_ts_pre
+  {frame1 : RecFrame} {A2 B2 : Type} (tsPre : A2 -> Prop)
+  (precond : Rel (FrameCall frame1) (FrameCall (unary1Frame A2 B2))) :
+  Rel (FrameCall frame1) (FrameCall (unary1Frame A2 B2)) :=
+  fun c1 c2 => exists a : A2, FrameCallOfArgs (unary1Frame A2 B2) 0 (existT _ a tt) = c2 /\ precond c1 (unary1Call a) /\ tsPre a.
+
+Definition lift_ts_post:
+  forall {frame1 : RecFrame} {A2 B2 : Type} (tsPost : A2 -> B2 -> Prop)
+    (postcond : PostRel (FrameCall frame1) (FrameCall (unary1Frame A2 B2))),
+    PostRel (FrameCall frame1) (FrameCall (unary1Frame A2 B2)).
+  intros frame1 A2 B2 tsPost postcond.
+  intros c1 c2 a b.
+  specialize (postcond c1 c2).
+  destruct c2. cbn in b. destruct n.
+  cbn in b. destruct args. apply (tsPost x b /\ postcond a b).
+  destruct args. destruct x.
+Defined.
+(*with some strategic lemmas this should be doable *)
+
+Lemma spec_refines_total_spec_monot_aux1:
+  forall (E1 E2 : EncType) (Γ1 Γ2 : FunStack) (frame1 : RecFrame) (A2 B2 : Type) (RPre : SpecPreRel E1 E2 Γ1 Γ2)
+    (precond : Rel (FrameCall frame1) (FrameCall (unary1Frame A2 B2))) (tsPre : A2 -> Prop)
+    (x0 : FrameCall frame1 +
+            (fix FunStackE (E : Type) (Γ : FunStack) {struct Γ} : Type :=
+               match Γ with
+               | nil => (ErrorE + E)%type
+               | frame :: Γ' => (FrameCall frame + FunStackE E Γ')%type
+               end) E1 Γ1) (x1 : FrameCall (unary1Frame A2 B2) + FunStackE E2 Γ2),
+    pushTSPreRel tsPre precond RPre x0 x1 -> HeterogeneousRelations.sum_rel (lift_ts_pre tsPre precond) RPre x0 x1.
+Proof.
+  intros E1 E2 Γ1 Γ2 frame1 A2 B2 RPre preEq pre.
+  intros x c PR. destruct x.
+  - cbn in PR. destruct c.
+    + destruct f0. destruct n. destruct args. 2 :destruct PR. 
+      cbn. constructor. exists x. destruct l. destruct PR. auto.
+    + destruct PR.
+  - destruct c; try (destruct PR; fail). red in PR. constructor. auto.
+Qed.
+
+Lemma spec_refines_total_spec_monot_aux2:
+  forall (E1 E2 : EncType) (Γ1 Γ2 : FunStack) (frame1 : RecFrame) (A2 B2 : Type) (RPost : SpecPostRel E1 E2 Γ1 Γ2)
+    (postcond : PostRel (FrameCall frame1) (FrameCall (unary1Frame A2 B2))) (tsPost : A2 -> B2 -> Prop)
+    (e1 : FrameCall frame1 +
+            (fix FunStackE (E : Type) (Γ : FunStack) {struct Γ} : Type :=
+               match Γ with
+               | nil => (ErrorE + E)%type
+               | frame :: Γ' => (FrameCall frame + FunStackE E Γ')%type
+               end) E1 Γ1) (e2 : FrameCall (unary1Frame A2 B2) + FunStackE E2 Γ2) (x0 : encodes e1) (x1 : encodes e2),
+    SumPostRel (lift_ts_post tsPost postcond) RPost e1 e2 x0 x1 -> pushTSPostRel tsPost postcond RPost e1 e2 x0 x1.
+Proof.
+  intros E1 E2 Γ1 Γ2 frame1 A2 B2 RPost postcond tsPost.
+  intros c1 c2 a b Hab.
+  destruct c1.
+  - destruct Hab; auto.
+    destruct e2. cbn in args. destruct n. cbn in args.
+    2 : destruct args as [ [] _ ].
+    destruct args as [ a2 [] ]. auto.
+  - cbn in *.  destruct c2; auto.
+    + dependent destruction Hab.
+    + dependent destruction Hab. auto.
+Qed.
+
+(*
+Lemma spec_refines_total_spec_post_aux {E1 Γ1 E2 Γ2 A B} `{EncodingType E1} `{EncodingType E2} `{QuantType A} `{QuantType B}
+           (pre : A -> Prop) (post : A -> B -> Prop) (rdec : A -> A -> Prop) (phi1) : 
+. *)
+
+Axiom inj_FrameCallOfArgs : forall frame n x y, FrameCallOfArgs frame n x = FrameCallOfArgs frame n y ->
+                                        x = y.
+
+Lemma spec_refines_total_spec (E1 E2 : EncType) Γ1 Γ2 frame1
+      A2 B2 `{QuantType A2} `{QuantType B2}
+      (RPre : SpecPreRel E1 E2 Γ1 Γ2) (RPost : SpecPostRel E1 E2 Γ1 Γ2)
+      (bodies1 : FrameTuple E1 (frame1 :: Γ1) frame1)
+      (call1 : FrameCall frame1) (a2 : A2)
+      (RR : Rel (FrameCallRet frame1 call1) B2)
+      (precond : Rel (FrameCall frame1) (FrameCall (unary1Frame A2 B2)))
+      (postcond : PostRel (FrameCall frame1) (FrameCall (unary1Frame A2 B2)))
+      (tsPre : A2 -> Prop) (tsPost : A2 -> B2 -> Prop)
+      (rdec : A2 -> A2 -> Prop) :
+  well_founded rdec ->
+  precond call1 (unary1Call a2) ->
+  (forall r1 r2, tsPost a2 r2 -> postcond call1 (unary1Call a2) r1 r2 -> RR r1 r2) ->
+  (forall call1' a2',
+      precond call1' (unary1Call a2') ->
+      spec_refines (pushTSPreRel tsPre precond RPre)
+                   (pushTSPostRel tsPost postcond RPost)
+                   (pushTSRR tsPost postcond call1' a2')
+                   (applyFrameTuple _ _ _ bodies1 call1')
+                   (total_spec_fix_body tsPre tsPost rdec a2')) ->
+  spec_refines RPre RPost RR
+               (MultiFixS E1 Γ1 frame1 bodies1 call1)
+               (total_spec tsPre tsPost a2).
+Proof.
+  intros Hwf Hca HPost HPost'. intros.
+  eapply total_spec_fix_refines_total_spec in Hwf as Hstrict. Unshelve. all : auto.
+  eapply padded_refines_weaken_l; eauto.
+  apply padded_refines_weaken_l with (phi2 := AssumeS (tsPre a2);; (total_spec_fix tsPre tsPost rdec a2)).
+  {
+    quantr. intros. quantl. auto. quantl. auto. reflexivity.
+  }
+  quantr. intros Ha2.
+  eapply padded_refines_interp_mrec_spec with (RPreInv := lift_ts_pre tsPre precond)
+                                              (RPostInv := lift_ts_post tsPost postcond). Unshelve.
+  - clear Hca Hstrict . rename a2 into a0. intros c1 c2 Hpre. destruct c2. destruct n.
+    2 : { destruct args as [ [] _]. }
+    cbn in args. destruct args as [a2 [] ]. simpl. setoid_rewrite bind_ret_r.
+    idtac. red in Hpre. destruct Hpre as [a2' [Heq [H1 H2] ]].
+    assert (a2 = a2'). apply inj_FrameCallOfArgs in Heq. dependent destruction Heq.
+    auto.
+    subst.
+    eapply padded_refines_monot; try apply HPost'; eauto.
+    + apply spec_refines_total_spec_monot_aux1.
+    + apply spec_refines_total_spec_monot_aux2.
+  - eapply padded_refines_monot; try eapply HPost'; eauto.
+    + apply spec_refines_total_spec_monot_aux1.
+    + apply spec_refines_total_spec_monot_aux2.
+    + intros. destruct PR. auto.
+Qed.
+
+
+(***
+ *** Hints for automation
+ ***)
+
+Create HintDb refines.
+Create HintDb prepostcond.
+
+(* If nothing else works, shelve the current refinement goal *)
+#[global] Hint Extern 999 (spec_refines _ _ _ _ _) => shelve : refines.
+
+
+(** IntroArg Definition and Hints **)
+
+(* Classes of variables and their associated naming conventions *)
+Inductive ArgName := Any | RetAny | Hyp | Call |
+                     SAWLet | Assert | Assume | Exists | Forall |
+                     If | Match | Destruct.
+Ltac argName n :=
+  match n with
+  | Any      => fresh "a"
+  | RetAny   => fresh "r"
+  | Hyp      => fresh "H"
+  | Call     => fresh "call"
+  | SAWLet   => fresh "e_let"
+  | Assert   => fresh "e_assert"
+  | Assume   => fresh "e_assume"
+  | Exists   => fresh "e_exists"
+  | Forall   => fresh "e_forall"
+  | If       => fresh "e_if"
+  | Match    => fresh "e_match"
+  | Destruct => fresh "e_destruct"
+  end.
+
+(* IntroArg marks a goal which introduces a variable. This is used to control
+   how variables are introduced, allowing them to be eliminated and to give them
+   meaningful names using argName above *)
+Polymorphic Definition IntroArg (n : ArgName) A (goal : A -> Type) :=
+  forall a, goal a.
+
+#[global] Hint Opaque IntroArg : refines prepostcond.
+
+Polymorphic Lemma IntroArg_fold n A goal : IntroArg n A goal -> forall a, goal a.
+Proof. intros H a; exact (H a). Qed.
+
+(* Polymorphic Lemma IntroArg_unfold n A (goal : A -> Prop) : (forall a, goal a) -> IntroArg n A goal. *)
+(* Proof. unfold IntroArg; intro H; exact H. Qed. *)
+
+Ltac IntroArg_intro e := intro e.
+
+Ltac IntroArg_forget := let e := fresh in intro e; clear e.
+
+Polymorphic Definition IntroArg_beta n A (f : A -> Type) x goal :
+  IntroArg n (f x) goal ->
+  IntroArg n ((fun x' => f x') x) goal := fun f x => f x.
+
+Polymorphic Definition IntroArg_prod n A B (goal : A * B -> Type) :
+  IntroArg n A (fun a => IntroArg n B (fun b => goal (a , b))) ->
+  IntroArg n _ goal := fun H '(a, b) => H a b.
+
+Polymorphic Definition IntroArg_sigT n A P (goal : sigT P -> Type) :
+  IntroArg n A (fun a => IntroArg n (P a) (fun p => goal (existT _ a p))) ->
+  IntroArg n _ goal := fun H '(a ; p) => H a p.
+
+Polymorphic Definition IntroArg_unit n (goal : unit -> Type) :
+  goal tt -> IntroArg n _ goal := fun H 'tt => H.
+
+Polymorphic Lemma IntroArg_and n P Q (goal : P /\ Q -> Prop)
+  : IntroArg n P (fun p => IntroArg n Q (fun q => goal (conj p q))) ->
+    IntroArg n _ goal.
+Proof. intros H [ p q ]; apply H. Qed.
+
+Polymorphic Lemma IntroArg_true n (goal : True -> Prop) : goal I -> IntroArg n _ goal.
+Proof. intros H []; eauto. Qed.
+
+Polymorphic Lemma IntroArg_false n (goal : False -> Prop) : IntroArg n _ goal.
+Proof. intros []. Qed.
+
+Polymorphic Lemma IntroArg_eq_prod_const n A B (a a' : A) (b b' : B) (goal : Type)
+  : IntroArg n (a = a') (fun _ => IntroArg n (b = b') (fun _ => goal)) ->
+    IntroArg n ((a,b) = (a',b')) (fun _ => goal).
+Proof. intros H eq; apply H; injection eq; eauto. Qed.
+
+Polymorphic Lemma IntroArg_eq_sigT_const n A B (a a' : A) (b b' : B) (goal : Type)
+  : IntroArg n (a = a') (fun _ => IntroArg n (b = b') (fun _ => goal)) ->
+    IntroArg n (existT _ a b = existT _ a' b') (fun _ => goal).
+Proof. intros H eq; apply H; injection eq; eauto. Qed.
+
+Polymorphic Lemma IntroArg_eq_dep1_const n A B (a : A) (b b' : B a) (goal : Type)
+  : IntroArg n (b = b') (fun _ => goal) ->
+    IntroArg n (eq_dep1 A B a b a b') (fun _ => goal).
+Proof.
+  intro H. unfold IntroArg in *. intro Heqdep. apply H.
+  apply eq_dep1_dep in Heqdep. apply eq_dep_eq. auto.
+Qed.
+
+Polymorphic Lemma IntroArg_eq_rect_const_l n A B (a1 a2 : A) b1 b2 eq goal :
+  IntroArg n (b1 = b2) (fun _ => goal) ->
+  IntroArg n (eq_rect a1 (fun _ => B) b1 a2 eq = b2) (fun _ => goal).
+Proof. destruct eq; do 2 intro; eauto. Qed.
+
+Polymorphic Lemma IntroArg_eqPostRel n E Γ e a1 a2 (goal : _ -> Prop) :
+  IntroArg n (a1 = a2) (fun pf => goal (eq_dep1_intro _ _ _ _ _ _ (eq_refl e) pf)) ->
+  IntroArg n (@eqPostRel E Γ e e a1 a2) goal.
+Proof.
+  intros H H0; dependent destruction H0.
+  apply H.
+Qed.
+
+Polymorphic Lemma IntroArg_pushPreRel_inl n E1 E2 Γ1 Γ2 frame1 frame2
+            (precond : Rel (FrameCall frame1) (FrameCall frame2))
+            (RPre : SpecPreRel E1 E2 Γ1 Γ2) e1 e2 (goal : _ -> Prop) :
+  IntroArg n (precond e1 e2) goal ->
+  IntroArg n (@pushPreRel E1 E2 Γ1 Γ2 frame1 frame2
+                          precond RPre (inl e1) (inl e2)) goal.
+Proof. intro H. apply H. Qed.
+
+Polymorphic Lemma IntroArg_pushPreRel_inr n E1 E2 Γ1 Γ2 frame1 frame2
+            (precond : Rel (FrameCall frame1) (FrameCall frame2))
+            (RPre : SpecPreRel E1 E2 Γ1 Γ2) e1 e2 (goal : _ -> Prop) :
+  IntroArg n (RPre e1 e2) goal ->
+  IntroArg n (@pushPreRel E1 E2 Γ1 Γ2 frame1 frame2
+                          precond RPre (inr e1) (inr e2)) goal.
+Proof. intro H. apply H. Qed.
+
+Polymorphic Lemma IntroArg_pushPostRel_inl n E1 E2 Γ1 Γ2 frame1 frame2
+            (postcond : PostRel (FrameCall frame1) (FrameCall frame2))
+            (RPost : SpecPostRel E1 E2 Γ1 Γ2)
+            (call1 : FrameCall frame1) (call2 : FrameCall frame2)
+            r1 r2 (goal : _ -> Prop) :
+  IntroArg n (postcond _ _ r1 r2) goal ->
+  IntroArg n (@pushPostRel E1 E2 Γ1 Γ2 frame1 frame2
+                           postcond RPost (inl call1) (inl call2) r1 r2) goal.
+Proof. intro H. apply H. Qed.
+
+Polymorphic Lemma IntroArg_pushPostRel_inr n E1 E2 Γ1 Γ2 frame1 frame2
+            (postcond : PostRel (FrameCall frame1) (FrameCall frame2))
+            (RPost : SpecPostRel E1 E2 Γ1 Γ2)
+            e1 e2 r1 r2 (goal : _ -> Prop) :
+  IntroArg n (RPost _ _ r1 r2) goal ->
+  IntroArg n (@pushPostRel E1 E2 Γ1 Γ2 frame1 frame2
+                           postcond RPost (inr e1) (inr e2) r1 r2) goal.
+Proof. intro H. apply H. Qed.
+
+Polymorphic Lemma IntroArg_pushTSPreRel_inl n E1 E2 Γ1 Γ2 frame1 A2 B2
+            (tsPre : A2 -> Prop)
+            (precond : Rel (FrameCall frame1) (FrameCall (unary1Frame A2 B2)))
+            (RPre : SpecPreRel E1 E2 Γ1 Γ2)
+            args1 a2 (goal : _ -> Prop) :
+  IntroArg n (tsPre a2 /\ precond args1 (unary1Call a2)) goal ->
+  IntroArg n (@pushTSPreRel E1 E2 Γ1 Γ2 frame1 A2 B2
+                            tsPre precond RPre (inl args1)
+                            (inl (mkFrameCall (unary1Frame A2 B2) 0 a2))) goal.
+Proof. intro H. apply H. Qed.
+
+Polymorphic Lemma IntroArg_pushTSPreRel_inr n E1 E2 Γ1 Γ2 frame1 A2 B2
+            (tsPre : A2 -> Prop)
+            (precond : Rel (FrameCall frame1) (FrameCall (unary1Frame A2 B2)))
+            (RPre : SpecPreRel E1 E2 Γ1 Γ2)
+            e1 e2 (goal : _ -> Prop) :
+  IntroArg n (RPre e1 e2) goal ->
+  IntroArg n (@pushTSPreRel E1 E2 Γ1 Γ2 frame1 A2 B2
+                            tsPre precond RPre (inr e1) (inr e2)) goal.
+Proof. intro H. apply H. Qed.
+
+Polymorphic Lemma IntroArg_pushTSPostRel_inl n E1 E2 Γ1 Γ2 frame1 A2 B2
+            (tsPost : A2 -> B2 -> Prop)
+            (postcond : PostRel (FrameCall frame1) (FrameCall (unary1Frame A2 B2)))
+            (RPost : SpecPostRel E1 E2 Γ1 Γ2)
+            args1 a2 r1 b2 (goal : _ -> Prop) :
+  IntroArg n (tsPost a2 b2 /\ postcond args1 (unary1Call a2) r1 b2) goal ->
+  IntroArg n (@pushTSPostRel E1 E2 Γ1 Γ2 frame1 A2 B2
+                             tsPost postcond RPost (inl args1)
+                             (inl (mkFrameCall (unary1Frame A2 B2) 0 a2)) r1 b2) goal.
+Proof. intro H. apply H. Qed.
+
+Polymorphic Lemma IntroArg_pushTSPostRel_inr n E1 E2 Γ1 Γ2 frame1 A2 B2
+            (tsPost : A2 -> B2 -> Prop)
+            (postcond : PostRel (FrameCall frame1) (FrameCall (unary1Frame A2 B2)))
+            (RPost : SpecPostRel E1 E2 Γ1 Γ2)
+            e1 e2 r1 r2 (goal : _ -> Prop) :
+  IntroArg n (RPost e1 e2 r1 r2) goal ->
+  IntroArg n (@pushTSPostRel E1 E2 Γ1 Γ2 frame1 A2 B2
+                             tsPost postcond RPost (inr e1) (inr e2) r1 r2) goal.
+Proof. intro H. apply H. Qed.
+
+Polymorphic Lemma IntroArg_pushTSRR n frame1 A2 B2
+            (tsPost : A2 -> B2 -> Prop)
+            (postcond : PostRel (FrameCall frame1) (FrameCall (unary1Frame A2 B2)))
+            call1 a2 r1 r2 (goal : _ -> Prop) :
+  IntroArg n (tsPost a2 r2 /\ postcond call1 (unary1Call a2) r1 r2) goal ->
+  IntroArg n (@pushTSRR frame1 A2 B2 tsPost postcond call1 a2 r1 r2) goal.
+Proof. intro H. apply H. Qed.
+
+(*
+Polymorphic Lemma IntroArg_FrameCall_nil n goal :
+  IntroArg n (FrameCall nil) goal.
+Proof.
+  intro call. destruct call. destruct args. destruct x.
+Qed.
+
+Polymorphic Lemma IntroArg_FrameCall_cons n lrt frame goal :
+  IntroArg n (LRTInput lrt)
+           (fun args => goal (FrameCallOfArgs (lrt :: frame) 0 args)) ->
+  IntroArg n (FrameCall frame) (fun call => goal (consFrameCall call)) ->
+  IntroArg n (FrameCall (cons lrt frame)) goal.
+Proof.
+  intros H H0. intro call. destruct call. destruct n0.
+  - apply H.
+  - apply (H0 (FrameCallOfArgs frame n0 args)).
+Qed.
+*)
+
+(* A FrameCall whose index is guaranteed to be below a given upper bound *)
+Definition FrameCallIxBelow frame k : Type@{entree_u} :=
+  { call : FrameCall frame | FrameCallIndex call < k }.
+
+Definition incrFrameCallIxBelow {frame k} (fcib : FrameCallIxBelow frame k) :
+  FrameCallIxBelow frame (S k) :=
+  match fcib with
+  | exist _ call ix_lt => exist _ call (le_S _ _ ix_lt)
+  end.
+
+Definition mkFrameCallIxBelow {frame k} (args : LRTInput (nthLRT frame k)) :
+  FrameCallIxBelow frame (S k) :=
+  exist _ (FrameCallOfArgs _ k args) (le_n _).
+
+Polymorphic Definition IntroArg_FrameCall n frame goal :
+  IntroArg n (FrameCallIxBelow frame (length frame))
+           (fun fcib => goal (proj1_sig fcib)) ->
+  IntroArg n (FrameCall frame) goal :=
+  fun H call => H (exist _ call (FrameCallIndexLt frame call)).
+
+Polymorphic Definition IntroArg_FrameCallIxBelow0 n frame goal :
+  IntroArg n (FrameCallIxBelow frame 0) goal.
+Proof.
+  intro. destruct a. elimtype False. eapply Lt.lt_n_0. eassumption.
+Defined.
+
+Lemma le_n_equals_le_n n (pf : n <= n) : pf = le_n n.
+Proof.
+  assert (forall n m (pf : n <= m) (e : n = m),
+             pf = eq_rect n (fun x => n <= x) (le_n n) m e).
+  - clear n pf. intros n m pf. destruct pf.
+    + intros. apply eq_rect_eq_dec. apply Nat.eq_dec.
+    + intros. subst n. elimtype False.
+      eapply (Lt.lt_not_le _ _ pf). apply le_n.
+  - etransitivity; [ apply (H _ _ _ (eq_refl _)) | ].
+    symmetry. apply eq_rect_eq_dec. apply Nat.eq_dec.
+Qed.
+
+(* NOTE: this should be provable just using UIP in a manner similar to the
+above, but we use full proof irrelevance because it is easier *)
+Lemma le_S_equals_le_S n m (pf : n <= S m) (pf2 : n <= m) :
+  { pf' | pf = le_S _ _ pf' }.
+Proof.
+  exists pf2. apply proof_irrelevance.
+Qed.
+
+Polymorphic Lemma IntroArg_FrameCallIxBelowS n frame k goal :
+  IntroArg n (FrameCallIxBelow frame k)
+           (fun fcib => goal (incrFrameCallIxBelow fcib)) ->
+  IntroArg n (LRTInput (nthLRT frame k))
+           (fun args => goal (mkFrameCallIxBelow args)) ->
+  IntroArg n (FrameCallIxBelow frame (S k)) goal.
+Proof.
+  intros H H0 [ call ix_lt ].
+  destruct (le_decide _ _ (Le.le_S_n _ _ ix_lt)).
+  - destruct (le_S_equals_le_S _ _ ix_lt g) as [ pf' e ]. rewrite e.
+    apply (H (exist _ call pf')).
+  - destruct call. simpl in e; subst n0.
+    rewrite (le_n_equals_le_n _ ix_lt).
+    apply H0.
+Qed.
+
+Polymorphic Definition IntroArg_LRTInput_Ret {n R goal} :
+  goal tt -> IntroArg n (LRTInput (LRT_Ret R)) goal :=
+  fun H 'tt => H.
+
+Polymorphic Definition IntroArg_LRTInput_Fun {n A lrt goal} :
+  IntroArg n A (fun a => IntroArg n (LRTInput (lrt a)) (fun args => goal (existT _ a args))) ->
+  IntroArg n (LRTInput (LRT_Fun A lrt)) goal :=
+  fun H '(existT _ x l) => H x l.
+
+Polymorphic Definition IntroArg_LRTOutput_Ret {n R goal} :
+  IntroArg n R goal ->
+  IntroArg n (LRTOutput (LRT_Ret R) tt) goal :=
+  fun H r => H r.
+
+Polymorphic Definition IntroArg_LRTOutput_Fun {n A lrt a args goal} :
+  IntroArg n (LRTOutput (lrt a) args) goal ->
+  IntroArg n (LRTOutput (LRT_Fun A lrt) (existT _ a args)) goal :=
+  fun H r => H r.
+
+Ltac IntroArg_intro_dependent_destruction n :=
+  let e := argName n in
+    IntroArg_intro e; dependent destruction e.
+
+Ltac IntroArg_base_tac n A g :=
+  lazymatch A with
+  | (fun _ => _) _ => simple apply IntroArg_beta
+  | prod _ _ => simple apply IntroArg_prod
+  | sigT _ => simple apply IntroArg_sigT
+  | unit => simple apply IntroArg_unit
+  | _ /\ _ => simple apply IntroArg_and
+  | True => simple apply IntroArg_true
+  | False => simple apply IntroArg_false
+  | @eq (prod _ _) _ _  => simple apply IntroArg_eq_prod_const
+  | eq_rect _ _ _ _ _ = _ => simple apply IntroArg_eq_rect_const_l
+  | eq_dep1 _ _ _ _ _ _ => simple apply IntroArg_eq_dep1_const
+  | @pushPreRel _ _ _ _ _ _ _ _ (inl _) (inl _) =>
+    simple apply IntroArg_pushPreRel_inl
+  | @pushPreRel _ _ _ _ _ _ _ _ (inr _) (inr _) =>
+    simple apply IntroArg_pushPreRel_inr
+  | @pushPostRel _ _ _ _ _ _ _ _ (inl _) (inl _) _ _ =>
+    simple apply IntroArg_pushPostRel_inl
+  | @pushPostRel _ _ _ _ _ _ _ _ (inr _) (inr _) _ _ =>
+    simple apply IntroArg_pushPostRel_inr
+  | @pushTSPreRel _ _ _ _ _ _ _ _ _ _ (inl _) (inl _) =>
+    simple apply IntroArg_pushTSPreRel_inl
+  | @pushTSPreRel _ _ _ _ _ _ _ _ _ _ (inr _) (inr _) =>
+    simple apply IntroArg_pushTSPreRel_inr
+  | @pushTSPostRel _ _ _ _ _ _ _ _ _ _ (inl _) (inl _) _ _ =>
+    simple apply IntroArg_pushTSPostRel_inl
+  | @pushTSPostRel _ _ _ _ _ _ _ _ _ _ (inr _) (inr _) _ _ =>
+    simple apply IntroArg_pushTSPostRel_inr
+  | @pushTSRR _ _ _ _ _ _ _ _ _ =>
+    simple apply IntroArg_pushTSRR
+  | eqPostRel _ _ _ _ _ _ => apply IntroArg_eqPostRel
+  | true  = true  => IntroArg_intro_dependent_destruction n
+  | false = false => IntroArg_intro_dependent_destruction n
+  | true  = false => IntroArg_intro_dependent_destruction n
+  | false = true  => IntroArg_intro_dependent_destruction n
+  end.
+
+#[global] Hint Extern 101 (IntroArg ?n ?A ?g) =>
+  IntroArg_base_tac n A g : refines prepostcond.
+
+#[global] Hint Extern 101 (IntroArg ?n (FrameCall ?frame) _) =>
+  apply (@IntroArg_FrameCall n) : refines.
+#[global] Hint Extern 101 (IntroArg ?n (FrameCallIxBelow ?frame (length ?frame)) ?goal) =>
+  let k := eval cbn in (length frame) in
+  change (IntroArg n (FrameCallIxBelow frame k) goal) : refines.
+#[global] Hint Extern 101 (IntroArg ?n (FrameCallIxBelow _ 0) _) =>
+  apply (@IntroArg_FrameCallIxBelow0 n) : refines.
+#[global] Hint Extern 101 (IntroArg ?n (FrameCallIxBelow _ (S _)) _) =>
+  apply (@IntroArg_FrameCallIxBelowS n) : refines.
+
+#[global] Hint Extern 101 (IntroArg ?n (encodes ?x) ?g) =>
+  let e := argName n in IntroArg_intro e;
+  progress encodes_unfold_in e;
+  revert e; apply (IntroArg_fold n _ _) : refines.
+
+#[global] Hint Extern 101 (IntroArg ?n (LRTInput _) _) =>
+  apply IntroArg_LRTInput_Fun || apply IntroArg_LRTInput_Ret : refines prepostcond.
+#[global] Hint Extern 101 (IntroArg ?n (LRTOutput _ _) _) =>
+  apply IntroArg_LRTOutput_Fun || apply IntroArg_LRTOutput_Ret : refines prepostcond.
+
+#[global] Hint Extern 101 (IntroArg ?n (FrameCallRet ?frame ?args) ?g) =>
+  let args' := eval hnf in args in
+  let A' := eval unfold FrameCallRet in (FrameCallRet frame args') in
+  progress change (IntroArg n A' g) : refines.
+
+#[global] Hint Extern 101 (IntroArg ?n (existT _ _ _ = existT _ _ _) _) =>
+  let e1 := argName n in IntroArg_intro e1;
+  let e2 := argName n in inversion_sigma e1 as [e1 e2];
+  revert e2; apply (IntroArg_fold n _ _);
+  revert e1; apply (IntroArg_fold n _ _) : refines.
+#[global] Hint Extern 101 (IntroArg ?n (eqPreRel (existT _ _ _) (existT _ _ _)) _) =>
+  let e := argName n in IntroArg_intro e;
+  unfold eqPreRel in e;
+  revert e; apply (IntroArg_fold n _ _) : refines.
+
+#[global] Hint Extern 199 (IntroArg SAWLet _ _) =>
+  let e := argName SAWLet in IntroArg_intro e : refinesFun.
+
+#[global] Hint Extern 201 (IntroArg ?n (@eq bool _ _) _) =>
+  let e := argName n in IntroArg_intro e; rewrite e in * : refines prepostcond.
+
+#[global] Hint Extern 299 (IntroArg ?n (?x = ?y) _) =>
+  let e := argName n in IntroArg_intro e;
+    try first [ is_var x; subst x | is_var y; subst y ] : refines.
+
+#[global] Hint Extern 999 (IntroArg ?n _ _) =>
+  let e := argName n in IntroArg_intro e : refines prepostcond.
+
+
+(** Hints for Relation Goals **)
+
+(* RelGoal marks a relation goal *)
+Definition RelGoal (goal : Prop) := goal.
+
+#[global] Hint Opaque RelGoal : refines.
+
+Polymorphic Lemma RelGoal_fold goal : RelGoal goal -> goal.
+Proof. eauto. Qed.
+
+(* If nothing else works for a RelGoal, try reflexivity and then shelve it *)
+#[global] Hint Extern 999 (RelGoal _) =>
+  unfold RelGoal, lt;
+  (timeout 1 reflexivity || apply RelGoal_fold; shelve) : refines.
+
+#[global] Lemma RelGoal_and P Q :
+  RelGoal P -> RelGoal Q -> RelGoal (P /\ Q).
+Proof. split; eauto. Qed.
+
+#[global] Hint Extern 101 (RelGoal (_ /\ _)) =>
+  simple apply RelGoal_and : refines.
+
+#[global] Lemma RelGoal_beta A (f : A -> Prop) x :
+  RelGoal (f x) -> RelGoal ((fun x' => f x') x).
+Proof. eauto. Qed.
+
+#[global] Hint Extern 101 (RelGoal ((fun _ => _) _)) =>
+  simple apply RelGoal_beta : refines.
+
+Lemma RelGoal_eqPreRel_refl {E Γ e} :
+  RelGoal (@eqPreRel E Γ e e).
+Proof. constructor. Qed.
+
+#[global] Hint Extern 101 (RelGoal (eqPreRel _ _ _ _)) =>
+  apply RelGoal_eqPreRel_refl : refines.
+
+Lemma RelGoal_eq_dep1_refl {U P p x} :
+  RelGoal (eq_dep1 U P p x p x).
+Proof. unshelve econstructor; eauto. Qed.
+
+#[global] Hint Extern 101 (RelGoal (eq_dep1 _ _ _ _ _ _)) =>
+  apply RelGoal_eq_dep1_refl : refines.
+
+Polymorphic Lemma RelGoal_pushPreRel_inl E1 E2 Γ1 Γ2 frame1 frame2
+            (precond : Rel (FrameCall frame1) (FrameCall frame2))
+            (RPre : SpecPreRel E1 E2 Γ1 Γ2) e1 e2 :
+  RelGoal (precond e1 e2) ->
+  RelGoal (@pushPreRel E1 E2 Γ1 Γ2 frame1 frame2 precond RPre (inl e1) (inl e2)).
+Proof. intro H. apply H. Qed.
+
+#[global] Hint Extern 101 (RelGoal
+                             (@pushPreRel _ _ _ _ _ _ _ _ (inl _) (inl _))) =>
+  apply RelGoal_pushPreRel_inl : refines.
+
+
+Polymorphic Lemma RelGoal_pushPreRel_inr E1 E2 Γ1 Γ2 frame1 frame2
+            (precond : Rel (FrameCall frame1) (FrameCall frame2))
+            (RPre : SpecPreRel E1 E2 Γ1 Γ2) e1 e2 :
+  RelGoal (RPre e1 e2) ->
+  RelGoal (@pushPreRel E1 E2 Γ1 Γ2 frame1 frame2 precond RPre (inr e1) (inr e2)).
+Proof. intro H. apply H. Qed.
+
+#[global] Hint Extern 101 (RelGoal
+                             (@pushPreRel _ _ _ _ _ _ _ _ (inr _) (inr _))) =>
+  apply RelGoal_pushPreRel_inr : refines.
+
+
+Polymorphic Lemma RelGoal_pushPostRel_inl E1 E2 Γ1 Γ2 frame1 frame2
+            (postcond : PostRel (FrameCall frame1) (FrameCall frame2))
+            (RPost : SpecPostRel E1 E2 Γ1 Γ2)
+            (call1 : FrameCall frame1) (call2 : FrameCall frame2)
+            r1 r2 :
+  RelGoal (postcond _ _ r1 r2) ->
+  RelGoal (@pushPostRel E1 E2 Γ1 Γ2 frame1 frame2
+                           postcond RPost (inl call1) (inl call2) r1 r2).
+Proof. intro H. apply H. Qed.
+
+#[global] Hint Extern 101 (RelGoal
+                             (@pushPostRel _ _ _ _ _ _ _ _ (inl _) (inl _))) =>
+  apply RelGoal_pushPostRel_inl : refines.
+
+
+Polymorphic Lemma RelGoal_pushPostRel_inr E1 E2 Γ1 Γ2 frame1 frame2
+            (postcond : PostRel (FrameCall frame1) (FrameCall frame2))
+            (RPost : SpecPostRel E1 E2 Γ1 Γ2)
+            e1 e2 r1 r2 :
+  RelGoal (RPost _ _ r1 r2) ->
+  RelGoal (@pushPostRel E1 E2 Γ1 Γ2 frame1 frame2
+                           postcond RPost (inr e1) (inr e2) r1 r2).
+Proof. intro H. apply H. Qed.
+
+#[global] Hint Extern 101 (RelGoal
+                             (@pushPostRel _ _ _ _ _ _ _ _ (inr _) (inr _))) =>
+  apply RelGoal_pushPostRel_inr : refines.
+
+
+Polymorphic Lemma RelGoal_pushTSPreRel_inl E1 E2 Γ1 Γ2 frame1 A2 B2
+            (tsPre : A2 -> Prop)
+            (precond : Rel (FrameCall frame1) (FrameCall (unary1Frame A2 B2)))
+            (RPre : SpecPreRel E1 E2 Γ1 Γ2)
+            args1 a2 :
+  RelGoal (tsPre a2 /\ precond args1 (unary1Call a2)) ->
+  RelGoal (@pushTSPreRel E1 E2 Γ1 Γ2 frame1 A2 B2
+                            tsPre precond RPre (inl args1)
+                            (inl (mkFrameCall (unary1Frame A2 B2) 0 a2))).
+Proof. intro H. apply H. Qed.
+
+#[global] Hint Extern 101 (RelGoal
+                             (@pushTSPreRel _ _ _ _ _ _ _ _ _ _ (inl _) (inl _))) =>
+  apply RelGoal_pushTSPreRel_inl : refines.
+
+Polymorphic Lemma RelGoal_pushTSPreRel_inr E1 E2 Γ1 Γ2 frame1 A2 B2
+            (tsPre : A2 -> Prop)
+            (precond : Rel (FrameCall frame1) (FrameCall (unary1Frame A2 B2)))
+            (RPre : SpecPreRel E1 E2 Γ1 Γ2)
+            e1 e2 :
+  RelGoal (RPre e1 e2) ->
+  RelGoal (@pushTSPreRel E1 E2 Γ1 Γ2 frame1 A2 B2
+                            tsPre precond RPre (inr e1) (inr e2)).
+Proof. intro H. apply H. Qed.
+
+#[global] Hint Extern 101 (RelGoal
+                             (@pushTSPreRel _ _ _ _ _ _ _ _ _ _ (inr _) (inr _))) =>
+  apply RelGoal_pushTSPreRel_inr : refines.
+
+
+Polymorphic Lemma RelGoal_pushTSPostRel_inl E1 E2 Γ1 Γ2 frame1 A2 B2
+            (tsPost : A2 -> B2 -> Prop)
+            (postcond : PostRel (FrameCall frame1) (FrameCall (unary1Frame A2 B2)))
+            (RPost : SpecPostRel E1 E2 Γ1 Γ2)
+            args1 a2 r1 b2 :
+  RelGoal (tsPost a2 b2 /\ postcond args1 (unary1Call a2) r1 b2) ->
+  RelGoal (@pushTSPostRel E1 E2 Γ1 Γ2 frame1 A2 B2
+                             tsPost postcond RPost (inl args1)
+                             (inl (mkFrameCall (unary1Frame A2 B2) 0 a2)) r1 b2).
+Proof. intro H. apply H. Qed.
+
+#[global] Hint Extern 101 (RelGoal
+                             (@pushTSPostRel _ _ _ _ _ _ _ _ _ _ (inl _) (inl _))) =>
+  apply RelGoal_pushTSPostRel_inl : refines.
+
+
+Polymorphic Lemma RelGoal_pushTSPostRel_inr E1 E2 Γ1 Γ2 frame1 A2 B2
+            (tsPost : A2 -> B2 -> Prop)
+            (postcond : PostRel (FrameCall frame1) (FrameCall (unary1Frame A2 B2)))
+            (RPost : SpecPostRel E1 E2 Γ1 Γ2)
+            e1 e2 r1 r2 :
+  RelGoal (RPost e1 e2 r1 r2) ->
+  RelGoal (@pushTSPostRel E1 E2 Γ1 Γ2 frame1 A2 B2
+                             tsPost postcond RPost (inr e1) (inr e2) r1 r2).
+Proof. intro H. apply H. Qed.
+
+#[global] Hint Extern 101 (RelGoal
+                             (@pushTSPostRel _ _ _ _ _ _ _ _ _ _ (inr _) (inr _))) =>
+  apply RelGoal_pushTSPostRel_inr : refines.
+
+
+Polymorphic Lemma RelGoal_pushTSRR frame1 A2 B2
+            (tsPost : A2 -> B2 -> Prop)
+            (postcond : PostRel (FrameCall frame1) (FrameCall (unary1Frame A2 B2)))
+            call1 a2 r1 r2 :
+  RelGoal (tsPost a2 r2 /\ postcond call1 (unary1Call a2) r1 r2) ->
+  RelGoal (@pushTSRR frame1 A2 B2 tsPost postcond call1 a2 r1 r2).
+Proof. intro H. apply H. Qed.
+
+#[global] Hint Extern 101 (RelGoal (@pushTSRR _ _ _ _ _ _ _ _ _)) =>
+  apply RelGoal_pushTSRR : refines.
+
+
+(** Hints for Goals to Shelve **)
+
+Polymorphic Definition Shelve (A : Type) := A.
+
+#[global] Hint Opaque Shelve : refines prepostcond.
+
+Ltac Shelve_fold :=
+  match goal with
+  | |- ?A => change (Shelve A)
+  end.
+
+#[global] Hint Extern 999 (Shelve _) => shelve : refines.
+
+#[global] Hint Extern 101 (Shelve (_ /\ _)) =>
+  unfold Shelve; split; Shelve_fold : refines.
+#[global] Hint Extern 101 (Shelve ({ _ : _ & _ })) =>
+  unfold Shelve; split; Shelve_fold : refines.
+#[global] Hint Extern 101 (Shelve (_ * _)) =>
+  unfold Shelve; split; Shelve_fold : refines.
+#[global] Hint Extern 101 (Shelve unit) =>
+  unfold Shelve; exact tt : refines.
+#[global] Hint Extern 101 (Shelve True) =>
+  unfold Shelve; trivial : refines.
+
+
+(** Refinement hints using IntroArg and RelGoal **)
+
+(* RetS |= RetS *)
+Polymorphic Definition spec_refines_ret_IntroArg E1 E2 Γ1 Γ2 R1 R2 RPre RPost RR r1 r2 :
+  (RelGoal (RR r1 r2 : Prop)) ->
+  @spec_refines E1 E2 Γ1 Γ2 R1 R2 RPre RPost RR (RetS r1) (RetS r2) :=
+  spec_refines_ret E1 E2 Γ1 Γ2 R1 R2 RPre RPost RR r1 r2.
+
+#[global] Hint Extern 102 (spec_refines _ _ _ (RetS _) (RetS _)) =>
+  apply spec_refines_ret_IntroArg : refines.
+
+
+(* Monad laws *)
+
+#[global]
+Hint Extern 101 (spec_refines _ _ _ _ (RetS _ >>= _)) =>
+  simple apply spec_refines_ret_bind_r : refines.
+#[global]
+Hint Extern 101 (spec_refines _ _ _ (RetS _ >>= _) _) =>
+  simple apply spec_refines_ret_bind_l : refines.
+
+#[global]
+Hint Extern 101 (spec_refines _ _ _ _ ((_ >>= _) >>= _)) =>
+  simple apply spec_refines_bind_bind_r : refines.
+#[global]
+Hint Extern 101 (spec_refines _ _ _ ((_ >>= _) >>= _) _) =>
+  simple apply spec_refines_bind_bind_l : refines.
+
+
+(* Trigger |= Trigger *)
+
+Definition spec_refines_trigger_bind_IntroArg (E1 E2 : EncType) Γ1 Γ2 R1 R2
+      (RPre : SpecPreRel E1 E2 Γ1 Γ2) (RPost : SpecPostRel E1 E2 Γ1 Γ2)
+      RR (e1 : E1) (e2 : E2)
+      (k1 : encodes e1 -> SpecM E1 Γ1 R1)
+      (k2 : encodes e2 -> SpecM E2 Γ2 R2) :
+  RelGoal (RPre (resum e1) (resum e2)) ->
+  (IntroArg Any _ (fun a =>
+     IntroArg Any _ (fun b =>
+       IntroArg Hyp (RPost (resum e1) (resum e2) a b) (fun _ =>
+         spec_refines RPre RPost RR (k1 (resum_ret e1 a)) (k2 (resum_ret e2 b)))))) ->
+  spec_refines RPre RPost RR (TriggerS e1 >>= k1) (TriggerS e2 >>= k2) :=
+  spec_refines_trigger_bind E1 E2 Γ1 Γ2 R1 R2 RPre RPost RR e1 e2 k1 k2.
+
+#[global]
+Hint Extern 102 (spec_refines _ _ _ (TriggerS _ >>= _) (TriggerS _ >>= _)) =>
+  apply spec_refines_trigger_bind_IntroArg; resum_unfold : refines.
+
+
+(* Rules for quantifiers *)
+
+Definition spec_refines_exists_l_IntroArg E1 E2 Γ1 Γ2 R1 R2 A `{QuantType A}
+      RPre RPost RR (phi : SpecM E2 Γ2 R2) (kphi : A -> SpecM E1 Γ1 R1) :
+  (IntroArg Exists A (fun a =>spec_refines RPre RPost RR (kphi a) phi)) ->
+  spec_refines RPre RPost RR (ExistsS A >>= kphi) phi :=
+  spec_refines_exists_l E1 E2 Γ1 Γ2 R1 R2 A RPre RPost RR phi kphi.
+
+Definition spec_refines_forall_r_IntroArg E1 E2 Γ1 Γ2 R1 R2 A `{QuantType A}
+      RPre RPost RR (phi : SpecM E1 Γ1 R1) (kphi : A -> SpecM E2 Γ2 R2) :
+  (IntroArg Forall A (fun a => spec_refines RPre RPost RR phi (kphi a))) ->
+  spec_refines RPre RPost RR phi (ForallS A >>= kphi) :=
+  spec_refines_forall_r E1 E2 Γ1 Γ2 R1 R2 A RPre RPost RR phi kphi.
+
+#[global] Hint Extern 101 (spec_refines _ _ _ _ (ForallS _ >>= _)) =>
+  simple apply spec_refines_forall_r_IntroArg : refines.
+#[global] Hint Extern 101 (spec_refines _ _ _ (ExistsS _ >>= _) _) =>
+  simple apply spec_refines_exists_l_IntroArg : refines.
+
+#[global] Hint Extern 202 (spec_refines _ _ _ _ (ExistsS _ >>= _)) =>
+  unshelve simple eapply spec_refines_exists_r; [ Shelve_fold |] : refines.
+#[global] Hint Extern 202 (spec_refines _ _ _ (ForallS _ >>= _) _) =>
+  unshelve simple eapply spec_refines_forall_l; [ Shelve_fold |] : refines.
+
+
+(* Rules for assume and assert *)
+
+Definition spec_refines_assert_l_IntroArg E1 E2 Γ1 Γ2 R1 R2 (P:Prop)
+      RPre RPost RR (phi : SpecM E2 Γ2 R2) (kphi : unit -> SpecM E1 Γ1 R1) :
+  (IntroArg Assert P (fun _ => spec_refines RPre RPost RR (kphi tt) phi)) ->
+  spec_refines RPre RPost RR (AssertS P >>= kphi) phi :=
+  spec_refines_assert_l E1 E2 Γ1 Γ2 R1 R2 P RPre RPost RR phi kphi.
+
+Definition spec_refines_assume_r_IntroArg E1 E2 Γ1 Γ2 R1 R2 (P:Prop)
+      RPre RPost RR (phi : SpecM E1 Γ1 R1) (kphi : unit -> SpecM E2 Γ2 R2) :
+  (IntroArg Assume P (fun _ => spec_refines RPre RPost RR phi (kphi tt))) ->
+  spec_refines RPre RPost RR phi (AssumeS P >>= kphi) :=
+  spec_refines_assume_r E1 E2 Γ1 Γ2 R1 R2 P RPre RPost RR phi kphi.
+
+Definition spec_refines_assert_r_IntroArg E1 E2 Γ1 Γ2 R1 R2 (P:Prop)
+      RPre RPost RR (phi : SpecM E1 Γ1 R1) (kphi : unit -> SpecM E2 Γ2 R2) :
+  RelGoal P -> spec_refines RPre RPost RR phi (kphi tt) ->
+  spec_refines RPre RPost RR phi (AssertS P >>= kphi) :=
+  spec_refines_assert_r E1 E2 Γ1 Γ2 R1 R2 P RPre RPost RR phi kphi.
+
+Definition spec_refines_assume_l_IntroArg E1 E2 Γ1 Γ2 R1 R2 (P:Prop)
+      RPre RPost RR (phi : SpecM E2 Γ2 R2) (kphi : unit -> SpecM E1 Γ1 R1) :
+      RelGoal P -> spec_refines RPre RPost RR (kphi tt) phi ->
+  spec_refines RPre RPost RR (AssumeS P >>= kphi) phi :=
+  spec_refines_assume_l E1 E2 Γ1 Γ2 R1 R2 P RPre RPost RR phi kphi.
+
+#[global] Hint Extern 101 (spec_refines _ _ _ _ (AssumeS _ >>= _)) =>
+  simple apply spec_refines_assume_r_IntroArg : refines.
+#[global] Hint Extern 101 (spec_refines _ _ _ (AssertS _ >>= _) _) =>
+  simple apply spec_refines_assert_l_IntroArg : refines.
+
+#[global] Hint Extern 101 (spec_refines _ _ _ _ (AssertS _ >>= _)) =>
+  simple apply spec_refines_assert_r_IntroArg : refines.
+#[global] Hint Extern 101 (spec_refines _ _ _ (AssumeS _ >>= _) _) =>
+  simple apply spec_refines_assume_l_IntroArg : refines.
+
+
+(** * Rules for Coq quantifiers *)
+
+Lemma exists_IntroArg n A (P : A -> Prop) (goal : Prop) :
+  IntroArg Any A (fun x => IntroArg n (P x) (fun _ => goal)) ->
+  IntroArg n (exists x, P x) (fun _ => goal).
+Proof. intros H []; eapply H; eauto. Qed.
+
+#[global] Hint Extern 101 (IntroArg _ (@ex _ _) _) =>
+  simple apply exists_IntroArg : refines.
+
+Lemma exists_RelGoal A P (x : A) :
+  RelGoal (P x) -> RelGoal (exists x, P x).
+Proof. intro; econstructor; eauto. Qed.
+
+Lemma forall_RelGoal A P :
+  IntroArg Any A (fun x => RelGoal (P x)) ->
+  RelGoal (forall x, P x).
+Proof. intros H x; apply H; eauto. Qed.
+
+Lemma impl_RelGoal P Q :
+  IntroArg Hyp P (fun _ => RelGoal Q) ->
+  RelGoal (P -> Q).
+Proof. intros H x; apply H; eauto. Qed.
+
+#[global] Hint Extern 202 (RelGoal (@ex _ _)) =>
+  unshelve simple eapply exists_RelGoal; [ Shelve_fold |] : refines.
+#[global] Hint Extern 102 (RelGoal (forall _, _)) =>
+  simple apply forall_RelGoal : refines.
+#[global] Hint Extern 101 (RelGoal (_ -> _)) =>
+  simple apply impl_RelGoal : refines.
+  
+
+(* Rules for if-then-else *)
+
+Definition spec_refines_if_r_IntroArg E1 E2 Γ1 Γ2 R1 R2
+           RPre RPost RR (t1 : SpecM E1 Γ1 R1) (t2 t3 : SpecM E2 Γ2 R2) b :
+  (IntroArg If (b = true) (fun _ => spec_refines RPre RPost RR t1 t2)) ->
+  (IntroArg If (b = false) (fun _ => spec_refines RPre RPost RR t1 t3)) ->
+  spec_refines RPre RPost RR t1 (if b then t2 else t3) :=
+  spec_refines_if_r E1 E2 Γ1 Γ2 R1 R2 RPre RPost RR t1 t2 t3 b.
+
+Definition spec_refines_if_l_IntroArg E1 E2 Γ1 Γ2 R1 R2
+           RPre RPost RR (t1 t2 : SpecM E1 Γ1 R1) (t3 : SpecM E2 Γ2 R2) b :
+  (IntroArg If (b = true) (fun _ => spec_refines RPre RPost RR t1 t3)) ->
+  (IntroArg If (b = false) (fun _ => spec_refines RPre RPost RR t2 t3)) ->
+  spec_refines RPre RPost RR (if b then t1 else t2) t3 :=
+  spec_refines_if_l E1 E2 Γ1 Γ2 R1 R2 RPre RPost RR t1 t2 t3 b.
+
+#[global] Hint Extern 101 (spec_refines _ _ _ _ (if _ then _ else _)) =>
+  apply spec_refines_if_r_IntroArg : refines.
+#[global] Hint Extern 101 (spec_refines _ _ _ (if _ then _ else _) _) =>
+  apply spec_refines_if_l_IntroArg : refines.
+
+#[global] Hint Extern 101 (spec_refines _ _ _ _ ((if _ then _ else _) >>= _)) =>
+  apply spec_refines_if_bind_r : refines.
+#[global] Hint Extern 101 (spec_refines _ _ _ ((if _ then _ else _) >>= _) _) =>
+  apply spec_refines_if_bind_l : refines.
+
+
+(* Rules for pattern-matching on lists *)
+
+Definition spec_refines_match_list_r_IntroArg E1 E2 Γ1 Γ2 RPre RPost R1 R2 RR A
+           (t1 : SpecM E1 Γ1 R1) (t2 : A -> list A -> SpecM E2 Γ2 R2)
+           (t3 : SpecM E2 Γ2 R2) xs :
+  (IntroArg Any A (fun x =>
+     IntroArg Any (list A) (fun xs' =>
+       IntroArg Match (xs = x :: xs') (fun _ =>
+         spec_refines RPre RPost RR t1 (t2 x xs'))))) ->
+  (IntroArg Match (xs = nil) (fun _ => spec_refines RPre RPost RR t1 t3)) ->
+  spec_refines RPre RPost RR t1 (match xs with
+                                 | x :: xs' => t2 x xs' | nil => t3 end) :=
+  spec_refines_match_list_r E1 E2 Γ1 Γ2 RPre RPost R1 R2 RR A t1 t2 t3 xs.
+
+Definition spec_refines_match_list_l_IntroArg E1 E2 Γ1 Γ2 RPre RPost R1 R2 RR A
+           (t3 : SpecM E2 Γ2 R2)
+           (t1 : A -> list A -> SpecM E1 Γ1 R1) (t2 : SpecM E1 Γ1 R1) xs :
+  (IntroArg Any A (fun x =>
+     IntroArg Any (list A) (fun xs' =>
+       IntroArg Match (xs = x :: xs') (fun _ =>
+         spec_refines RPre RPost RR (t1 x xs') t3)))) ->
+  (IntroArg Match (xs = nil) (fun _ => spec_refines RPre RPost RR t2 t3)) ->
+  spec_refines RPre RPost RR (match xs with
+                              | x :: xs' => t1 x xs' | nil => t2 end) t3 :=
+  spec_refines_match_list_l E1 E2 Γ1 Γ2 RPre RPost R1 R2 RR A t3 t1 t2 xs.
+
+#[global]
+Hint Extern 101 (spec_refines _ _ _ _ (match _ with | _ :: _ => _ | nil => _ end)) =>
+  apply spec_refines_match_list_r_IntroArg : refines.
+#[global]
+Hint Extern 101 (spec_refines _ _ _ (match _ with | _ :: _ => _ | nil => _ end) _) =>
+  apply spec_refines_match_list_l_IntroArg : refines.
+
+#[global]
+Hint Extern 101 (spec_refines _ _ _ _ ((match _ with | _ :: _ => _ | nil => _ end) >>= _)) =>
+  apply spec_refines_match_list_bind_r : refines.
+#[global]
+Hint Extern 101 (spec_refines _ _ _ ((match _ with | _ :: _ => _ | nil => _ end) >>= _) _) =>
+  apply spec_refines_match_list_bind_l : refines.
+
+
+(* Rules for pattern-matching on pairs *)
+
+Definition spec_refines_match_pair_r_IntroArg E1 E2 Γ1 Γ2 RPre RPost R1 R2 RR A B
+           (t1 : SpecM E1 Γ1 R1) (t2 : A -> B -> SpecM E2 Γ2 R2) pr :
+  (IntroArg Any A (fun x =>
+     IntroArg Any B (fun y =>
+       IntroArg Match (pr = (x, y)) (fun _ =>
+         spec_refines RPre RPost RR t1 (t2 x y))))) ->
+  spec_refines RPre RPost RR t1 (match pr with | (x,y) => t2 x y end) :=
+  spec_refines_match_pair_r E1 E2 Γ1 Γ2 RPre RPost R1 R2 RR A B t1 t2 pr.
+
+Definition spec_refines_match_pair_l_IntroArg E1 E2 Γ1 Γ2 RPre RPost R1 R2 RR A B
+           (t1 : A -> B -> SpecM E1 Γ1 R1) (t2 : SpecM E2 Γ2 R2) pr :
+  (IntroArg Any A (fun x =>
+     IntroArg Any B (fun y =>
+       IntroArg Match (pr = (x, y)) (fun _ =>
+         spec_refines RPre RPost RR (t1 x y) t2)))) ->
+  spec_refines RPre RPost RR (match pr with | (x,y) => t1 x y end) t2 :=
+  spec_refines_match_pair_l E1 E2 Γ1 Γ2 RPre RPost R1 R2 RR A B t1 t2 pr.
+
+#[global]
+Hint Extern 101 (spec_refines _ _ _ _ (match _ with | (_,_) => _ end)) =>
+  apply spec_refines_match_pair_r_IntroArg : refines.
+#[global]
+Hint Extern 101 (spec_refines _ _ _ (match _ with | (_,_) => _ end) _) =>
+  apply spec_refines_match_pair_l_IntroArg : refines.
+
+#[global]
+Hint Extern 101 (spec_refines _ _ _ _ ((match _ with | (_,_) => _ end) >>= _)) =>
+  apply spec_refines_match_pair_bind_r : refines.
+#[global]
+Hint Extern 101 (spec_refines _ _ _ ((match _ with | (_,_) => _ end) >>= _) _) =>
+  apply spec_refines_match_pair_bind_l : refines.
+
+
+(** * Rules for liftStackS  *)
+
+Lemma spec_refines_liftStackS_ret_bind_l (E1 E2 : EncType) Γ1 Γ2 R1 R2
+  (RPre : SpecPreRel E1 E2 Γ1 Γ2) (RPost : SpecPostRel E1 E2 Γ1 Γ2)
+  (RR : Rel R1 R2) A1 a k1 t2 :
+  spec_refines RPre RPost RR (k1 a) t2 ->
+  spec_refines RPre RPost RR (liftStackS A1 (RetS a) >>= k1) t2.
+Proof.
+  intros. setoid_rewrite resumEntree_Ret. setoid_rewrite bind_ret_l.
+  auto.
+Qed.
+
+Lemma spec_refines_liftStackS_bind_bind_l (E1 E2 : EncType) Γ1 Γ2 R1 R2
+  (RPre : SpecPreRel E1 E2 Γ1 Γ2) (RPost : SpecPostRel E1 E2 Γ1 Γ2)
+  (RR : Rel R1 R2) A1 B1 t1 k1 k2 t2 :
+  spec_refines RPre RPost RR (x <- liftStackS A1 t1 ;; liftStackS B1 (k1 x) >>= k2) t2 ->
+  spec_refines RPre RPost RR (liftStackS B1 (t1 >>= k1) >>= k2) t2.
+Proof.
+  intros. setoid_rewrite resumEntree_bind. setoid_rewrite bind_bind. eauto.
+Qed.
+
+Lemma spec_refines_liftStackS_assume_bind_l (E1 E2 : EncType) Γ1 Γ2 R1 R2
+  (RPre : SpecPreRel E1 E2 Γ1 Γ2) (RPost : SpecPostRel E1 E2 Γ1 Γ2)
+  (RR : Rel R1 R2) P k1 t2 :
+  spec_refines RPre RPost RR (AssumeS P >>= k1) t2 ->
+  spec_refines RPre RPost RR (liftStackS _ (AssumeS P) >>= k1) t2.
+Proof.
+  intros.
+  enough (@liftStackS E1 Γ1 unit (AssumeS P) ≅ AssumeS P).
+  rewrite H0. auto.
+  setoid_rewrite resumEntree_Vis.
+  setoid_rewrite bind_vis. cbn. apply eqit_Vis.
+  cbn. intros. rewrite bind_ret_l. setoid_rewrite resumEntree_Ret. 
+  apply eqit_Ret. auto.
+Qed.
+
+Lemma spec_refines_liftStackS_assert_bind_l (E1 E2 : EncType) Γ1 Γ2 R1 R2
+  (RPre : SpecPreRel E1 E2 Γ1 Γ2) (RPost : SpecPostRel E1 E2 Γ1 Γ2)
+  (RR : Rel R1 R2) P k1 t2 :
+  spec_refines RPre RPost RR (AssertS P >>= k1) t2 ->
+  spec_refines RPre RPost RR (liftStackS _ (AssertS P) >>= k1) t2.
+Proof.
+  intros.
+  enough (@liftStackS E1 Γ1 unit (AssertS P) ≅ AssertS P).
+  rewrite H0. auto.
+  setoid_rewrite resumEntree_Vis.
+  setoid_rewrite bind_vis. cbn. apply eqit_Vis.
+  cbn. intros. rewrite bind_ret_l. setoid_rewrite resumEntree_Ret. 
+  apply eqit_Ret. auto.
+Qed.
+
+Lemma spec_refines_liftStackS_forall_bind_l (E1 E2 : EncType) Γ1 Γ2 R1 R2
+  (RPre : SpecPreRel E1 E2 Γ1 Γ2) (RPost : SpecPostRel E1 E2 Γ1 Γ2)
+  (RR : Rel R1 R2) A1 `{QuantType A1} k1 t2 :
+  spec_refines RPre RPost RR (ForallS A1 >>= k1) t2 ->
+  spec_refines RPre RPost RR (liftStackS _ (ForallS A1) >>= k1) t2.
+Proof.
+  intros.
+  enough (@liftStackS E1 Γ1 A1 (ForallS A1) ≅ ForallS A1).
+  rewrite H1. auto.
+  setoid_rewrite resumEntree_Vis.
+  apply eqit_Vis.
+  cbn. intros. setoid_rewrite resumEntree_Ret. apply eqit_Ret. 
+  auto.
+Qed.
+
+Lemma spec_refines_liftStackS_exists_bind_l (E1 E2 : EncType) Γ1 Γ2 R1 R2
+  (RPre : SpecPreRel E1 E2 Γ1 Γ2) (RPost : SpecPostRel E1 E2 Γ1 Γ2)
+  (RR : Rel R1 R2) A1 `{QuantType A1} k1 t2 :
+  spec_refines RPre RPost RR (ExistsS A1 >>= k1) t2 ->
+  spec_refines RPre RPost RR (liftStackS _ (ExistsS A1) >>= k1) t2.
+Proof.
+  intros.
+  enough (@liftStackS E1 Γ1 A1 (ExistsS A1) ≅ ExistsS A1).
+  rewrite H1. auto.
+  setoid_rewrite resumEntree_Vis.
+  apply eqit_Vis.
+  cbn. intros. setoid_rewrite resumEntree_Ret. apply eqit_Ret. 
+  auto.
+Qed.
+
+#[global] Hint Extern 101 (spec_refines _ _ _ (liftStackS _ (RetS _) >>= _) _) =>
+  simple apply spec_refines_liftStackS_ret_bind_l : refines.
+#[global] Hint Extern 101 (spec_refines _ _ _ (liftStackS _ (_ >>= _) >>= _) _) =>
+  simple apply spec_refines_liftStackS_bind_bind_l : refines.
+#[global] Hint Extern 101 (spec_refines _ _ _ (liftStackS _ (AssumeS _) >>= _) _) =>
+  simple apply spec_refines_liftStackS_assume_bind_l : refines.
+#[global] Hint Extern 101 (spec_refines _ _ _ (liftStackS _ (AssertS _) >>= _) _) =>
+  simple apply spec_refines_liftStackS_assert_bind_l : refines.
+#[global] Hint Extern 101 (spec_refines _ _ _ (liftStackS _ (ForallS _) >>= _) _) =>
+  simple apply spec_refines_liftStackS_forall_bind_l : refines.
+#[global] Hint Extern 101 (spec_refines _ _ _ (liftStackS _ (ExistsS _) >>= _) _) =>
+  simple apply spec_refines_liftStackS_exists_bind_l : refines.
+
+#[global] Hint Extern 101 (spec_refines _ _ _ (liftStackS _ (total_spec _ _ _) >>= _) _) =>
+  apply spec_refines_liftStackS_bind_bind_l : refines.
+
+Lemma spec_refines_liftStackS_bind_ret_l (E1 E2 : EncType) Γ1 Γ2 frame1 frame2 R1 R2
+      (RPre : SpecPreRel E1 E2 (frame1 :: Γ1) (frame2 :: Γ2))
+      (RPost : SpecPostRel E1 E2 (frame1 :: Γ1) (frame2 :: Γ2))
+      t1 t2 (RR : Rel R1 R2) :
+  spec_refines RPre RPost RR (liftStackS _ t1 >>= RetS) t2 ->
+  spec_refines RPre RPost RR (liftStackS _ t1) t2.
+Proof. intro; rewrite <- (bind_ret_r (liftStackS _ _)); eauto. Qed.
+
+#[global] Hint Extern 101 (spec_refines _ _ _ (liftStackS _ ?t1) _) =>
+  simple apply (spec_refines_liftStackS_bind_ret_l _ _ _ _ _ _ _ _ _ _ t1) : refines.
+
+
+Lemma spec_refines_liftStackS_proper:
+  forall (E1 : EncType) (Γ1 : list RecFrame) (frame1 : RecFrame) (R1 : Type) (t1 t2 : SpecM E1 nil R1),
+    spec_refines eqPreRel eqPostRel eq t1 t2 ->
+    spec_refines eqPreRel eqPostRel eq (@liftStackS E1 (frame1 :: Γ1) R1 t1) (liftStackS R1 t2).
+Proof.
+  intros E1 Γ1 frame1 R1 t1 t2 H. 
+  enough (strict_refines  (@liftStackS E1 (frame1 :: Γ1) R1 t1) (liftStackS R1 t2)).
+  {
+    eapply padded_refines_monot; try apply H0; auto.
+    intros. red in PR. dependent destruction PR. subst. cbn. constructor.
+  }
+  apply padded_refines_liftStackS_proper.
+  eapply padded_refines_monot; try apply H; auto.
+  intros. dependent destruction PR. red. econstructor.
+  Unshelve. all : auto. simpl. auto.
+Qed.
+
+(* I think this is backwards *)
+Lemma spec_refines_liftStackS_trans_bind_l {E1 E2 Γ1 Γ2 frame1 frame2 R1 R2}
+      {RPre : SpecPreRel E1 E2 (frame1 :: Γ1) (frame2 :: Γ2)}
+      {RPost : SpecPostRel E1 E2 (frame1 :: Γ1) (frame2 :: Γ2)}
+      {RR : Rel R1 R2} {A t1 t2 k1 t3} :
+  spec_refines eqPreRel eqPostRel eq t1 t2 ->
+  spec_refines RPre RPost RR (liftStackS A t2 >>= k1) t3 ->
+  spec_refines RPre RPost RR (liftStackS A t1 >>= k1) t3.
+Proof.
+  intros.
+  assert (spec_refines eqPreRel eqPostRel eq (@liftStackS E1 (frame1 :: Γ1) A t1) (liftStackS A t2)).
+  apply spec_refines_liftStackS_proper. auto.
+  eapply padded_refines_weaken_r; try eapply H0.
+  eapply padded_refines_bind with (RR := eq).
+  - red in H1. eapply padded_refines_monot; try apply H1; auto.
+    intros. dependent destruction PR. red. econstructor. auto. Unshelve. 2 : auto.
+    cbn. auto.
+  - intros. subst. reflexivity.
+Qed.
+
+Create HintDb refines_proofs.
+#[global] Hint Extern 201 (spec_refines _ _ _ (liftStackS _ _ >>= _) _) =>
+  (simple eapply spec_refines_liftStackS_trans_bind_l;
+   [ typeclasses eauto with refines_proofs |]) || shelve : refines.
+
+
+(** * Refinement Hints About Recursion *)
+
+Polymorphic Definition WellFoundedRelation A := sig (@well_founded A).
+Polymorphic Definition PreAndPostConditions frame1 frame2 : Type :=
+  Rel (FrameCall frame1) (FrameCall frame2) *
+  PostRel (FrameCall frame1) (FrameCall frame2).
+Polymorphic Definition from_user {A} {x : A} := x.
+
+Polymorphic Definition wfRelOf {A} :
+  WellFoundedRelation A -> Rel A A := @proj1_sig _ (@well_founded A).
+Polymorphic Definition preOf {frame1 frame2} :
+  PreAndPostConditions frame1 frame2 ->
+  Rel (FrameCall frame1) (FrameCall frame2) := fst.
+Polymorphic Definition postOf {frame1 frame2} :
+  PreAndPostConditions frame1 frame2 ->
+  PostRel (FrameCall frame1) (FrameCall frame2) := snd.
+
+Definition Continue {precond : Prop} {goal1 goal2} : Type :=
+  precond * goal1 * goal2.
+
+Lemma Continue_unfold precond goal1 goal2 :
+  RelGoal precond -> goal1 -> goal2 ->
+  @Continue precond goal1 goal2.
+Proof. split; eauto. Qed.
+Ltac Continue_unfold := simple apply Continue_unfold.
+
+#[global] Hint Opaque WellFoundedRelation : refines prepostcond.
+#[global] Hint Opaque PreAndPostConditions : refines prepostcond.
+#[global] Hint Opaque Continue : refines prepostcond.
+
+#[global] Hint Extern 999 (WellFoundedRelation _) => shelve : refines prepostcond.
+#[global] Hint Extern 999 (PreAndPostConditions _ _) => shelve : refines prepostcond.
+#[global] Hint Extern 999 (Continue) => shelve : refines prepostcond.
+
+Lemma spec_refines_multifix_bind_IntroArg (E1 E2 : EncType) Γ1 Γ2 frame1 frame2 R1 R2
+      (RPre : SpecPreRel E1 E2 Γ1 Γ2) (RPost : SpecPostRel E1 E2 Γ1 Γ2) RR
+      (bodies1 : FrameTuple E1 (frame1 :: Γ1) frame1)
+      (bodies2 : FrameTuple E2 (frame2 :: Γ2) frame2)
+      (call1 : FrameCall frame1) (call2 : FrameCall frame2)
+      (k1 : FrameCallRet frame1 call1 -> SpecM E1 Γ1 R1)
+      (k2 : FrameCallRet frame2 call2 -> SpecM E2 Γ2 R2)
+      (prepostconds : PreAndPostConditions frame1 frame2) :
+  @Continue (preOf prepostconds call1 call2)
+            (IntroArg Call _ (fun call1' => IntroArg Call _ (fun call2' =>
+              IntroArg Hyp (preOf prepostconds call1' call2') (fun _ =>
+              spec_refines (pushPreRel (preOf prepostconds) RPre)
+                           (pushPostRel (postOf prepostconds) RPost)
+                           (postOf prepostconds call1' call2')
+                           (applyFrameTuple _ _ _ bodies1 call1')
+                           (applyFrameTuple _ _ _ bodies2 call2')))))
+            (IntroArg RetAny _ (fun r1 => IntroArg RetAny _ (fun r2 =>
+              IntroArg Hyp (postOf prepostconds call1 call2 r1 r2) (fun _ =>
+              spec_refines RPre RPost RR (k1 r1) (k2 r2))))) ->
+  spec_refines RPre RPost RR
+               (MultiFixS E1 Γ1 frame1 bodies1 call1 >>= k1)
+               (MultiFixS E2 Γ2 frame2 bodies2 call2 >>= k2).
+Proof.
+  destruct prepostconds; intros [[]].
+  unfold IntroArg in *; eapply spec_refines_multifix_bind; eauto.
+Qed.
+
+Lemma spec_refines_multifix_IntroArg (E1 E2 : EncType) Γ1 Γ2 frame1 frame2
+      (RPre : SpecPreRel E1 E2 Γ1 Γ2) (RPost : SpecPostRel E1 E2 Γ1 Γ2)
+      (bodies1 : FrameTuple E1 (frame1 :: Γ1) frame1)
+      (bodies2 : FrameTuple E2 (frame2 :: Γ2) frame2)
+      (call1 : FrameCall frame1) (call2 : FrameCall frame2)
+      (RR : Rel (encodes call1) (encodes call2))
+      (prepostconds : PreAndPostConditions frame1 frame2) :
+  @Continue (preOf prepostconds call1 call2)
+            (IntroArg RetAny _ (fun r1 => IntroArg RetAny _ (fun r2 =>
+              IntroArg Hyp (postOf prepostconds call1 call2 r1 r2) (fun _ =>
+              RelGoal (RR r1 r2)))))
+            (IntroArg Call _ (fun call1' => IntroArg Call _ (fun call2' =>
+              IntroArg Hyp (preOf prepostconds call1' call2') (fun _ =>
+              spec_refines (pushPreRel (preOf prepostconds) RPre)
+                           (pushPostRel (postOf prepostconds) RPost)
+                           (postOf prepostconds call1' call2')
+                           (applyFrameTuple _ _ _ bodies1 call1')
+                           (applyFrameTuple _ _ _ bodies2 call2'))))) ->
+  spec_refines RPre RPost RR
+               (MultiFixS E1 Γ1 frame1 bodies1 call1)
+               (MultiFixS E2 Γ2 frame2 bodies2 call2).
+Proof.
+  destruct prepostconds; intros [[]].
+  unfold IntroArg in *; eapply spec_refines_multifix; eauto.
+Qed.
+
+Lemma spec_refines_total_spec_IntroArg (E1 E2 : EncType) Γ1 Γ2 frame1
+      A2 B2 `{QuantType A2} `{QuantType B2}
+      (RPre : SpecPreRel E1 E2 Γ1 Γ2) (RPost : SpecPostRel E1 E2 Γ1 Γ2)
+      (bodies1 : FrameTuple E1 (frame1 :: Γ1) frame1)
+      (call1 : FrameCall frame1) (a2 : A2)
+      (RR : Rel (FrameCallRet frame1 call1) B2)
+      (tsPre : A2 -> Prop) (tsPost : A2 -> B2 -> Prop)
+      (rdec : WellFoundedRelation A2)
+      (prepostconds : PreAndPostConditions frame1 (unary1Frame A2 B2)) :
+  @Continue (preOf prepostconds call1 (unary1Call a2))
+            (IntroArg RetAny _ (fun r1 => IntroArg RetAny _ (fun r2 =>
+              IntroArg Hyp (tsPost a2 r2) (fun _ =>
+              IntroArg Hyp (postOf prepostconds call1 (unary1Call a2) r1 r2) (fun _ =>
+              RelGoal (RR r1 r2))))))
+            (IntroArg Call _ (fun call1' => IntroArg Any _ (fun a2' =>
+              IntroArg Hyp (preOf prepostconds call1' (unary1Call a2')) (fun _ =>
+              spec_refines (pushTSPreRel tsPre (preOf prepostconds) RPre)
+                           (pushTSPostRel tsPost (postOf prepostconds) RPost)
+                           (pushTSRR tsPost (postOf prepostconds) call1' a2')
+                           (applyFrameTuple _ _ _ bodies1 call1')
+                           (total_spec_fix_body tsPre tsPost (wfRelOf rdec) a2'))))) ->
+  spec_refines RPre RPost RR
+               (MultiFixS E1 Γ1 frame1 bodies1 call1)
+               (total_spec tsPre tsPost a2).
+Proof.
+  destruct rdec, prepostconds; intros [[]].
+  unfold IntroArg, RelGoal in *; simpl in *.
+  unshelve eapply spec_refines_total_spec; eauto.
+Qed.
+
+#[global]
+Hint Extern 101 (spec_refines ?RPre ?RPost ?RR
+                              (MultiFixS ?E1 ?Γ1 ?frame1 ?bodies1 ?call1 >>= ?k1)
+                              (MultiFixS ?E2 ?Γ2 ?frame2 ?bodies2 ?call2 >>= ?k2)) =>
+  unshelve (
+    let HPrePost := fresh "HPrePost" in
+    epose (HPrePost := from_user (A:=PreAndPostConditions frame1 frame2));
+    apply (spec_refines_multifix_bind_IntroArg E1 E2 Γ1 Γ2 frame1 frame2 _ _
+              RPre RPost RR bodies1 bodies2 call1 call2 k1 k2 HPrePost)) : refines.
+#[global]
+Hint Extern 101 (spec_refines ?RPre ?RPost ?RR
+                              (MultiFixS ?E1 ?Γ1 ?frame1 ?bodies1 ?call1)
+                              (MultiFixS ?E2 ?Γ2 ?frame2 ?bodies2 ?call2)) =>
+  unshelve (
+    let HPrePost := fresh "HPrePost" in
+    epose (HPrePost := from_user (A:=PreAndPostConditions frame1 frame2));
+    apply (spec_refines_multifix_IntroArg E1 E2 Γ1 Γ2 frame1 frame2
+              RPre RPost bodies1 bodies2 call1 call2 RR HPrePost)) : refines.
+#[global]
+Hint Extern 101 (spec_refines ?RPre ?RPost ?RR
+                              (MultiFixS ?E1 ?Γ1 ?frame1 ?bodies1 ?call1)
+                              (@total_spec ?E2 ?Γ2 ?A2 ?B2 _ ?tsPre ?tsPost ?a2)) =>
+  unshelve (
+    let HWf := fresh "HWf" in
+    epose (HWf := from_user (A:=WellFoundedRelation A2));
+    let HPrePost := fresh "HPrePost" in
+    epose (HPrePost := from_user (A:=PreAndPostConditions frame1 (unary1Frame A2 B2)));
+    apply (spec_refines_total_spec_IntroArg E1 E2 Γ1 Γ2 frame1 A2 B2
+              RPre RPost bodies1 call1 a2 RR tsPre tsPost HWf HPrePost));
+  unfold total_spec_fix_body : refines.
+
+Lemma spec_refines_call_bind_IntroArg (E1 E2 : EncType) Γ1 Γ2 frame1 frame2 R1 R2
+      (RPre : SpecPreRel E1 E2 (frame1 :: Γ1) (frame2 :: Γ2))
+      (RPost : SpecPostRel E1 E2 (frame1 :: Γ1) (frame2 :: Γ2))
+      RR (call1 : FrameCall frame1) (call2 : FrameCall frame2)
+      (k1 : FrameCallRet frame1 call1 -> SpecM E1 (frame1 :: Γ1) R1)
+      (k2 : FrameCallRet frame2 call2 -> SpecM E2 (frame2 :: Γ2) R2) :
+  RelGoal (RPre (inl call1) (inl call2)) ->
+  (IntroArg RetAny _ (fun r1 => IntroArg RetAny _ (fun r2 =>
+   IntroArg Hyp (RPost (inl call1) (inl call2) r1 r2) (fun _ =>
+   spec_refines RPre RPost RR (k1 (resum_ret call1 r1)) (k2 (resum_ret call2 r2)))))) ->
+  spec_refines RPre RPost RR (CallS _ _ _ call1 >>= k1) (CallS _ _ _ call2 >>= k2).
+Proof. apply spec_refines_call_bind. Qed.
+
+Lemma spec_refines_call_IntroArg (E1 E2 : EncType) Γ1 Γ2 frame1 frame2
+      (RPre : SpecPreRel E1 E2 (frame1 :: Γ1) (frame2 :: Γ2))
+      (RPost : SpecPostRel E1 E2 (frame1 :: Γ1) (frame2 :: Γ2))
+      (call1 : FrameCall frame1) (call2 : FrameCall frame2)
+      (RR : Rel (FrameCallRet frame1 call1) (FrameCallRet frame2 call2)) :
+  RelGoal (RPre (inl call1) (inl call2)) ->
+  IntroArg RetAny _ (fun r1 => IntroArg RetAny _ (fun r2 =>
+   IntroArg Hyp (RPost (inl call1) (inl call2) r1 r2) (fun _ =>
+   RelGoal (RR r1 r2)))) ->
+  spec_refines RPre RPost RR (CallS _ _ _ call1) (CallS _ _ _ call2).
+Proof. intros; apply spec_refines_call; eauto. Qed.
+
+#[global] Hint Extern 101 (spec_refines _ _ _ (CallS _ _ _ _ >>= _) (CallS _ _ _ _ >>= _)) =>
+  apply spec_refines_call_bind_IntroArg; resum_unfold : refines.
+#[global] Hint Extern 101 (spec_refines _ _ _ (CallS _ _ _ _) (CallS _ _ _ _)) =>
+  apply spec_refines_call_IntroArg : refines.
+
+#[global] Hint Extern 102 (spec_refines _ _ _ (CallS _ _ _ ?call1) _) =>
+  simple apply (spec_refines_call_bind_ret_l _ _ _ _ _ _ _ _ _ call1) : refines.
+#[global] Hint Extern 102 (spec_refines _ _ _ _ (CallS _ _ _ ?call2)) =>
+  simple apply (spec_refines_call_bind_ret_r _ _ _ _ _ _ _ _ _ _ _ call2) : refines.
+
+#[global] Hint Extern 991 (spec_refines _ _ _ (CallS _ _ _ _ >>= _) (trepeat _ _)) =>
+  simple apply spec_refines_trepeat_suc_r : refines.
+#[global] Hint Extern 991 (spec_refines _ _ _ (CallS _ _ _ _ >>= _) (trepeat _ _ >>= _)) =>
+  simple apply spec_refines_trepeat_bind_suc_r : refines.
+
+#[global] Hint Extern 992 (spec_refines _ _ _ _ (trepeat _ _)) =>
+  simple apply spec_refines_trepeat_zero_r : refines.
+#[global] Hint Extern 992 (spec_refines _ _ _ _ (trepeat _ _ >>= _)) =>
+  simple apply spec_refines_trepeat_bind_zero_r : refines.
+
+#[global] Hint Extern 101 (spec_refines ?RPre ?RPost ?RR
+                                        (applyFrameTuple ?E ?Γ ?frame ?bodies ?call) ?t2) =>
+  let call' := eval hnf in call in
+  let frame' := eval cbv in frame in
+  let t1' := eval cbv [ applyFrameTuple nthLRT nth_default'
+                        lrtApply nthFrameTupleFun fst snd ]
+                   in (applyFrameTuple E Γ frame' bodies call') in
+  progress change (spec_refines RPre RPost RR t1' t2) : refines.
+#[global] Hint Extern 101 (spec_refines ?RPre ?RPost ?RR ?t1
+                                        (applyFrameTuple ?E ?Γ ?frame ?bodies ?call)) =>
+  let call' := eval hnf in call in
+  let frame' := eval cbv in frame in
+  let t2' := eval cbv [ applyFrameTuple nthLRT nth_default'
+                        lrtApply nthFrameTupleFun fst snd ]
+                   in (applyFrameTuple E Γ frame' bodies call') in
+  progress change (spec_refines RPre RPost RR t1 t2') : refines.
+
+(** * Tactics for proving refinement *)
+
+Ltac unfold_RelGoal_goals :=
+  match goal with
+  | |- RelGoal _ => unfold RelGoal
+  | |- _ => idtac
+  end.
+
+Ltac prove_refinement_rewrite :=
+  match goal with
+  | |- spec_refines _ _ _ _ _ => idtac
+  | |- _ => try unshelve rewrite_strat (bottomup (hints refines))
+  end.
+
+Ltac prove_refinement_prepostcond :=
+  unshelve typeclasses eauto with prepostcond;
+  unfold_RelGoal_goals; cbn [ FrameCallIndex ];
+  prove_refinement_rewrite.
+
+Tactic Notation "prove_refinement_eauto_then" tactic(tac) :=
+  unshelve typeclasses eauto with refines;
+  match goal with
+  | |- Shelve _ => unfold Shelve; shelve
+  | |- RelGoal _ => tac
+  | |- _ => idtac
+  end.
+
+Ltac prove_refinement_eauto :=
+  (prove_refinement_eauto_then (prove_refinement_eauto_then idtac)).
+
+Ltac prove_refinement_solve :=
+  try solve [ assumption | reflexivity | contradiction ].
+
+Variant ProveRefOpt := NoRewrite | NoSolve.
+
+Definition in_opts (o : ProveRefOpt) (os : list ProveRefOpt) : bool.
+Proof.
+  refine (proj1_sig (bool_of_sumbool (in_dec _ o os))).
+  destruct x, y ; (left; reflexivity) || (right; discriminate).
+Defined.
+
+Ltac prove_refinement_with opts :=
+  prove_refinement_eauto; unfold_RelGoal_goals;
+  let noRewrite := eval vm_compute in (in_opts NoRewrite opts) in
+  first [ constr_eq_strict noRewrite true | prove_refinement_rewrite ];
+  let noSolve := eval vm_compute in (in_opts NoSolve opts) in
+  first [ constr_eq_strict noSolve true | prove_refinement_solve   ].
+
+Ltac prove_refinement :=
+  prove_refinement_with (@nil ProveRefOpt).
+Tactic Notation "prove_refinement" "with" constr(o) :=
+  prove_refinement_with (cons o nil).
+Tactic Notation "prove_refinement" "with" constr(o1) constr(o2) :=
+  prove_refinement_with (cons o1 (cons o2 nil)).
+
+Ltac prove_refinement_continue :=
+  Continue_unfold; prove_refinement.
+Tactic Notation "prove_refinement_continue" "with" constr(o) :=
+  Continue_unfold; prove_refinement with o.
+Tactic Notation "prove_refinement_continue" "with" constr(o1) constr(o2) :=
+  Continue_unfold; prove_refinement with o1 o2.
+
+
+(** * Tactics for pre/post-conditions and well-founded relations *)
+
+Definition DecreasingNat {A} (_ : A) := nat.
+#[global] Hint Opaque DecreasingNat : prepostcond.
+#[global] Hint Extern 999 (DecreasingNat _) => shelve : prepostcond.
+
+Tactic Notation "wellfounded_decreasing_nat" :=
+  let f := fresh "f" in
+  enough (IntroArg Any _ DecreasingNat) as f
+    by (exact (exist _ (fun a b => f a < f b) (well_founded_ltof _ f)));
+  prove_refinement_prepostcond.
+Tactic Notation "wellfounded_decreasing_nat" uconstr(f) :=
+  exact (exist _ (fun a b => f a < f b) (well_founded_ltof _ f)).
+
+Definition well_founded_False {A} :
+  @well_founded A (fun _ _ => False).
+Proof. constructor; contradiction. Defined.
+
+Ltac wellfounded_none :=
+  exact (exist _ (fun _ _ => False) well_founded_False).
+
+Polymorphic Definition PreCase {frame1 frame2} i j
+  (a1 : LRTInput (nthLRT frame1 i))
+  (a2 : LRTInput (nthLRT frame2 j)) := Prop.
+Polymorphic Definition PostCase {frame1 frame2} i j args1 args2
+  (r1 : LRTOutput (nthLRT frame1 i) args1)
+  (r2 : LRTOutput (nthLRT frame2 j) args2) := Prop.
+
+#[global] Hint Opaque PreCase : prepostcond.
+#[global] Hint Opaque PostCase : prepostcond.
+
+#[global] Hint Extern 999 (PreCase _ _ _ _) => shelve : prepostcond.
+#[global] Hint Extern 999 (PostCase _ _ _ _ _ _) => shelve : prepostcond.
+
+Polymorphic Definition prepost_case {frame1 frame2} i j
+  (pre : IntroArg Any (LRTInput (nthLRT frame1 i)) (fun a1 =>
+         IntroArg Any (LRTInput (nthLRT frame2 j)) (fun a2 =>
+         PreCase i j a1 a2)))
+  (post : IntroArg Any _ (fun args1 => IntroArg Any _ (fun args2 =>
+          IntroArg RetAny (LRTOutput (nthLRT frame1 i) args1) (fun r1 =>
+          IntroArg RetAny (LRTOutput (nthLRT frame2 j) args2) (fun r2 =>
+          PostCase i j args1 args2 r1 r2)))))
+  (prepostcond : PreAndPostConditions frame1 frame2) :
+  PreAndPostConditions frame1 frame2.
+Proof.
+  unfold IntroArg, PreCase, PostCase in *; split.
+  all: intros [m args1] [n args2].
+  all: destruct (Nat.eq_dec m i) as [p1|];
+       [ destruct p1; destruct (Nat.eq_dec n j) as [p2|];
+                      [ destruct p2 |] |].
+  1: apply pre; eauto.
+  1-2: exact (preOf prepostcond (FrameCallOfArgs _ m args1)
+                                (FrameCallOfArgs _ n args2)).
+  1: apply post; eauto.
+  1-2: exact (postOf prepostcond (FrameCallOfArgs _ m args1)
+                                 (FrameCallOfArgs _ n args2)).
+Defined.
+
+Notation eqPreCase :=
+  (fun (args1 : LRTInput (nthLRT _ _)) (args2 : LRTInput (nthLRT _ _)) =>
+       eq args1 args2)
+  (only parsing).
+Notation eqPostCase :=
+  (ltac:(intros args1 args2 r1 r2;
+         apply (eq_dep1 _ _ args1 r1 args2 r2)))
+  (only parsing).
+
+Tactic Notation "prepost_case" constr(i) constr(j) :=
+  apply (prepost_case i j); prove_refinement_prepostcond.
+Tactic Notation "prepost_case" constr(i) constr(j) "withPre" uconstr(pre) :=
+  apply (prepost_case i j); [ exact pre | prove_refinement_prepostcond |].
+Tactic Notation "prepost_case" constr(i) constr(j) "withPost" uconstr(post) :=
+  apply (prepost_case i j); [ prove_refinement_prepostcond | exact post |].
+Tactic Notation "prepost_case" constr(i) constr(j) "with" uconstr(pre) "," uconstr(post) :=
+  apply (prepost_case i j); [exact pre | exact post |].
+
+Definition PreExcludedCase (i j : nat) := False.
+Definition PostExcludedCase (i j : nat) := False.
+
+#[global] Hint Extern 101 (IntroArg ?n (PreExcludedCase _ _) _) =>
+  apply IntroArg_false : refines.
+#[global] Hint Extern 101 (IntroArg ?n (PostExcludedCase _ _) _) =>
+ apply IntroArg_false : refines.
+
+Tactic Notation "prepost_exclude_case" constr(i) constr(j) :=
+  apply (prepost_case i j); [ exact (fun _ _ => PreExcludedCase i j)
+                            | exact (fun _ _ _ _ => PostExcludedCase i j)].
+Tactic Notation "prepost_exclude_remaining" :=
+  exact (fun calli callj => PreExcludedCase (FrameCallIndex calli) (FrameCallIndex callj),
+         fun calli callj _ _ => PostExcludedCase (FrameCallIndex calli) (FrameCallIndex callj)).
+
+Ltac wf_pre_post_IntroArg_unfold A :=
+  let A' := eval cbv [ wfRelOf proj1_sig preOf fst postOf snd prepost_case
+                       Nat.eq_dec nat_rec nat_rect f_equal_nat f_equal
+                       IntroArg_prod IntroArg_sigT IntroArg_unit IntroArg_FrameCall
+                       IntroArg_FrameCallIxBelow0
+                       IntroArg_LRTInput_Fun IntroArg_LRTInput_Ret
+                       IntroArg_LRTOutput_Fun IntroArg_LRTOutput_Ret ]
+              in A in A'.
+
+#[global] Hint Extern 101 (IntroArg ?n (wfRelOf ?H ?a1 ?a2) ?g) =>
+  let H' := eval unfold H, from_user in H in
+  let A' := wf_pre_post_IntroArg_unfold (wfRelOf H' a1 a2) in
+  progress change (IntroArg n A' g) : refines.
+#[global] Hint Extern 101 (RelGoal (wfRelOf ?H ?a1 ?a2)) =>
+  let H' := eval unfold H, from_user in H in
+  let A' := wf_pre_post_IntroArg_unfold (wfRelOf H' a1 a2) in
+  progress change (RelGoal A') : refines.
+
+#[global] Hint Extern 101 (IntroArg ?n (preOf ?H ?call1 ?call2) ?g) =>
+  let H' := eval unfold H, from_user in H in
+  let call1' := eval hnf in call1 in
+  let call2' := eval hnf in call2 in
+  let A' := wf_pre_post_IntroArg_unfold (preOf H' call1' call2') in
+  progress change (IntroArg n A' g) : refines.
+#[global] Hint Extern 101 (RelGoal (preOf ?H ?call1 ?call2)) =>
+  let H' := eval unfold H, from_user in H in
+  let call1' := eval hnf in call1 in
+  let call2' := eval hnf in call2 in
+  let A' := wf_pre_post_IntroArg_unfold (preOf H' call1' call2') in
+  progress change (RelGoal A') : refines.
+
+#[global] Hint Extern 101 (IntroArg ?n (postOf ?H ?call1 ?call2 ?r1 ?r2) ?g) =>
+  let H' := eval unfold H, from_user in H in
+  let call1' := eval hnf in call1 in
+  let call2' := eval hnf in call2 in
+  let A' := wf_pre_post_IntroArg_unfold (postOf H' call1' call2' r1 r2) in
+  progress change (IntroArg n A' g) : refines.
+#[global] Hint Extern 101 (RelGoal (postOf ?H ?call1 ?call2 ?r1 ?r2)) =>
+  let H' := eval unfold H, from_user in H in
+  let call1' := eval hnf in call1 in
+  let call2' := eval hnf in call2 in
+  let A' := wf_pre_post_IntroArg_unfold (postOf H' call1' call2' r1 r2)  in
+  progress change (RelGoal A') : refines.
+
+
+(** * Testing *)
+
+Open Scope nat_scope.
+
+Lemma test_ifs E x :
+  @spec_refines E E nil nil eqPreRel eqPostRel nat nat eq
+                  (if 0 <=? x then if x <? 256 then RetS 1 else RetS 0 else RetS 0)
+                  (if x <? 256 then if 0 <=? x then RetS 1 else RetS 0 else RetS 0).
+Proof.
+  prove_refinement.
+Qed.
+
+Lemma test_exists E x y :
+  @spec_refines E E nil nil eqPreRel eqPostRel nat nat eq
+                  (RetS ((x+1) + (y+2)))
+                  ('(x', y') <- ExistsS (nat * nat) ;; RetS (x' + y')).
+Proof.
+  prove_refinement.
+Qed.
+
+Lemma test_spins E (x : nat) :
+  @spec_refines E E nil nil eqPreRel eqPostRel nat nat eq
+                  (MultiFixS E nil (unary1Frame nat nat)
+                    ((fun a => CallS _ _ _ (mkFrameCall (unary1Frame nat nat) 0 a)), tt)
+                    (mkFrameCall (unary1Frame nat nat) 0 x))
+                  (MultiFixS E nil (unary1Frame nat nat)
+                    ((fun a => CallS _ _ _ (mkFrameCall (unary1Frame nat nat) 0 a)), tt)
+                    (mkFrameCall (unary1Frame nat nat) 0 x)).
+Proof.
+  prove_refinement.
+  - prepost_case 0 0 with eqPreCase, eqPostCase.
+    prepost_exclude_remaining.
+  - prove_refinement_continue.
+Qed.
+
+Definition testFrame1 : RecFrame :=
+  LRT_Fun nat (fun _ => LRT_Ret nat) :: LRT_Fun nat (fun _ => LRT_Ret nat) :: nil.
+
+Lemma test_spins_rets E (x : nat) :
+  @spec_refines E E nil nil eqPreRel eqPostRel nat nat eq
+                  (MultiFixS E nil testFrame1
+                    ((fun a => CallS _ _ _ (mkFrameCall testFrame1 0 a)),
+                     ((fun a => RetS a), tt))
+                    (mkFrameCall testFrame1 1 x))
+                  (MultiFixS E nil testFrame1
+                    ((fun a => RetS a),
+                     ((fun a => CallS _ _ _ (mkFrameCall testFrame1 1 a)), tt))
+                    (mkFrameCall testFrame1 0 x)).
+Proof.
+  prove_refinement.
+  - prepost_case 1 0 with eqPreCase, eqPostCase.
+    prepost_case 0 1 with eqPreCase, eqPostCase.
+    prepost_exclude_remaining.
+  - prove_refinement_continue.
+Qed.
+
+Lemma test_total_spec_easy E (x : nat) :
+  @spec_refines E E nil nil eqPreRel eqPostRel nat nat eq
+                  (MultiFixS E nil (unary1Frame nat nat)
+                    ((fun a => RetS (a + 1)), tt)
+                    (mkFrameCall (unary1Frame nat nat) 0 x))
+                  (total_spec (fun _ => True)
+                              (fun a b => b = (a + 1)) x).
+Proof.
+  prove_refinement.
+  - wellfounded_none.
+  - prepost_case 0 0 withPre eqPreCase; [ exact (r = r0) |].
+    prepost_exclude_remaining.
+  - prove_refinement_continue.
+Qed.
+
+Lemma test_total_spec_loop E (x : nat) :
+  @spec_refines E E nil nil eqPreRel eqPostRel nat nat eq
+                  (MultiFixS E nil (unary1Frame nat nat)
+                    ((fun a => if a =? 0 then RetS 0
+                               else a' <- CallS _ _ _ (mkFrameCall (unary1Frame nat nat)
+                                                      0 (pred a)) ;;
+                                    RetS (S a')), tt)
+                    (mkFrameCall (unary1Frame nat nat) 0 x))
+                  (total_spec (fun _ => True)
+                              (fun a b => a = b) x).
+Proof.
+  prove_refinement.
+  - wellfounded_decreasing_nat; exact a.
+  - prepost_case 0 0 withPre eqPreCase; [ exact (r = r0) |].
+    prepost_exclude_remaining.
+  - prove_refinement_continue.
+    + apply Nat.eqb_eq in e_if; eauto.
+    + destruct a; [ discriminate e_if | eauto ].
+    + destruct a; [ discriminate e_if | eauto ].
+Qed.
+
+(* 
+Lemma test_total_spec_less_easy E (x : nat) :
+  @spec_refines E E nil nil eqPreRel eqPostRel nat nat eq
+                  (MultiFixS E nil testFrame1
+                    ((fun a => CallS _ _ _ (mkFrameCall testFrame1 1 (a + 1))),
+                     ((fun a => RetS (a + 1)), tt))
+                    (mkFrameCall testFrame1 1 x))
+                  (total_spec (fun _ => True)
+                              (fun a b => a = (b + 2)) x).
+Proof.
+  prove_refinement.
+  - wellfounded_none.
+  - prepost_case 0 0 withPre eqPreCase.
+    { simpl; intros. exact () } *)
