src/ITreeSpec/Concrete.v
@@ -1,0 +1,125 @@
+From Stdlib Require Import
+     Program
+     Setoid
+     Morphisms
+     Relations.
+
+From Paco Require Import paco.
+
+From ITree Require Import
+     Basics.Basics
+     Basics.Utils
+     Basics.HeterogeneousRelations
+     Basics.Monad
+     Basics.HeterogeneousRelations
+     Core.ITreeDefinition
+     Eq.Eqit
+     Eq.Paco2.
+
+From ITreeSpec Require Import
+     ITreeSpecDefinition
+     ITreeSpecFacts.
+
+Local Open Scope itree_scope.
+
+
+
+Inductive isConcreteF {E R} (F : itree_spec E R -> Prop) :
+  itree_spec' E R -> Prop :=
+  | isConcrete_Ret (r : R) : isConcreteF F (RetF r)
+  | isConcrete_Tau (phi : itree_spec E R) :
+      F phi -> isConcreteF F (TauF phi)
+  | isConcrete_Vis {X} (e : E X) kphi :
+      (forall a, F (kphi a)) -> isConcreteF F (VisF (Spec_vis e) kphi).
+
+Hint Constructors isConcreteF.
+Definition isConcrete_ {E R} F (t: itree_spec E R) : Prop :=
+  isConcreteF F (observe t).
+
+Lemma monotone_isConcreteF {E R} (ot : itree_spec' E R) sim sim'
+  (LE : sim <1= sim')
+  (IN : isConcreteF sim ot) :
+  isConcreteF sim' ot.
+Proof.
+  induction IN; eauto.
+Qed.
+
+Lemma monotone_isConcrete_ {E R} : monotone1 (@isConcrete_ E R).
+Proof. red. intros. eapply monotone_isConcreteF; eauto. Qed.
+
+Hint Resolve monotone_isConcrete_ : paco.
+
+Definition isConcrete {E R} : itree_spec E R -> Prop := paco1 isConcrete_ bot1.
+
+Lemma isConcreteVisInv {E R X} (e : E X) (k : _ -> itree_spec E R) a :
+  isConcrete (Vis (Spec_vis e) k) -> isConcrete (k a).
+Proof.
+  intro isc; punfold isc. inversion isc.
+  assert (kphi0 = k); [ inj_existT; assumption | ].
+  subst. pclearbot.
+  apply H0.
+Qed.
+
+
+Variant voidE : Type -> Type := .
+
+Section non_padded_completeness_counter.
+  Definition top1 : itree_spec voidE unit :=
+    ITree.bind (assume_spec False) (fun _ => Ret tt).
+
+  Lemma top1_top : forall (t : itree_spec voidE unit) RPre RPost RR,
+      refines RPre RPost RR t top1.
+  Proof.
+    intros. pstep. red. cbn. constructor. cbn. intros [].
+  Qed.
+
+
+  Definition top2 : itree_spec voidE unit :=
+    ITree.bind (exists_spec bool) (fun b => if b then Ret tt else ITree.spin).
+  Context (Hdec : forall (t : itree_spec voidE unit), isConcrete t -> eutt eq t (Ret tt) \/ eutt eq t ITree.spin).
+
+
+  Lemma top2_top : forall (t : itree_spec voidE unit) RPre RPost,
+      isConcrete t ->
+      refines RPre RPost eq t top2.
+  Proof.
+    intros. specialize (Hdec t H). destruct Hdec; clear H Hdec; rename H0 into Ht.
+    - punfold Ht. red in Ht. cbn in Ht. pstep. red.
+      remember (RetF tt) as x.
+      hinduction Ht before t; intros; inv Heqx; eauto.
+      + unfold top2.
+        cbn.
+        apply refinesF_existsR with (a:=true).
+        cbn.
+        constructor; auto.
+      + constructor. auto.
+    - pstep. red. cbn.
+      apply refinesF_existsR with (a:=false).
+      cbn.
+      constructor. pstep_reverse.
+      generalize dependent t. pcofix CIH. intros t Ht.
+      pstep. red. punfold Ht. red in Ht. remember (observe ITree.spin) as x.
+      hinduction Ht before r; intros; inv Heqx; pclearbot; eauto.
+      + constructor. eauto.
+      + cbn. constructor. left. pstep. red. eapply IHHt; eauto.
+  Qed.
+
+
+  Lemma not_refines_top1_top2 RPre RPost RR : ~ refines RPre RPost RR top1 top2.
+    Proof.
+      intro Hcontra. punfold Hcontra. red in Hcontra.
+      inversion Hcontra.
+      - cbn in *. destruct a; cbn in *.
+        + inj_existT. subst.
+          cbn in *.
+          inv H1.
+          contradiction.
+        + inj_existT. subst. cbn in *. clear Hcontra.
+          remember (TauF ITree.spin) as y.
+          remember (VisF (Spec_forall False)
+                      (fun x : False =>
+                         ITree.subst (fun _ : () => Ret ()) (ITree.subst (fun _ : False => Ret ()) (Ret x)))) as x.
+          hinduction H1 before RR; intros; inv Heqx; try inv Heqy; eauto.
+      - destruct a.
+    Qed.
+End non_padded_completeness_counter.
