src/ITreeSpec/LetRecRefines.v
@@ -1,0 +1,1287 @@
+From Stdlib Require Export
+  Datatypes
+  Arith.PeanoNat
+  Arith.Peano_dec
+  Arith.Compare
+  Wf_nat
+  Morphisms
+  Setoid
+  Program.Equality
+  Lists.List
+  Logic.Eqdep_dec
+  Logic.EqdepFacts
+  Eqdep EqdepFacts
+  Logic.ProofIrrelevance.
+
+From ITree Require Import
+  Basics.HeterogeneousRelations
+  Eq.Eqit.
+
+From ITreeSpec Require Import
+  ITreeSpecDefinition
+  ITreeSpecFacts
+  ITreeSpecCombinatorFacts
+  RecSpecFix
+  SpecM
+  MRecSpec.
+
+From Paco Require Import paco.
+
+Export SigTNotations.
+Import SpecMNotations.
+Local Open Scope entree_scope.
+
+
+(*** Pre- and Post-condition relations for SpecM ***)
+
+Definition SpecPreRel (E1 E2 : EvType) stk1 stk2 :=
+  Rel (FunStackE E1 stk1) (FunStackE E2 stk2).
+Definition SpecPostRel (E1 E2 : EvType) stk1 stk2 :=
+  PostRel (FunStackE E1 stk1) (FunStackE E2 stk2).
+
+(* The precondition requiring events on both sides to be equal *)
+Definition eqPreRel {E stk} : SpecPreRel E E stk stk := eq.
+
+(* The postcondition requiring return values on both sides to be equal *)
+Definition eqPostRel {E stk} : SpecPostRel E E stk stk :=
+  fun e1 e2 a1 a2 => eq_dep1 _ _ e1 a1 e2 a2.
+
+
+
+(*** The definition of letrec refinement ***)
+Section lr_refines.
+
+Context {E1 E2 : EvType} {stk1 stk2 : FunStack} {R1 R2 : Type}.
+Context (funs1 : StackTuple E1 stk1 stk1) (funs2 : StackTuple E2 stk2 stk2).
+
+Context (RPre : SpecPreRel E1 E2 stk1 stk2)
+  (RPost : SpecPostRel E1 E2 stk1 stk2) (RR : R1 -> R2 -> Prop).
+
+Inductive lr_refinesF (sim : SpecM E1 stk1 R1 -> SpecM E2 stk2 R2 -> Prop) : SpecM' E1 stk1 R1 -> SpecM' E2 stk2 R2 -> Prop :=
+
+(* Ret |= Ret *)
+| lr_refinesF_Ret r1 r2 : RR r1 r2 -> lr_refinesF sim (RetF r1) (RetF r2)
+
+(* t1 |= t2 => Tau t1 |= Tau t2 *)
+| lr_refinesF_Tau t1 t2 : sim t1 t2 -> lr_refinesF sim (TauF t1) (TauF t2)
+
+(* RPre e1 e2 -> (forall a b, RPost e1 e2 a b -> k1 a |= k2 b) ->
+   Vis e1 k1 |= Vis e2 k2 *)
+| lr_refinesF_Vis e1 e2 k1 k2 :
+  RPre e1 e2 -> (forall a b, RPost e1 e2 a b -> sim (k1 a) (k2 b)) ->
+  lr_refinesF sim (VisF (Spec_vis e1) k1) (VisF (Spec_vis e2) k2)
+
+(* t1 |= t2 => Tau t1 |= t2 *)
+| lr_refinesF_TauL t1 ot2 : lr_refinesF sim (observe t1) ot2 ->
+                            lr_refinesF sim (TauF t1) ot2
+
+(* t1 |= t2 => t1 |= Tau t2 *)
+| lr_refinesF_TauR ot1 t2 : lr_refinesF sim ot1 (observe t2) ->
+                            lr_refinesF sim ot1 (TauF t2)
+
+(* (forall a, t1 |= k a) => t1 |= Forall k *)
+| lr_refinesF_forallR A ot1 k : (forall a, lr_refinesF sim ot1 (TauF (k a))) ->
+                                lr_refinesF sim ot1 (VisF (Spec_forall A) k)
+
+(* (exists a, t1 |= k a) => t1 |= Exists k *)
+| lr_refinesF_existsR A ot1 k a : lr_refinesF sim ot1 (TauF (k a)) ->
+                                  lr_refinesF sim ot1 (VisF (Spec_exists A) k)
+
+(* (exists a, k a |= t2) => Forall k |= t2 *)
+| lr_refinesF_forallL A ot2 k a : lr_refinesF sim (TauF (k a)) ot2 ->
+                                  lr_refinesF sim (VisF (Spec_forall A) k) ot2
+
+(* (forall a, k a |= t2) => Exists k |= t2 *)
+| lr_refinesF_existsL A ot2 k : (forall a, lr_refinesF sim (TauF (k a)) ot2) ->
+                                lr_refinesF sim (VisF (Spec_exists A) k) ot2
+
+(* apply funs1 call1 >>= k1 |= t2 => CallS call1 >>= k1 |= t2 *)
+| lr_refinesF_unfoldL call1 k1 ot2 :
+    lr_refinesF sim (TauF (applyStackTuple E1 stk1 funs1 call1 >>= k1)) ot2 ->
+    lr_refinesF sim (VisF (Spec_vis (inl call1)) k1) ot2
+
+(* t1 |= apply funs2 call2 >>= k2 => t1 |= CallS call2 >>= k2 *)
+| lr_refinesF_unfoldR ot1 call2 k2 :
+    lr_refinesF sim ot1 (TauF (applyStackTuple E2 stk2 funs2 call2 >>= k2)) ->
+    lr_refinesF sim ot1 (VisF (Spec_vis (inl call2)) k2)
+.
+
+
+(** The standard Paco nonsense **)
+
+Hint Constructors lr_refinesF : entree_spec.
+
+Definition lr_refines_ sim : SpecM E1 stk1 R1 -> SpecM E2 stk2 R2 -> Prop :=
+  fun t1 t2 => lr_refinesF sim (observe t1) (observe t2).
+
+Lemma monotone_lr_refinesF ot1 ot2 sim sim' (LE : sim <2= sim')
+      (IN : lr_refinesF sim ot1 ot2) : lr_refinesF sim' ot1 ot2.
+Proof with eauto with entree_spec.
+  induction IN...
+Qed.
+
+Lemma monotone_lr_refines_: monotone2 lr_refines_.
+Proof. red. intros. eapply monotone_lr_refinesF; eauto. Qed.
+
+(* lr_refines is the coinductive closure of lr_refinesF *)
+Definition lr_refines := paco2 lr_refines_ bot2.
+
+(* The unfolding of lr_refines to an lr_refinesF *)
+Definition lr_refinesF_u := lr_refinesF (upaco2 lr_refines_ bot2).
+
+End lr_refines.
+
+Global Hint Resolve monotone_lr_refines_ : paco.
+
+
+
+(*** Pre/post conditions on SpecM events ***)
+
+(* Lift a relation on FunStackE events from the nil stack to arbitrary ones *)
+Definition liftNilRel {E1 E2 stk1 stk2}
+  (R : Rel (FunStackE E1 pnil) (FunStackE E2 pnil)) :
+  Rel (FunStackE E1 stk1) (FunStackE E2 stk2) :=
+  fun e1 e2 => match e1,e2 with
+               | inr e1', inr e2' => R (inr e1') (inr e2')
+               | _,_ => False
+               end.
+
+(* Lift a postcondition on FunStackE events from the nil stack to arbitrary ones *)
+Definition liftNilPostRel {E1 E2 stk1 stk2}
+  (R : PostRel (FunStackE E1 pnil) (FunStackE E2 pnil)) :
+  PostRel (FunStackE E1 stk1) (FunStackE E2 stk2) :=
+  fun e1 e2 => match e1,e2 with
+               | inr e1', inr e2' => R (inr e1') (inr e2')
+               | _,_ => fun _ _ => False
+               end.
+
+(* Compose two liftNilRel proofs *)
+Lemma liftNilRel_compose {E1 E2 E3 stk1 stk2 stk3} R12 R23 x y z :
+  @liftNilRel E1 E2 stk1 stk2 R12 x y ->
+  @liftNilRel E2 E3 stk2 stk3 R23 y z ->
+  liftNilRel (rcompose R12 R23) x z.
+Proof.
+  intros. destruct x; destruct y; destruct z; cbn in *; try contradiction.
+  eexists; split; eassumption.
+Qed.
+
+Lemma elim_RComposePostRel {E1 E2 E3} `{EncodingType E1} `{EncodingType E2}
+  `{EncodingType E3} {R1 : Rel E1 E2} {R2 : Rel E2 E3}
+  {RPost1 RPost2 a b c x z} :
+  R1 a b -> R2 b c ->
+  RComposePostRel R1 R2 RPost1 RPost2 a c x z ->
+  exists y, RPost1 a b x y /\ RPost2 b c y z.
+Proof.
+  intros. destruct H4. apply H4; assumption.
+Qed.
+
+(* Destruct the composition of two liftNilPostRel proofs *)
+Lemma liftNilPostRel_compose_elim {E1 E2 E3 stk1 stk2 stk3 R12 R23 RPost12 RPost23}
+  {e1 : FunStackE E1 stk1} {e2 : FunStackE E2 stk2} {e3 : FunStackE E3 stk3} {x z} :
+  liftNilRel R12 e1 e2 -> liftNilRel R23 e2 e3 ->
+  liftNilPostRel (RComposePostRel R12 R23 RPost12 RPost23) e1 e3 x z ->
+  exists y:encodes e2,
+    liftNilPostRel RPost12 e1 e2 x y /\ liftNilPostRel RPost23 e2 e3 y z.
+Proof.
+  intros. destruct e1; destruct e2; destruct e3; cbn in *; try contradiction.
+  destruct (elim_RComposePostRel H H0 H1). destruct H2.
+  eexists; split; eassumption.
+Qed.
+
+(* Add a precondition for recursive calls *)
+Definition addCallPreRel {E1 E2 : EvType} {stk1 stk2}
+           (precond : Rel (StackCall stk1) (StackCall stk2))
+           (RPre : Rel (FunStackE E1 pnil) (FunStackE E2 pnil)) :
+  Rel (FunStackE E1 stk1) (FunStackE E2 stk2) :=
+  fun a1 a2 => match a1,a2 with
+               | inl args1, inl args2 => precond args1 args2
+               | inr ev1, inr ev2 => RPre (inr ev1) (inr ev2)
+               | _, _ => False
+               end.
+
+(* Add a postcondition for recursive calls *)
+Definition addCallPostRel {E1 E2 : EvType} {stk1 stk2}
+           (postcond : PostRel (StackCall stk1) (StackCall stk2))
+           (RPost : PostRel (FunStackE E1 pnil) (FunStackE E2 pnil)) :
+  PostRel (FunStackE E1 stk1) (FunStackE E2 stk2) :=
+  fun a1 a2 => match a1,a2 with
+               | inl args1, inl args2 => postcond args1 args2
+               | inr ev1, inr ev2 => RPost (inr ev1) (inr ev2)
+               | _, _ => fun _ _ => False
+               end.
+
+
+(*** Inversion lemmas about refinement ***)
+Section lr_refines_inv.
+Context {E1 E2 : EvType} {stk1 stk2 : FunStack} {R1 R2 : Type}.
+Context (funs1 : StackTuple E1 stk1 stk1) (funs2 : StackTuple E2 stk2 stk2).
+
+Context (RPre : Rel (FunStackE E1 stk1) (FunStackE E2 stk2))
+  (RPost : PostRel (FunStackE E1 stk1) (FunStackE E2 stk2))
+  (RR : R1 -> R2 -> Prop).
+
+(* Invert a Tau on the left of a refinement *)
+Lemma lr_refines_TauL_inv t1 t2 :
+  lr_refines funs1 funs2 RPre RPost RR (Tau t1) t2 ->
+  lr_refines funs1 funs2 RPre RPost RR t1 t2.
+Proof.
+  remember (TauF t1) as x.
+  intro. punfold H. red in H. simpl in H. pfold. red.
+  remember (observe t2) as ot2.
+  clear t2 Heqot2.
+  induction H; inversion Heqx.
+  - pclearbot. constructor. pstep_reverse. rewrite <- H1.
+    eapply paco2_mon; [ eassumption | ]. intros x0 x1 b; destruct b.
+  - rewrite <- H1. eapply monotone_lr_refinesF; [ | eassumption ].
+    intros. pclearbot. left. eapply paco2_mon; [ eassumption | ].
+    intros. contradiction.
+  - constructor. apply IHlr_refinesF. assumption.
+  - constructor. intros. apply H0. assumption.
+  - econstructor. apply IHlr_refinesF. assumption.
+  - constructor. apply IHlr_refinesF. assumption.
+Qed.
+
+(* Invert a Tau on the left of an unfolded lr_refinesF refinement *)
+Lemma lr_refinesF_TauL_inv t1 t2 :
+  lr_refinesF_u funs1 funs2 RPre RPost RR (TauF t1) (observe t2) ->
+  lr_refinesF_u funs1 funs2 RPre RPost RR (observe t1) (observe t2).
+Proof.
+  unfold lr_refinesF_u.
+  intros. pstep_reverse. apply lr_refines_TauL_inv. pstep. assumption.
+Qed.
+
+(* Invert a Tau on the right of a refinement *)
+Lemma lr_refines_TauR_inv t1 t2 :
+  lr_refines funs1 funs2 RPre RPost RR t1 (Tau t2) ->
+  lr_refines funs1 funs2 RPre RPost RR t1 t2.
+Proof.
+  remember (TauF t2) as x.
+  intro. punfold H. red in H. simpl in H. pfold. red.
+  remember (observe t1) as ot1. clear t1 Heqot1.
+  induction H; inversion Heqx.
+  - pclearbot. constructor. pstep_reverse. rewrite <- H1.
+    eapply paco2_mon; [ eassumption | ]. intros x0 x1 b; destruct b.
+  - constructor. apply IHlr_refinesF. assumption.
+  - rewrite <- H1. eapply monotone_lr_refinesF; [ | eassumption ].
+    intros. pclearbot. left. eapply paco2_mon; [ eassumption | ].
+    intros. contradiction.
+  - econstructor. apply IHlr_refinesF. assumption.
+  - constructor. intros. apply H0. assumption.
+  - constructor. apply IHlr_refinesF. assumption.
+Qed.
+
+(* Invert a Tau on the right of an unfolded lr_refinesF refinement *)
+Lemma lr_refinesF_TauR_inv t1 t2 :
+  lr_refinesF_u funs1 funs2 RPre RPost RR (observe t1) (TauF t2) ->
+  lr_refinesF_u funs1 funs2 RPre RPost RR (observe t1) (observe t2).
+Proof.
+  unfold lr_refinesF_u.
+  intros. pstep_reverse. apply lr_refines_TauR_inv. pstep. apply H.
+Qed.
+
+(* Invert a refinement with a forall on the right to a unviversal *)
+Lemma lr_refines_forallR_inv A t1 k2 :
+  lr_refines funs1 funs2 RPre RPost RR
+    t1 (Vis (@Spec_forall (FunStackE E2 stk2) A) k2) ->
+  forall a, lr_refines funs1 funs2 RPre RPost RR t1 (Tau (k2 a)).
+Proof.
+  intros ref12 a. punfold ref12. red in ref12. cbn in ref12. pstep. red.
+  remember (observe t1) as ot1; clear t1 Heqot1.
+  remember (VisF (Spec_forall A) k2) as ot2.
+  induction ref12; try discriminate.
+  - apply lr_refinesF_TauL. apply IHref12. assumption.
+  - inversion Heqot2. revert k Heqot2 H H0 H3; rewrite H2; intros.
+    inj_existT. rewrite H3 in H. apply H.
+  - eapply lr_refinesF_forallL. apply IHref12. assumption.
+  - apply lr_refinesF_existsL. intros. apply H0. assumption.
+  - apply lr_refinesF_unfoldL. apply IHref12. assumption.
+Qed.
+
+
+(* Invert a refinement with an exists on the left to a unviversal *)
+Lemma lr_refines_existsL_inv A k1 t2 :
+  lr_refines funs1 funs2 RPre RPost RR
+    (Vis (@Spec_exists (FunStackE E1 stk1) A) k1) t2 ->
+  forall a, lr_refines funs1 funs2 RPre RPost RR (Tau (k1 a)) t2.
+Proof.
+  intros ref12 a. punfold ref12. red in ref12. cbn in ref12. pstep. red.
+  remember (observe t2) as ot2; clear t2 Heqot2.
+  remember (VisF (Spec_exists A) k1) as ot1.
+  induction ref12; try discriminate.
+  - apply lr_refinesF_TauR. apply IHref12. assumption.
+  - apply lr_refinesF_forallR. intros. apply H0. assumption.
+  - eapply lr_refinesF_existsR. apply IHref12. assumption.
+  - inversion Heqot1. revert k Heqot1 ot2 H a H0 H3; rewrite H2; intros.
+    inj_existT. rewrite H3 in H. apply H.
+  - apply lr_refinesF_unfoldR. apply IHref12. assumption.
+Qed.
+
+
+(* The result of inverting a refinement with a forall on the left, which could
+take 0 or more right-hand side steps before the forallL rule. Note that the Taus
+in the quantifier rules are removed in this definition, because this is needed
+in the transitivity proof. *)
+Inductive forallL_LRRefinesF {A : QuantEnc} (k1 : encodes A -> SpecM E1 stk1 R1)
+  : SpecM' E2 stk2 R2 -> Prop :=
+  | forallL_LRRefinesF_forallL t (a : encodes A) :
+    lr_refinesF_u funs1 funs2 RPre RPost RR (TauF (k1 a)) t ->
+    forallL_LRRefinesF k1 t
+  | forallL_LRRefinesF_forallR (B : QuantEnc) k2 :
+    (forall b, forallL_LRRefinesF k1 (observe (k2 b))) ->
+    forallL_LRRefinesF k1 (VisF (Spec_forall B) k2)
+  | forallL_LRRefinesF_existsR B k2 (b : encodes B) :
+    forallL_LRRefinesF k1 (observe (k2 b)) ->
+    forallL_LRRefinesF k1 (VisF (Spec_exists B : SpecEvent (FunStackE _ _)) k2)
+  | forallL_LRRefinesF_TauR t2 :
+    forallL_LRRefinesF k1 (observe t2) ->
+    forallL_LRRefinesF k1 (TauF t2)
+  | forallL_LRRefinesF_unfoldR call2 k2 :
+    forallL_LRRefinesF k1 (observe (applyStackTuple E2 stk2 funs2 call2 >>= k2)) ->
+    forallL_LRRefinesF k1 (VisF (Spec_vis (inl call2)) k2)
+.
+
+(* Helper lemma to invert a Tau in a forallL_LRRefinesF *)
+Lemma forallL_LRRefinesF_TauL_inv A k1 t2 :
+  @forallL_LRRefinesF A k1 (TauF t2) ->
+  @forallL_LRRefinesF A k1 (observe t2).
+Proof.
+  intro H. remember (TauF t2) as tau_t2.
+  revert t2 Heqtau_t2; induction H; intros; try discriminate.
+  - subst t. eapply forallL_LRRefinesF_forallL. red. observe_tau. pstep_reverse.
+    apply lr_refines_TauR_inv. pstep. apply H.
+  - inversion Heqtau_t2. subst t0. assumption.
+Qed.
+
+(* Invert a refinement of a forall on the left to a forallL_LRRefinesF *)
+Lemma lr_refinesF_forallL_inv A k1 t2 :
+  lr_refinesF_u funs1 funs2 RPre RPost RR
+    (VisF (@Spec_forall (FunStackE E1 stk1) A) k1) t2 ->
+  forallL_LRRefinesF k1 t2.
+Proof.
+  intros. remember (VisF (Spec_forall A) k1) as ot1.
+  induction H; try discriminate.
+  - apply forallL_LRRefinesF_TauR; apply IHlr_refinesF; assumption.
+  - apply forallL_LRRefinesF_forallR; intros.
+    apply forallL_LRRefinesF_TauL_inv. apply H0. assumption.
+  - eapply forallL_LRRefinesF_existsR.
+    apply forallL_LRRefinesF_TauL_inv.
+    apply IHlr_refinesF. assumption.
+  - inversion Heqot1. subst A0. inj_existT. subst k.
+    eapply forallL_LRRefinesF_forallL. apply H.
+  - apply forallL_LRRefinesF_unfoldR. apply forallL_LRRefinesF_TauL_inv.
+    apply IHlr_refinesF. assumption.
+Qed.
+
+
+(* The result of inverting a refinement with an exists on the right, which could
+take 0 or more left-hand side steps before the existsR rule. Note that the Taus
+in the quantifier rules are removed in this definition, because this is needed
+in the transitivity proof. *)
+Inductive existsR_LRRefinesF {A : QuantEnc} (k2 : encodes A -> SpecM E2 stk2 R2)
+  : SpecM' E1 stk1 R1 -> Prop :=
+  | existsR_LRRefinesF_existsR t (a : encodes A) :
+    lr_refinesF_u funs1 funs2 RPre RPost RR t (TauF (k2 a)) ->
+    existsR_LRRefinesF k2 t
+  | existsR_LRRefinesF_forallL B k1 (b : encodes B) :
+    existsR_LRRefinesF k2 (observe (k1 b)) ->
+    existsR_LRRefinesF k2 (VisF (Spec_forall B : SpecEvent (FunStackE _ _)) k1)
+  | existsR_LRRefinesF_existsL (B : QuantEnc) k1 :
+    (forall b, existsR_LRRefinesF k2 (observe (k1 b))) ->
+    existsR_LRRefinesF k2 (VisF (Spec_exists B) k1)
+  | existsR_LRRefinesF_TauL t1 :
+    existsR_LRRefinesF k2 (observe t1) ->
+    existsR_LRRefinesF k2 (TauF t1)
+  | existsR_LRRefinesF_unfoldL call1 k1 :
+    existsR_LRRefinesF k2 (observe (applyStackTuple E1 stk1 funs1 call1 >>= k1)) ->
+    existsR_LRRefinesF k2 (VisF (Spec_vis (inl call1)) k1)
+.
+
+(* Helper lemma to invert a Tau in an existsR_LRRefinesF *)
+Lemma existsR_LRRefinesF_TauL_inv A k2 t1 :
+  @existsR_LRRefinesF A k2 (TauF t1) ->
+  @existsR_LRRefinesF A k2 (observe t1).
+Proof.
+  intro H. remember (TauF t1) as tau_t1.
+  revert t1 Heqtau_t1; induction H; intros; try discriminate.
+  - subst t. eapply existsR_LRRefinesF_existsR. red. observe_tau. pstep_reverse.
+    apply lr_refines_TauL_inv. pstep. apply H.
+  - inversion Heqtau_t1. rewrite <- H1. assumption.
+Qed.
+
+(* Invert a refinement of an exists on the right to an existsR_LRRefinesF *)
+Lemma lr_refinesF_existsR_inv A t1 k2 :
+  lr_refinesF_u funs1 funs2 RPre RPost RR
+    t1 (VisF (@Spec_exists (FunStackE E2 stk2) A) k2) ->
+  existsR_LRRefinesF k2 t1.
+Proof.
+  intros. remember (VisF (Spec_exists A) k2) as ot2.
+  induction H; try discriminate.
+  - apply existsR_LRRefinesF_TauL; apply IHlr_refinesF; assumption.
+  - inversion Heqot2. revert k Heqot2 a H IHlr_refinesF H2; rewrite H1; intros.
+    inj_existT. rewrite H2 in H. eapply existsR_LRRefinesF_existsR. apply H.
+  - eapply existsR_LRRefinesF_forallL. apply existsR_LRRefinesF_TauL_inv.
+    apply IHlr_refinesF. assumption.
+  - apply existsR_LRRefinesF_existsL. intros. apply existsR_LRRefinesF_TauL_inv.
+    apply H0. assumption.
+  - apply existsR_LRRefinesF_unfoldL. apply existsR_LRRefinesF_TauL_inv.
+    apply IHlr_refinesF. assumption.
+Qed.
+
+(* Invert a refinement with a corecursive call on the left *)
+Lemma lr_refines_callL_inv pre post call1 k1 t2 :
+  lr_refines funs1 funs2 (liftNilRel pre) (liftNilPostRel post) RR
+    (Vis (Spec_vis (inl call1)) k1) t2 ->
+  lr_refines funs1 funs2 (liftNilRel pre) (liftNilPostRel post) RR
+    (Tau (applyStackTuple E1 stk1 funs1 call1 >>= k1)) t2.
+Proof.
+  intros ref12. punfold ref12. red in ref12. cbn in ref12. pstep. red.
+  remember (observe t2) as ot2; clear t2 Heqot2.
+  remember (VisF (Spec_vis (inl call1)) k1) as ot1.
+  induction ref12; try discriminate.
+  - inversion Heqot1. rewrite H2 in H. destruct e2; destruct H.
+  - apply lr_refinesF_TauR. apply IHref12. assumption.
+  - apply lr_refinesF_forallR; intros. apply H0. assumption.
+  - eapply lr_refinesF_existsR. apply IHref12. assumption.
+  - inversion Heqot1. revert k0 Heqot1 ref12 IHref12. rewrite H0. intros.
+    remember (injection_VisF_eq Heqot1) as e. clear Heqe. inj_existT.
+    rewrite <- e. apply ref12.
+  - apply lr_refinesF_unfoldR. apply IHref12. assumption.
+Qed.
+
+(* Invert a refinement with a corecursive call on the right *)
+Lemma lr_refines_callR_inv pre post t1 call2 k2 :
+  lr_refines funs1 funs2 (liftNilRel pre) (liftNilPostRel post) RR
+    t1 (Vis (Spec_vis (inl call2)) k2) ->
+  lr_refines funs1 funs2 (liftNilRel pre) (liftNilPostRel post) RR
+    t1 (Tau (applyStackTuple E2 stk2 funs2 call2 >>= k2)).
+Proof.
+  intros ref12. punfold ref12. red in ref12. cbn in ref12. pstep. red.
+  remember (observe t1) as ot1; clear t1 Heqot1.
+  remember (VisF (Spec_vis (inl call2)) k2) as ot2.
+  induction ref12; try discriminate.
+  - inversion Heqot2. rewrite H2 in H. destruct e1; destruct H.
+  - apply lr_refinesF_TauL. apply IHref12. assumption.
+  - eapply lr_refinesF_forallL. apply IHref12. assumption.
+  - apply lr_refinesF_existsL; intros. apply H0. assumption.
+  - apply lr_refinesF_unfoldL. apply IHref12. assumption.
+  - inversion Heqot2. revert k0 Heqot2 ref12 IHref12. rewrite H0. intros.
+    remember (injection_VisF_eq Heqot2) as e. clear Heqe. inj_existT.
+    rewrite <- e. apply ref12.
+Qed.
+
+(* The result of inverting a refinement with a Vis on the right, which could
+take 0 or more left-hand side steps before either the Vis rule or the unfoldR
+rule *)
+Inductive visR_LRRefinesF :
+  SpecM' E1 stk1 R1 ->
+  forall (e2: FunStackE E2 stk2), (encodes e2 -> SpecM E2 stk2 R2) -> Prop :=
+  | visR_LRRefinesF_Vis e1 k1 e2 k2 :
+    RPre e1 e2 ->
+    (forall x y, RPost e1 e2 x y ->
+                 lr_refinesF_u funs1 funs2 RPre RPost RR
+                   (observe (k1 x)) (observe (k2 y))) ->
+    visR_LRRefinesF (VisF (Spec_vis e1) k1) e2 k2
+  | visR_LRRefinesF_unfoldR ot1 call2 k2 :
+    lr_refinesF_u funs1 funs2 RPre RPost RR
+      ot1 (observe (applyStackTuple E2 stk2 funs2 call2 >>= k2)) ->
+    visR_LRRefinesF ot1 (inl call2) k2
+  | visR_LRRefinesF_forallL B k1 (b : encodes B) e2 k2 :
+    visR_LRRefinesF (observe (k1 b)) e2 k2 ->
+    visR_LRRefinesF (VisF (Spec_forall B : SpecEvent (FunStackE _ _)) k1) e2 k2
+  | visR_LRRefinesF_existsL (B : QuantEnc) k1 e2 k2 :
+    (forall b, visR_LRRefinesF (observe (k1 b)) e2 k2) ->
+    visR_LRRefinesF (VisF (Spec_exists B) k1) e2 k2
+  | visR_LRRefinesF_TauL t1 e2 k2 :
+    visR_LRRefinesF (observe t1) e2 k2 ->
+    visR_LRRefinesF (TauF t1) e2 k2
+  | visR_LRRefinesF_unfoldL call1 k1 e2 k2 :
+    visR_LRRefinesF (observe (applyStackTuple E1 stk1 funs1 call1 >>= k1)) e2 k2 ->
+    visR_LRRefinesF (VisF (Spec_vis (inl call1)) k1) e2 k2
+.
+
+(* Helper lemma to invert a Tau in a visR_LRRefinesF *)
+Lemma visR_LRRefinesF_TauL_inv t1 e2 k2 :
+  visR_LRRefinesF (TauF t1) e2 k2 ->
+  visR_LRRefinesF (observe t1) e2 k2.
+Proof.
+  intro H. remember (TauF t1) as tau_t1.
+  revert t1 Heqtau_t1; induction H; intros; try discriminate.
+  - subst ot1. apply visR_LRRefinesF_unfoldR.
+    apply lr_refinesF_TauL_inv. assumption.
+  - inversion Heqtau_t1. subst t0. assumption.
+Qed.
+
+(* Invert a refinement of an event on the right to an visR_LRRefinesF *)
+Lemma lr_refinesF_VisR_inv t1 e2 k2 :
+  lr_refinesF_u funs1 funs2 RPre RPost RR t1 (VisF (Spec_vis e2) k2) ->
+  visR_LRRefinesF t1 e2 k2.
+Proof.
+  intros. remember (VisF (Spec_vis e2) k2) as ot2.
+  induction H; try discriminate.
+  - inversion Heqot2. subst e0.
+    set (e := injection_VisF_eq Heqot2); inversion e. inj_existT. subst k0.
+    apply visR_LRRefinesF_Vis; [ assumption | ]. intros.
+    destruct (H0 x y H2) as [ ref | []]. red.
+    pstep_reverse.
+  - apply visR_LRRefinesF_TauL; apply IHlr_refinesF; assumption.
+  - eapply visR_LRRefinesF_forallL. apply visR_LRRefinesF_TauL_inv.
+    apply IHlr_refinesF. assumption.
+  - apply visR_LRRefinesF_existsL. intros. apply visR_LRRefinesF_TauL_inv.
+    apply H0. assumption.
+  - apply visR_LRRefinesF_unfoldL. apply visR_LRRefinesF_TauL_inv.
+    apply IHlr_refinesF. assumption.
+  - inversion Heqot2. subst e2.
+    set (e := injection_VisF_eq Heqot2); inversion e. inj_existT. subst k0.
+    apply visR_LRRefinesF_unfoldR. rewrite (entree_beta ot1).
+    apply lr_refinesF_TauR_inv. apply H.
+Qed.
+
+(* The result of inverting a refinement with a Vis on the left, which could take
+0 or more right-hand side steps before either the Vis rule or the unfoldL rule
+*)
+Inductive visL_LRRefinesF :
+  forall (e1: FunStackE E1 stk1), (encodes e1 -> SpecM E1 stk1 R1) ->
+  SpecM' E2 stk2 R2 -> Prop :=
+  | visL_LRRefinesF_Vis e1 k1 e2 k2 :
+    RPre e1 e2 ->
+    (forall x y, RPost e1 e2 x y ->
+                 lr_refinesF_u funs1 funs2 RPre RPost RR
+                   (observe (k1 x)) (observe (k2 y))) ->
+    visL_LRRefinesF e1 k1 (VisF (Spec_vis e2) k2)
+  | visL_LRRefinesF_unfoldL call1 k1 ot2 :
+    lr_refinesF_u funs1 funs2 RPre RPost RR
+      (observe (applyStackTuple E1 stk1 funs1 call1 >>= k1)) ot2 ->
+    visL_LRRefinesF (inl call1) k1 ot2
+  | visL_LRRefinesF_forallR e1 k1 (B : QuantEnc) k2 :
+    (forall b, visL_LRRefinesF e1 k1 (observe (k2 b))) ->
+    visL_LRRefinesF e1 k1 (VisF (Spec_forall B) k2)
+  | visL_LRRefinesF_existsR e1 k1 B (b : encodes B) k2 :
+    visL_LRRefinesF e1 k1 (observe (k2 b)) ->
+    visL_LRRefinesF e1 k1 (VisF (Spec_exists B : SpecEvent (FunStackE _ _)) k2)
+  | visL_LRRefinesF_TauR e1 k1 t2 :
+    visL_LRRefinesF e1 k1 (observe t2) ->
+    visL_LRRefinesF e1 k1 (TauF t2)
+  | visL_LRRefinesF_unfoldR e1 k1 call2 k2 :
+    visL_LRRefinesF e1 k1 (observe (applyStackTuple E2 stk2 funs2 call2 >>= k2)) ->
+    visL_LRRefinesF e1 k1 (VisF (Spec_vis (inl call2)) k2)
+.
+
+(* Helper lemma to invert a Tau in a visL_LRRefinesF *)
+Lemma visL_LRRefinesF_TauR_inv e1 k1 t2 :
+  visL_LRRefinesF e1 k1 (TauF t2) ->
+  visL_LRRefinesF e1 k1 (observe t2).
+Proof.
+  intro H. remember (TauF t2) as tau_t2.
+  revert t2 Heqtau_t2; induction H; intros; try discriminate.
+  - subst ot2. apply visL_LRRefinesF_unfoldL.
+    apply lr_refinesF_TauR_inv. assumption.
+  - inversion Heqtau_t2. subst t0. assumption.
+Qed.
+
+(* Invert a refinement of an event on the right to an visL_LRRefinesF *)
+Lemma lr_refinesF_VisL_inv e1 k1 t2 :
+  lr_refinesF_u funs1 funs2 RPre RPost RR (VisF (Spec_vis e1) k1) t2 ->
+  visL_LRRefinesF e1 k1 t2.
+Proof.
+  intros. remember (VisF (Spec_vis e1) k1) as ot1.
+  induction H; try discriminate.
+  - inversion Heqot1. subst e0.
+    set (e := injection_VisF_eq Heqot1); inversion e. inj_existT. subst k0.
+    apply visL_LRRefinesF_Vis; [ assumption | ]. intros.
+    destruct (H0 x y H2) as [ ref | []].
+    red. pstep_reverse.
+  - apply visL_LRRefinesF_TauR; apply IHlr_refinesF; assumption.
+  - apply visL_LRRefinesF_forallR. intros. apply visL_LRRefinesF_TauR_inv.
+    apply H0. assumption.
+  - eapply visL_LRRefinesF_existsR. apply visL_LRRefinesF_TauR_inv.
+    apply IHlr_refinesF. assumption.
+  - inversion Heqot1. subst e1.
+    set (e := injection_VisF_eq Heqot1); inversion e. inj_existT. subst k0.
+    apply visL_LRRefinesF_unfoldL. rewrite (entree_beta ot2).
+    apply lr_refinesF_TauL_inv. apply H.
+  - apply visL_LRRefinesF_unfoldR. apply visL_LRRefinesF_TauR_inv.
+    apply IHlr_refinesF. assumption.
+Qed.
+
+
+End lr_refines_inv.
+
+
+(*** Refinement respects entree equivalence ***)
+Section lr_refines_proper.
+
+Context {E1 E2 : EvType} {stk1 stk2 : FunStack} {R1 R2 : Type}.
+Context (funs1 : StackTuple E1 stk1 stk1) (funs2 : StackTuple E2 stk2 stk2).
+
+Context (RPre : Rel (FunStackE E1 stk1) (FunStackE E2 stk2))
+  (RPost : PostRel (FunStackE E1 stk1) (FunStackE E2 stk2))
+  (RR : Rel R1 R2).
+
+
+(* lr_refines is Proper wrt eutt on the right *)
+Lemma lr_refines_euttR t1 t2 t2' :
+  lr_refines funs1 funs2 RPre RPost RR t1 t2 -> eutt eq t2 t2' ->
+  lr_refines funs1 funs2 RPre RPost RR t1 t2'.
+Proof.
+  revert t1 t2 t2'; pcofix CIH; intros t1 t2 t2' ref12 e.
+  destruct t1 as [ ot1 ]. destruct t2 as [ ot2 ].
+  punfold ref12. red in ref12. simpl in ref12.
+  revert t2' e; induction ref12; intros.
+  - destruct t2' as [ ot2' ]; punfold e; red in e. simpl in e.
+    remember (RetF r2) as ret_r2. induction e; inversion Heqret_r2.
+    + rewrite <- REL; rewrite H1. pstep. apply lr_refinesF_Ret; assumption.
+    + pstep. apply lr_refinesF_TauR. pstep_reverse. rewrite <- entree_eta in IHe.
+      apply IHe. assumption.
+  - pclearbot.
+    assert (eutt eq t2 t2'); [ apply eqit_inv_Tau_l; assumption | ]. clear e.
+    punfold H0. red in H0. punfold H. red in H.
+    destruct t2 as [ ot2 ]. destruct t2' as [ ot2' ].
+    simpl in H. simpl in H0. pstep. red. simpl. revert t1 H; induction H0; intros.
+    + apply lr_refinesF_TauL. simpl.
+      remember (observe t1) as ot1; clear t1 Heqot1.
+      remember (RetF r1) as ret_r1.
+      induction H; inversion Heqret_r1.
+      * apply lr_refinesF_Ret. rewrite <- REL. rewrite <- H1. assumption.
+      * apply lr_refinesF_TauL. apply IHlr_refinesF. assumption.
+      * eapply lr_refinesF_forallL. apply IHlr_refinesF. assumption.
+      * apply lr_refinesF_existsL; intros. apply H0. assumption.
+      * apply lr_refinesF_unfoldL. apply IHlr_refinesF. assumption.
+    + apply lr_refinesF_Tau. right. pclearbot. eapply CIH; [ | eassumption ].
+      apply lr_refines_TauR_inv. pstep. assumption.
+    + destruct e.
+      * remember (lr_refinesF_VisR_inv _ _ _ _ _ _ _ _ H) as visRef.
+        clear H HeqvisRef.
+        destruct t1 as [ ot1 ]; simpl in visRef.
+        induction visRef.
+        -- apply lr_refinesF_TauL.
+           apply lr_refinesF_Vis; [ assumption | ]. intros.
+           right. pclearbot. eapply CIH; [ | apply REL ].
+           pstep; apply H0; assumption.
+        -- apply lr_refinesF_unfoldR. apply lr_refinesF_Tau. right.
+           pclearbot. eapply CIH; [ pstep; apply H | ].
+           eapply (eqit_bind _ (UU:=eq));
+             [ | intros u1 u2 eq_u; rewrite eq_u; apply REL ].
+           reflexivity.
+        -- apply lr_refinesF_TauL.
+           eapply (lr_refinesF_forallL _ _ _ _ _ _ _ _ _ b).
+           rewrite (entree_eta (k1 b)). apply IHvisRef. intros. apply REL.
+        -- apply lr_refinesF_TauL. apply lr_refinesF_existsL; intros.
+           rewrite (entree_eta (k1 a)). apply H0. intros. apply REL.
+        -- apply lr_refinesF_TauL. rewrite (entree_eta t1).
+           apply IHvisRef. intros; apply REL.
+        -- apply lr_refinesF_TauL. rewrite <- entree_eta in IHvisRef.
+           apply lr_refinesF_unfoldL. apply IHvisRef. intros; apply REL.
+      * apply lr_refinesF_forallR. intros. apply lr_refinesF_Tau.
+        right. eapply CIH.
+        -- apply lr_refines_forallR_inv. pstep. apply H.
+        -- pstep. apply EqTauL; [ reflexivity | ].
+           destruct (REL a) as [ e | []]. pstep_reverse.
+      * assert (existsR_LRRefinesF funs1 funs2 RPre RPost RR k1 (observe t1))
+        as ref_exR;
+        [ apply lr_refinesF_existsR_inv; apply H | ]. clear H.
+        destruct t1 as [ ot1 ]. simpl in ref_exR. induction ref_exR.
+        -- eapply lr_refinesF_existsR. apply lr_refinesF_Tau. right.
+           pclearbot. eapply CIH; [ | apply REL ].
+           apply lr_refines_TauR_inv. pstep. apply H.
+        -- apply lr_refinesF_TauL. eapply lr_refinesF_forallL.
+           rewrite <- entree_eta in IHref_exR. apply IHref_exR.
+        -- apply lr_refinesF_TauL. apply lr_refinesF_existsL. intros.
+           rewrite (entree_eta (k0 a)). apply H0.
+        -- apply lr_refinesF_TauL. rewrite <- entree_eta in IHref_exR.
+           apply IHref_exR.
+        -- apply lr_refinesF_TauL. apply lr_refinesF_unfoldL.
+           rewrite <- entree_eta in IHref_exR. apply IHref_exR.
+    + apply IHeqitF. apply lr_refinesF_TauR_inv. assumption.
+    + apply lr_refinesF_Tau. right. rewrite (entree_beta ot1) in H.
+      eapply CIH; pstep; [ eassumption | apply H0 ].
+  - punfold e; red in e. pstep; red.
+    remember (observe t2') as ot2'; clear t2' Heqot2'.
+    remember (observe (Vis (Spec_vis e2) k2)) as ot1.
+    induction e; inversion Heqot1.
+    + subst e. inj_existT. subst k0. apply lr_refinesF_Vis; [ assumption | ].
+      intros. destruct (H0 a b H1); [ | destruct H2 ].
+      destruct (REL b); [ | destruct H3 ].
+      right. eapply CIH; eassumption.
+    + apply lr_refinesF_TauR. apply IHe. assumption.
+  - pstep. apply lr_refinesF_TauL. pstep_reverse.
+    rewrite <- entree_eta in IHref12. apply IHref12. assumption.
+  - apply IHref12. apply eqit_inv_Tau_l. rewrite <- entree_eta. assumption.
+  - punfold e; red in e. pstep; red. simpl.
+    remember (observe t2') as ot2'; clear t2' Heqot2'.
+    remember (observe (Vis (Spec_forall A) k)) as ot2.
+    induction e; inversion Heqot2.
+    + subst e. inj_existT. subst k1. apply lr_refinesF_forallR. intros.
+      observe_tau. rewrite (entree_beta ot1). pstep_reverse. eapply H0.
+      pstep. constructor. left. destruct (REL a); [ eassumption | destruct H1 ].
+    + apply lr_refinesF_TauR. apply IHe. assumption.
+  - punfold e; red in e. pstep; red. simpl.
+    remember (observe t2') as ot2'; clear t2' Heqot2'.
+    remember (observe (Vis (Spec_exists A) k)) as ot2.
+    induction e; inversion Heqot2.
+    + subst e. inj_existT. subst k1. eapply lr_refinesF_existsR.
+      observe_tau. rewrite (entree_beta ot1). pstep_reverse. apply IHref12.
+      pstep. constructor. left. destruct (REL a); [ eassumption | destruct H ].
+    + apply lr_refinesF_TauR. apply IHe. assumption.
+  - pstep. eapply lr_refinesF_forallL. observe_tau. pstep_reverse.
+  - pstep. apply lr_refinesF_existsL; intros. observe_tau. pstep_reverse.
+  - pstep. apply lr_refinesF_unfoldL. observe_tau. pstep_reverse.
+  - punfold e; red in e. pstep; red. simpl.
+    remember (observe t2') as ot2'; clear t2' Heqot2'. simpl in e.
+    remember (VisF (Spec_vis (inl call2)) k2) as ot2.
+    induction e; inversion Heqot2.
+    + subst e. inj_existT. subst k1. apply lr_refinesF_unfoldR.
+      observe_tau. rewrite (entree_beta ot1). pstep_reverse. apply IHref12.
+      pstep. constructor. left. eapply eqit_bind; [ reflexivity | ]. intros.
+      rewrite H. destruct (REL u2); [ | destruct H0 ]. assumption.
+    + apply lr_refinesF_TauR. apply IHe. assumption.
+Qed.
+
+
+(* lr_refines is Proper wrt eutt on the left *)
+Lemma lr_refines_euttL t1 t1' t2 :
+  eutt eq t1' t1 -> lr_refines funs1 funs2 RPre RPost RR t1 t2 ->
+  lr_refines funs1 funs2 RPre RPost RR t1' t2.
+Proof.
+  revert t1 t1' t2; pcofix CIH; intros t1 t1' t2 e ref12.
+  destruct t1 as [ ot1 ]. destruct t2 as [ ot2 ].
+  punfold ref12. red in ref12. simpl in ref12.
+  revert t1' e; induction ref12; intros.
+  - destruct t1' as [ ot1' ]; punfold e; red in e. simpl in e.
+    remember (RetF r1) as ret_r1. induction e; inversion Heqret_r1.
+    + subst r3; subst r0. pstep. apply lr_refinesF_Ret; assumption.
+    + pstep. apply lr_refinesF_TauL. pstep_reverse. rewrite <- entree_eta in IHe.
+      apply IHe. assumption.
+  - pclearbot.
+    assert (eutt eq t1' t1); [ apply eqit_inv_Tau_r; assumption | ]. clear e.
+    punfold H0. red in H0. punfold H. red in H.
+    destruct t1 as [ ot1 ]. destruct t1' as [ ot1' ].
+    simpl in H. simpl in H0. pstep. red. simpl. revert t2 H; induction H0; intros.
+    + apply lr_refinesF_TauR. simpl.
+      remember (observe t2) as ot2; clear t2 Heqot2.
+      remember (RetF r2) as ret_r2.
+      induction H; inversion Heqret_r2.
+      * apply lr_refinesF_Ret. rewrite REL. rewrite <- H1. assumption.
+      * apply lr_refinesF_TauR. apply IHlr_refinesF. assumption.
+      * apply lr_refinesF_forallR; intros. apply H0. assumption.
+      * eapply lr_refinesF_existsR. apply IHlr_refinesF. assumption.
+      * apply lr_refinesF_unfoldR. apply IHlr_refinesF. assumption.
+    + apply lr_refinesF_Tau. right. pclearbot. eapply CIH; [ eassumption | ].
+      apply lr_refines_TauL_inv. pstep. assumption.
+    + destruct e.
+      * remember (lr_refinesF_VisL_inv _ _ _ _ _ _ _ _ H) as visRef.
+        clear H HeqvisRef.
+        destruct t2 as [ ot2 ]; simpl in visRef.
+        induction visRef.
+        -- apply lr_refinesF_TauR.
+           apply lr_refinesF_Vis; [ assumption | ]. intros.
+           right. pclearbot. eapply CIH; [ apply REL | ].
+           pstep; apply H0; assumption.
+        -- apply lr_refinesF_unfoldL. apply lr_refinesF_Tau. right.
+           pclearbot. eapply CIH; [ | pstep; apply H ].
+           eapply (eqit_bind _ (UU:=eq));
+             [ | intros u1 u2 eq_u; rewrite eq_u; apply REL ].
+           reflexivity.
+        -- apply lr_refinesF_TauR. apply lr_refinesF_forallR; intros.
+           rewrite (entree_eta (k2 a)). apply H0. intros. apply REL.
+        -- apply lr_refinesF_TauR.
+           apply (lr_refinesF_existsR _ _ _ _ _ _ _ _ _ b).
+           rewrite (entree_eta (k2 b)). apply IHvisRef. intros. apply REL.
+        -- apply lr_refinesF_TauR. rewrite (entree_eta t2).
+           apply IHvisRef. intros; apply REL.
+        -- apply lr_refinesF_TauR. rewrite <- entree_eta in IHvisRef.
+           apply lr_refinesF_unfoldR. apply IHvisRef. intros; apply REL.
+      * assert (forallL_LRRefinesF funs1 funs2 RPre RPost RR k2 (observe t2))
+          as ref_allL;
+          [ apply lr_refinesF_forallL_inv; apply H | ]. clear H.
+        destruct t2 as [ ot2 ]. simpl in ref_allL. induction ref_allL.
+        -- eapply lr_refinesF_forallL. apply lr_refinesF_Tau. right.
+           pclearbot. eapply CIH; [ apply REL | ].
+           apply lr_refines_TauL_inv. pstep. apply H.
+        -- apply lr_refinesF_TauR. apply lr_refinesF_forallR. intros.
+           rewrite (entree_eta (k0 a)). apply H0.
+        -- apply lr_refinesF_TauR. eapply lr_refinesF_existsR.
+           rewrite <- entree_eta in IHref_allL. apply IHref_allL.
+        -- apply lr_refinesF_TauR. rewrite <- entree_eta in IHref_allL.
+           apply IHref_allL.
+        -- apply lr_refinesF_TauR. apply lr_refinesF_unfoldR.
+           rewrite <- entree_eta in IHref_allL. apply IHref_allL.
+      * apply lr_refinesF_existsL. intros. apply lr_refinesF_Tau.
+        right. eapply CIH; [ | apply lr_refines_existsL_inv; pstep; apply H ].
+        destruct (REL a) as [ e | []]. pstep. apply EqTauR; [ reflexivity | ].
+        pstep_reverse.
+    + apply lr_refinesF_Tau. right. rewrite (entree_beta ot2) in H0.
+      eapply CIH; pstep; [ apply H0 | eassumption ].
+    + apply IHeqitF. apply lr_refinesF_TauL_inv. assumption.
+  - punfold e; red in e. pstep; red.
+    remember (observe t1') as ot1'; clear t1' Heqot1'.
+    remember (observe (Vis (Spec_vis e1) k1)) as ot1.
+    induction e; inversion Heqot1.
+    + subst e. inj_existT. subst k3. apply lr_refinesF_Vis; [ assumption | ].
+      intros. destruct (H0 a b H1); [ | destruct H2 ].
+      destruct (REL a); [ | destruct H3 ].
+      right. eapply CIH; eassumption.
+    + apply lr_refinesF_TauL. apply IHe. assumption.
+  - apply IHref12. apply eqit_inv_Tau_r. rewrite <- entree_eta. assumption.
+  - pstep. apply lr_refinesF_TauR. pstep_reverse.
+    rewrite <- entree_eta in IHref12. apply IHref12. assumption.
+  - pstep. apply lr_refinesF_forallR; intros. observe_tau. pstep_reverse.
+  - pstep. eapply lr_refinesF_existsR. observe_tau. pstep_reverse.
+  - punfold e; red in e. pstep; red. simpl.
+    remember (observe t1') as ot1'; clear t1' Heqot1'.
+    remember (observe (Vis (Spec_forall A) k)) as ot1.
+    induction e; inversion Heqot1.
+    + subst e. inj_existT. subst k2. eapply lr_refinesF_forallL.
+      observe_tau. rewrite (entree_beta ot2). pstep_reverse. apply IHref12.
+      pstep. constructor. left. destruct (REL a); [ eassumption | destruct H ].
+    + apply lr_refinesF_TauL. apply IHe. assumption.
+  - punfold e; red in e. pstep; red. simpl.
+    remember (observe t1') as ot1'; clear t1' Heqot1'.
+    remember (observe (Vis (Spec_exists A) k)) as ot1.
+    induction e; inversion Heqot1.
+    + subst e. inj_existT. subst k2. apply lr_refinesF_existsL. intros.
+      observe_tau. rewrite (entree_beta ot2). pstep_reverse. eapply H0.
+      pstep. constructor. left. destruct (REL a); [ eassumption | destruct H1 ].
+    + apply lr_refinesF_TauL. apply IHe. assumption.
+  - punfold e; red in e. pstep; red. simpl.
+    remember (observe t1') as ot1'; clear t1' Heqot1'. simpl in e.
+    remember (VisF (Spec_vis (inl call1)) k1) as ot1.
+    induction e; inversion Heqot1.
+    + subst e. inj_existT. subst k2. apply lr_refinesF_unfoldL.
+      observe_tau. rewrite (entree_beta ot2). pstep_reverse. apply IHref12.
+      pstep. constructor. left. eapply eqit_bind; [ reflexivity | ]. intros.
+      rewrite H. destruct (REL u2); [ | destruct H0 ]. assumption.
+    + apply lr_refinesF_TauL. apply IHe. assumption.
+  - pstep. apply lr_refinesF_unfoldR. observe_tau. pstep_reverse.
+Qed.
+
+End lr_refines_proper.
+
+
+(* Refinement is proper wrt eutt *)
+Global Instance Proper_eutt_lr_refines {E1 E2 : EvType} {stk1 stk2} {R1 R2}
+  funs1 funs2 RPre RPost RR :
+  Proper (eutt eq ==> eutt eq ==> flip impl)
+    (@lr_refines E1 E2 stk1 stk2 R1 R2 funs1 funs2 RPre RPost RR).
+Proof.
+  repeat intro. eapply lr_refines_euttL; [ eassumption | ].
+  eapply lr_refines_euttR; [ | symmetry ]; eassumption.
+Qed.
+
+
+(*** Reflexivity and Transitivity of refinemenet ***)
+
+(* Reflexivity *)
+Lemma lr_refines_refl {E stk R funs1 funs2}
+  (RPre : Rel (FunStackE E stk) (FunStackE E stk))
+  (RPost : PostRel (FunStackE E stk) (FunStackE E stk))
+  (RR : Rel R R) :
+  Reflexive RPre -> ReflexivePostRel RPost -> Reflexive RR ->
+  forall t, lr_refines funs1 funs2 RPre RPost RR t t.
+Proof.
+  intros HRPre HRPost HRR. pcofix CIH. intros t. pstep. red.
+  destruct t as [ ot ]. destruct ot.
+  - apply lr_refinesF_Ret. auto.
+  - apply lr_refinesF_Tau. right. pclearbot. eauto.
+  - destruct e.
+    + apply lr_refinesF_Vis; [ eauto | ]. intros.
+      rewrite (HRPost e a b); [ | assumption ]. right. apply CIH.
+    + apply lr_refinesF_forallR. intros. eapply lr_refinesF_forallL.
+      apply lr_refinesF_Tau. right. apply CIH.
+    + apply lr_refinesF_existsL. intros. eapply lr_refinesF_existsR.
+      apply lr_refinesF_Tau. right. apply CIH.
+Qed.
+
+(* Transitivity *)
+Lemma lr_refines_trans {E1 E2 E3} {stk1 stk2 stk3} {R1 R2 R3}
+  RPre1 RPre2 RPost1 RPost2
+  (RR1 : R1 -> R2 -> Prop) (RR2 : R2 -> R3 -> Prop)
+  (funs1 : StackTuple E1 stk1 stk1) (funs2 : StackTuple E2 stk2 stk2)
+  (funs3 : StackTuple E3 stk3 stk3)
+  (t1 : SpecM E1 stk1 R1) (t2 : SpecM E2 stk2 R2) (t3 : SpecM E3 stk3 R3) :
+  lr_refines funs1 funs2 (liftNilRel RPre1) (liftNilPostRel RPost1) RR1 t1 t2 ->
+  lr_refines funs2 funs3 (liftNilRel RPre2) (liftNilPostRel RPost2) RR2 t2 t3 ->
+  lr_refines funs1 funs3 (liftNilRel (rcompose RPre1 RPre2))
+    (liftNilPostRel (RComposePostRel RPre1 RPre2 RPost1 RPost2))
+    (rcompose RR1 RR2) t1 t3.
+Proof.
+  revert t1 t2 t3; pcofix CIH; intros t1 t2 t3 ref12 ref23.
+  pfold. red. punfold ref12. red in ref12. punfold ref23. red in ref23.
+  remember (observe t1) as ot1. clear t1 Heqot1.
+  remember (observe t2) as ot2. clear t2 Heqot2.
+  revert t3 ref23; induction ref12; intros.
+  - remember (RetF r2) as x. induction ref23; inversion Heqx.
+    + constructor. exists r2; split; [ assumption | ].
+      rewrite <- H2. assumption.
+    + constructor. apply IHref23. assumption.
+    + constructor. intros. apply H1. assumption.
+    + econstructor. apply IHref23. assumption.
+    + constructor. apply IHref23. assumption.
+  - pclearbot.
+    assert (lr_refines funs2 funs3 (liftNilRel RPre2) (liftNilPostRel RPost2) RR2 t2 t3) as ref23'.
+    { apply lr_refines_TauL_inv. pstep. assumption. }
+    clear ref23. punfold ref23'. red in ref23'.
+    remember (observe t3) as ot3; clear t3 Heqot3.
+    punfold H. red in H.
+    remember (observe t2) as ot2. clear t2 Heqot2.
+    revert t1 H. induction ref23'; intros.
+    + apply lr_refinesF_TauL.
+      (* Proof that  t1 |= Ret r1 |= Ret r2  implies Tau t1 |= Ret r2 *)
+      remember (observe t1) as ot1; clear t1 Heqot1.
+      remember (RetF r1) as ot0. induction H0; try discriminate Heqot0.
+      * inversion Heqot0. apply lr_refinesF_Ret. rewrite H2 in H0.
+        eexists; split; eassumption.
+      * apply lr_refinesF_TauL. apply IHlr_refinesF. assumption.
+      * eapply lr_refinesF_forallL. apply IHlr_refinesF. assumption.
+      * apply lr_refinesF_existsL. intros. apply H1. assumption.
+      * apply lr_refinesF_unfoldL. apply IHlr_refinesF. assumption.
+    + apply lr_refinesF_Tau. right. pclearbot. eapply CIH; [ | eassumption ].
+      apply lr_refines_TauR_inv. pstep. apply H0.
+    + apply lr_refinesF_TauL.
+      (* Proof that  t1 |= Vis e2 k2 |= Vis e3 k3  implies t1 |= Vis e3 k3 *)
+      remember (observe t1) as ot1; clear t1 Heqot1.
+      remember (VisF (Spec_vis e1) k1) as ot0.
+      induction H1; try discriminate Heqot0.
+      * set (e := injection_VisF_eq Heqot0). inversion e.
+        revert k3 Heqot0 H1 H2 e; rewrite H4; intros. clear e3 H4. inj_existT.
+        apply lr_refinesF_Vis; [ eapply liftNilRel_compose; eassumption | ].
+        intros.
+        destruct (liftNilPostRel_compose_elim H1 H H3)
+          as [ c [ PR_ac PR_cb ]].
+        remember (H2 a c PR_ac) as ref_k0_k3. clear Heqref_k0_k3.
+        rewrite <- e in H0.
+        remember (H0 c b PR_cb) as ref_k3_k2. clear Heqref_k3_k2.
+        pclearbot.
+        right. eapply CIH; eassumption.
+      * apply lr_refinesF_TauL. apply IHlr_refinesF. assumption.
+      * eapply lr_refinesF_forallL. apply IHlr_refinesF. assumption.
+      * eapply lr_refinesF_existsL. intros. apply H2. assumption.
+      * apply lr_refinesF_unfoldL. apply IHlr_refinesF. assumption.
+      * inversion Heqot0. rewrite <- H3 in H. destruct e2; simpl in H; contradiction.
+    + apply IHref23'. pstep_reverse. apply lr_refines_TauR_inv.
+      pstep. apply H.
+    + apply lr_refinesF_Tau. right.
+      apply (CIH _ (go _ _ ot1)); pstep; assumption.
+    + apply lr_refinesF_forallR. intros. apply H0. assumption.
+    + eapply lr_refinesF_existsR. apply IHref23'. assumption.
+    + apply IHref23'. observe_tau. pstep_reverse.
+      apply lr_refines_forallR_inv. pstep. apply H.
+    + assert (existsR_LRRefinesF funs1 funs2
+                (liftNilRel RPre1) (liftNilPostRel RPost1) RR1
+                k (observe t1))
+        as ref_exR;
+        [ apply lr_refinesF_existsR_inv; assumption | ].
+      clear H1.
+      destruct t1 as [ ot1 ]. simpl in ref_exR.
+      induction ref_exR.
+      * apply (H0 a). assumption.
+      * apply lr_refinesF_TauL. eapply lr_refinesF_forallL.
+        rewrite <- (entree_eta (k1 b)) in IHref_exR. apply IHref_exR.
+      * apply lr_refinesF_TauL. eapply lr_refinesF_existsL. intros.
+        rewrite (entree_eta (k1 a)). apply H2.
+      * apply lr_refinesF_TauL. simpl. rewrite (entree_eta t1).
+        apply IHref_exR.
+      * apply lr_refinesF_TauL. apply lr_refinesF_unfoldL.
+        rewrite <- entree_eta in IHref_exR. apply IHref_exR.
+    + apply IHref23'. observe_tau. pstep_reverse.
+      apply lr_refines_callR_inv. pstep. assumption.
+    + apply lr_refinesF_unfoldR. apply IHref23'. assumption.
+  - (* Vis e1 k1 |= Vis e2 k2 |= t3  implies Vis e1 k1 |= t3 *)
+    remember (observe t3) as ot3; clear t3 Heqot3.
+    remember (VisF (Spec_vis e2) k2) as ot2.
+    induction ref23; try discriminate Heqot2.
+    + inversion Heqot2. revert k0 Heqot2 H1 H2; rewrite H4; intros.
+      remember (injection_VisF_eq Heqot2) as e. clear Heqe. inj_existT.
+      subst k0. apply lr_refinesF_Vis.
+      * eapply liftNilRel_compose; eassumption.
+      * intros. destruct (liftNilPostRel_compose_elim H H1 H3) as [ c [ Rac Rcb ] ].
+        remember (H0 a c Rac) as ref_k1_k2; clear Heqref_k1_k2.
+        remember (H2 c b Rcb) as ref_k2_k3; clear Heqref_k2_k3.
+        pclearbot.
+        right. eapply CIH; eassumption.
+    + apply lr_refinesF_TauR. apply IHref23. assumption.
+    + apply lr_refinesF_forallR; intros. apply H2. assumption.
+    + eapply lr_refinesF_existsR. apply IHref23. assumption.
+    + inversion Heqot2. rewrite <- H2 in H.
+      destruct e1; destruct H.
+    + apply lr_refinesF_unfoldR. apply IHref23. assumption.
+  - apply lr_refinesF_TauL. apply IHref12. assumption.
+  - apply IHref12. pstep_reverse. apply lr_refines_TauL_inv. pstep. assumption.
+  - assert (forallL_LRRefinesF funs2 funs3
+              (liftNilRel RPre2) (liftNilPostRel RPost2) RR2 k (observe t3))
+      as ref_allL;
+      [ apply lr_refinesF_forallL_inv; assumption | ].
+    clear ref23. remember (observe t3) as ot3; clear t3 Heqot3.
+    induction ref_allL.
+    + apply (H0 a (go _ _ t)). apply H1.
+    + apply lr_refinesF_forallR; intros. apply lr_refinesF_TauR. apply H2.
+    + eapply lr_refinesF_existsR. apply lr_refinesF_TauR. apply IHref_allL.
+    + apply lr_refinesF_TauR. apply IHref_allL.
+    + apply lr_refinesF_unfoldR. apply lr_refinesF_TauR. apply IHref_allL.
+  - apply IHref12. observe_tau.
+    pstep_reverse. apply lr_refines_existsL_inv. pstep. apply ref23.
+  - eapply lr_refinesF_forallL. apply IHref12. assumption.
+  - apply lr_refinesF_existsL. intros. apply H0. assumption.
+  - apply lr_refinesF_unfoldL. apply IHref12. assumption.
+  - apply IHref12. observe_tau. pstep_reverse.
+    apply lr_refines_callL_inv. pstep. assumption.
+Qed.
+
+
+(*** Laws about refinement of bind ***)
+Section lr_refines_bind.
+Context {E1 E2 : EvType} {stk1 stk2 : FunStack} {R1 R2 : Type} {RR : Rel R1 R2}.
+Context {funs1 : StackTuple E1 stk1 stk1} {funs2 : StackTuple E2 stk2 stk2}.
+
+(* Helper lemma to apply entree_beta to the lhs of a bind *)
+Lemma observing_BindS E stk A B m (k : A -> SpecM E stk B) :
+  BindS m k = BindS (go _ _ (observe m)) k.
+Proof.
+  reflexivity.
+Qed.
+
+Lemma BindS_Ret_l_eq {E stk R S} (r : R) (k : R -> SpecM E stk S) :
+  Ret r >>= k = k r.
+Proof.
+  rewrite (entree_eta (Ret r >>= k)). rewrite (entree_eta (k r)).
+  reflexivity.
+Qed.
+
+Lemma BindS_Tau_eq {E stk R S} (m : SpecM E stk R) (k : R -> SpecM E stk S) :
+  Tau m >>= k = Tau (m >>= k).
+Proof.
+  rewrite (entree_eta (Tau m >>= k)). rewrite (entree_eta (Tau (m >>= k))).
+  reflexivity.
+Qed.
+
+
+Lemma eq_itree_TauR_inv {E stk R} (t1 t2 : SpecM E stk R) :
+  eq_itree eq t1 (Tau t2) ->
+  exists t1', t1 = Tau t1' /\ eq_itree eq t1' t2.
+Proof.
+  intro e. punfold e. inversion e; try discriminate.
+  exists m1. rewrite (entree_eta t1). rewrite <- H0. pclearbot.
+  split; [ reflexivity | assumption ].
+Qed.
+
+Lemma BindS_Vis_eq {E:EvType} {stk R S} (e : SpecEvent (FunStackE E stk))
+  (k1 : encodes e -> SpecM E stk R) (k2 : R -> SpecM E stk S) :
+  Vis e k1 >>= k2 = Vis e (fun x => k1 x >>= k2).
+Proof.
+  rewrite (entree_eta (Vis e k1 >>= k2)).
+  rewrite (entree_eta (Vis e (fun x => k1 x >>= k2))).
+  reflexivity.
+Qed.
+
+Lemma eq_itree_VisR_inv {E stk R} (t : SpecM E stk R) e k :
+  eq_itree eq t (Vis e k) ->
+  exists k', t = Vis e k' /\ (forall x, eq_itree eq (k' x) (k x)).
+Proof.
+  intro H. punfold H.
+  destruct t as [ ot ]; destruct ot;
+    [ inversion H | inversion H; discriminate | ].
+  assert (e0 = e); [ inversion H; reflexivity | ]. subst e0.
+  exists k0; split; [ reflexivity | ].
+  apply eqit_Vis_inv. pstep. assumption.
+Qed.
+
+
+(* Refinement commutes with bind *)
+Lemma lr_refines_bind {RPre RPost S1 S2} {RS : Rel S1 S2} m1 m2 k1 k2 :
+  lr_refines funs1 funs2 RPre RPost RS m1 m2 ->
+  (forall x1 x2, RS x1 x2 ->
+                 lr_refines funs1 funs2 RPre RPost RR (k1 x1) (k2 x2)) ->
+  lr_refines funs1 funs2 RPre RPost RR (m1 >>= k1) (m2 >>= k2).
+Proof.
+  intros mref kref; revert m1 m2 mref.
+  assert (forall t1 t2 m1 m2,
+             eq_itree eq t1 (m1 >>= k1) -> eq_itree eq t2 (m2 >>= k2) ->
+             lr_refines funs1 funs2 RPre RPost RS m1 m2 ->
+             lr_refines funs1 funs2 RPre RPost RR t1 t2) as H;
+    [ | intros; apply (H (m1 >>= k1) (m2 >>= k2) m1 m2);
+        try reflexivity; assumption ].
+  pcofix CIH; intros t1 t2 m1 m2 e1 e2 mref.
+  punfold mref; red in mref.
+  rewrite observing_BindS in e1. rewrite observing_BindS in e2.
+  remember (observe m1) as om1. remember (observe m2) as om2.
+  clear m1 m2 Heqom1 Heqom2.
+  revert t1 t2 e1 e2; induction mref; intros; pclearbot.
+  - rewrite BindS_Ret_l_eq in e1. rewrite BindS_Ret_l_eq in e2.
+    eapply paco2_mon.
+    + eapply lr_refines_euttL; [ apply eq_sub_eutt; apply e1 | ].
+      eapply lr_refines_euttR; [ | apply eq_sub_eutt; symmetry; apply e2 ].
+      apply kref; assumption.
+    + intros. destruct PR.
+  - pstep. rewrite BindS_Tau_eq in e1. rewrite BindS_Tau_eq in e2.
+    destruct (eq_itree_TauR_inv _ _ e1) as [ t0' [ e_t0 e_t0' ]]; subst t0.
+    destruct (eq_itree_TauR_inv _ _ e2) as [ t3' [ e_t3 e_t3' ]]; subst t3.
+    apply lr_refinesF_Tau. right. eapply CIH; eassumption.
+  - pstep. rewrite BindS_Vis_eq in e0. rewrite BindS_Vis_eq in e3.
+    destruct (eq_itree_VisR_inv _ _ _ e0) as [ k1' [ e_k1 e_k1' ]]; subst t1.
+    destruct (eq_itree_VisR_inv _ _ _ e3) as [ k2' [ e_k2 e_k2' ]]; subst t2.
+    apply lr_refinesF_Vis; [ assumption | ].
+    intros. right. eapply CIH; [ apply e_k1' | apply e_k2' | ].
+    destruct (H0 a b H1) as [ H2 | []]. assumption.
+  - cbn in e1; rewrite bind_Tau_eq in e1.
+    destruct (eq_itree_TauR_inv _ _ e1) as [ t0' [ e_t0 e_t0' ]]; subst t0.
+    pstep. apply lr_refinesF_TauL. pstep_reverse.
+  - cbn in e2; rewrite bind_Tau_eq in e2.
+    destruct (eq_itree_TauR_inv _ _ e2) as [ t0' [ e_t0 e_t0' ]]; subst t0.
+    pstep. apply lr_refinesF_TauR. pstep_reverse.
+  - cbn in e2; rewrite bind_Vis_eq in e2.
+    destruct (eq_itree_VisR_inv _ _ _ e2) as [ k2' [ e_k2 e_k2' ]]; subst t2.
+    pstep. apply lr_refinesF_forallR. intros.
+    observe_tau. pstep_reverse.
+    eapply H0; [ eassumption | ].
+    transitivity (Tau (BindS (k a) k2));
+      [ | rewrite <- BindS_Tau_eq; reflexivity ].
+    apply eqit_Tau. apply e_k2'.
+  - cbn in e2; rewrite bind_Vis_eq in e2.
+    destruct (eq_itree_VisR_inv _ _ _ e2) as [ k2' [ e_k2 e_k2' ]]; subst t2.
+    pstep. apply (lr_refinesF_existsR _ _ _ _ _ _ _ _ _ a).
+    observe_tau. pstep_reverse. apply IHmref; [ assumption | ].
+    transitivity (Tau (BindS (k a) k2));
+      [ | rewrite <- BindS_Tau_eq; reflexivity ].
+    apply eqit_Tau. apply e_k2'.
+  - cbn in e1; rewrite bind_Vis_eq in e1.
+    destruct (eq_itree_VisR_inv _ _ _ e1) as [ k1' [ e_k1 e_k1' ]]; subst t1.
+    pstep. apply (lr_refinesF_forallL _ _ _ _ _ _ _ _ _ a).
+    observe_tau. pstep_reverse. apply IHmref; [ | assumption ].
+    transitivity (Tau (BindS (k a) k1));
+      [ | rewrite <- BindS_Tau_eq; reflexivity ].
+    apply eqit_Tau. apply e_k1'.
+  - cbn in e1; rewrite bind_Vis_eq in e1.
+    destruct (eq_itree_VisR_inv _ _ _ e1) as [ k1' [ e_k1 e_k1' ]]; subst t1.
+    pstep. apply lr_refinesF_existsL. intros.
+    observe_tau. pstep_reverse. apply (H0 a); [ | assumption ].
+    transitivity (Tau (BindS (k a) k1));
+      [ | rewrite <- BindS_Tau_eq; reflexivity ].
+    apply eqit_Tau. apply e_k1'.
+  - cbn in e1. unfold SpecM, entree_spec in e1. rewrite bind_Vis_eq in e1.
+    destruct (eq_itree_VisR_inv _ _ _ e1) as [ k1' [ e_k1 e_k1' ]]; subst t1.
+    pstep. apply lr_refinesF_unfoldL. observe_tau. pstep_reverse.
+    apply IHmref; [ | assumption ].
+    rewrite BindS_Tau_eq. apply eqit_Tau. cbn. rewrite bind_bind.
+    eapply eqit_bind; [ reflexivity | ]. intros. subst u2. apply e_k1'.
+  - cbn in e2. unfold SpecM, entree_spec in e2. rewrite bind_Vis_eq in e2.
+    destruct (eq_itree_VisR_inv _ _ _ e2) as [ k2' [ e_k2 e_k2' ]]; subst t2.
+    pstep. apply lr_refinesF_unfoldR. observe_tau. pstep_reverse.
+    apply IHmref; [ assumption | ].
+    rewrite BindS_Tau_eq. apply eqit_Tau. cbn. rewrite bind_bind.
+    eapply eqit_bind; [ reflexivity | ]. intros. subst u2. apply e_k2'.
+Qed.
+
+
+End lr_refines_bind.
+
+
+(*** LetRec Lemma ***)
+Section lr_refines_letrec.
+Context {E1 E2 : EvType} {stk1 stk2 : FunStack} {R1 R2 : Type}.
+Context (funs1 : StackTuple E1 stk1 stk1) (funs2 : StackTuple E2 stk2 stk2).
+Context (RPre : Rel (FunStackE E1 pnil) (FunStackE E2 pnil))
+  (RPost : PostRel (FunStackE E1 pnil) (FunStackE E2 pnil))
+  (RR : Rel R1 R2).
+
+Lemma lr_refines_letrec t1 t2 :
+  lr_refines funs1 funs2 (liftNilRel RPre) (liftNilPostRel RPost) RR t1 t2 ->
+  lr_refines (emptyStackTuple E1 _) (emptyStackTuple E2 _) RPre RPost RR
+    (LetRecS _ R1 _ funs1 t1) (LetRecS _ R2 _ funs2 t2).
+Proof.
+  revert t1 t2; pcofix CIH; intros t1 t2 ref12.
+  punfold ref12; red in ref12. destruct t1 as [ ot1 ]. destruct t2 as [ ot2 ].
+  pstep. red.
+  simpl in ref12. induction ref12.
+  - apply lr_refinesF_Ret. assumption.
+  - apply lr_refinesF_Tau. right. apply CIH. pclearbot. assumption.
+  - destruct e1; destruct e2; try destruct H.
+    apply lr_refinesF_Vis; [ apply H | ]. right.
+    apply CIH. destruct (H0 _ _ H1); [ | destruct H2 ]. apply H2.
+  - apply lr_refinesF_TauL. assumption.
+  - apply lr_refinesF_TauR. assumption.
+  - apply lr_refinesF_forallR; intros; apply H0.
+  - eapply lr_refinesF_existsR; apply IHref12.
+  - eapply lr_refinesF_forallL; apply IHref12.
+  - apply lr_refinesF_existsL; intros; apply H0.
+  - apply IHref12.
+  - apply IHref12.
+Qed.
+
+End lr_refines_letrec.
+
+
+(*** Discharge and Push lemmas ***)
+Section lr_refines_discharge_push.
+Context {E1 E2 : EvType} {stk1 stk2 : FunStack} {R1 R2 : Type} {RR : Rel R1 R2}.
+Context (funs1 : StackTuple E1 stk1 stk1) (funs2 : StackTuple E2 stk2 stk2).
+
+(* Discharge a local pre/postcondition about calls *)
+Lemma lr_refines_discharge RPre RPost precond postcond t1 t2 :
+  (forall call1 call2,
+      (precond call1 call2 : Prop) ->
+      lr_refines funs1 funs2 (addCallPreRel precond RPre)
+        (addCallPostRel postcond RPost) (postcond call1 call2)
+        (applyStackTuple _ _ funs1 call1)
+        (applyStackTuple _ _ funs2 call2)) ->
+  lr_refines funs1 funs2 (addCallPreRel precond RPre)
+    (addCallPostRel postcond RPost) RR t1 t2 ->
+  lr_refines funs1 funs2 (liftNilRel RPre) (liftNilPostRel RPost) RR t1 t2.
+Proof.
+  intro funsRef. revert t1 t2; pcofix CIH; intros.
+  punfold H0. red in H0. pstep. red.
+  remember (observe t1) as ot1.
+  remember (observe t2) as ot2.
+  clear t1 Heqot1 t2 Heqot2.
+  hinduction H0 before ot1; intros; pclearbot.
+  - apply lr_refinesF_Ret. assumption.
+  - apply lr_refinesF_Tau. right. apply CIH. apply H.
+  - destruct e1; destruct e2.
+    + apply lr_refinesF_unfoldL. apply lr_refinesF_unfoldR.
+      apply lr_refinesF_Tau. right. apply CIH.
+      apply (lr_refines_bind (RS:=postcond s s0)).
+      -- apply funsRef. assumption.
+      -- intros. destruct (H0 x1 x2 H1) as [ H3 | [] ].
+         assumption.
+    + destruct H.
+    + destruct H.
+    + apply lr_refinesF_Vis; [ apply H | ]. intros.
+      right. apply CIH. destruct (H0 a b H1) as [ H2 | [] ].
+      assumption.
+  - apply lr_refinesF_TauL. assumption.
+  - apply lr_refinesF_TauR. assumption.
+  - apply lr_refinesF_forallR. intros. apply H0.
+  - eapply lr_refinesF_existsR. apply IHlr_refinesF.
+  - eapply lr_refinesF_forallL. apply IHlr_refinesF.
+  - apply lr_refinesF_existsL. intros. apply H0.
+  - apply lr_refinesF_unfoldL. apply IHlr_refinesF.
+  - apply lr_refinesF_unfoldR. apply IHlr_refinesF.
+Qed.
+
+(* Push a pre/postcondition onto those of a refinement *)
+Lemma lr_refines_push_prepost RPre RPost precond postcond t1 t2 :
+  lr_refines funs1 funs2 (liftNilRel RPre) (liftNilPostRel RPost) RR t1 t2 ->
+  lr_refines funs1 funs2 (addCallPreRel precond RPre)
+    (addCallPostRel postcond RPost) RR t1 t2.
+Proof.
+  revert t1 t2; pcofix CIH; intros.
+  punfold H0. red in H0. pstep. red.
+  remember (observe t1) as ot1.
+  remember (observe t2) as ot2.
+  clear t1 Heqot1 t2 Heqot2.
+  hinduction H0 before ot1; intros; pclearbot.
+  - apply lr_refinesF_Ret. assumption.
+  - apply lr_refinesF_Tau. right. apply CIH. assumption.
+  - destruct e1 as [ call1 | ]; destruct e2 as [ call2 | ];
+      [ destruct H | destruct H | destruct H | ].
+    apply lr_refinesF_Vis; [ assumption | ]. intros.
+    right. apply CIH. destruct (H0 a b H1) as [ H2 | [] ]. assumption.
+  - apply lr_refinesF_TauL. apply IHlr_refinesF.
+  - apply lr_refinesF_TauR. apply IHlr_refinesF.
+  - apply lr_refinesF_forallR. intros. apply (H0 a).
+  - eapply lr_refinesF_existsR. apply IHlr_refinesF.
+  - eapply lr_refinesF_forallL. apply IHlr_refinesF.
+  - apply lr_refinesF_existsL. intros. apply (H0 a).
+  - apply lr_refinesF_unfoldL. apply IHlr_refinesF.
+  - apply lr_refinesF_unfoldR. apply IHlr_refinesF.
+Qed.
+
+End lr_refines_discharge_push.
