src/ITreeSpec/Padded.v
@@ -1,0 +1,148 @@
+From Stdlib Require Import
+  Program
+  Setoid
+  Morphisms
+  Relations.
+
+From ITree Require Import
+  Basics.Basics
+  Basics.Utils
+  Basics.HeterogeneousRelations.
+
+From ITree Require Import
+  Basics.HeterogeneousRelations
+  Core.ITreeDefinition
+  Eq.Eqit.
+
+From Paco Require Import paco.
+
+Local Open Scope itree_scope.
+
+Section padded.
+Context {E : Type -> Type} {R : Type}.
+
+Variant paddedF (F : itree E R -> Prop) : itree' E R -> Prop :=
+  | paddedF_Ret r : paddedF F (RetF r)
+  | paddedF_Tau t : F t -> paddedF F (TauF t)
+  | paddedF_Vis {X} e (k : X -> itree E R) :
+    (forall a, F (k a)) -> paddedF F (VisF e (fun a => (Tau (k a))))
+.
+Hint Constructors paddedF : itree_spec.
+
+Definition padded_ sim := fun t => paddedF sim (observe t).
+
+Lemma padded_monotone_ : monotone1 padded_.
+Proof with eauto with itree_spec. 
+  red. unfold padded_. intros. 
+  induction IN...
+Qed.
+
+Hint Resolve padded_monotone_ : itree_spec.
+
+Definition padded := paco1 padded_ bot1.
+
+Lemma padded_VisF_inv {X} (e : E X) k F :
+  paddedF F (VisF e k) ->
+  exists k', forall a, k a ≅ Tau (k' a).
+Proof with eauto with itree_spec.
+  intros. dependent destruction H... eexists. reflexivity.
+Qed.
+
+
+CoFixpoint pad' (ot : itree' E R) : itree E R :=
+  match ot with
+  | RetF r => Ret r
+  | TauF t => Tau (pad' (observe t))
+  | VisF e k => Vis e (fun x => Tau (pad' (observe (k x)))) 
+  end.
+
+Definition pad t := pad' (observe t).
+
+Lemma pad_ret r : pad (Ret r) ≅ Ret r.
+Proof.
+  pstep.
+  red. simpl.
+  constructor. auto.
+Qed.
+
+Lemma pad_tau t : pad (Tau t) ≅ Tau (pad t).
+Proof.
+  pstep. red. cbn. constructor. left. enough (pad t ≅ pad t). auto.
+  reflexivity.
+Qed.
+
+Lemma pad_vis {X} (e : E X) k : pad (Vis e k) ≅ Vis e (fun x => Tau (pad (k x))).
+Proof.
+  pstep. red. cbn. constructor. left.  pstep. constructor.
+  left. enough (pad (k v) ≅ pad (k v)). auto. reflexivity.
+Qed.
+
+End padded.
+
+#[global] Hint Constructors paddedF : itree_spec.
+
+Theorem pad_is_padded {E : Type -> Type} {R : Type} : forall t : itree E R, padded (pad t).
+Proof with eauto with itree_spec.
+  pcofix CIH. intros. pstep. unfold pad.
+  destruct (observe t); red; simpl; eauto with itree_spec.
+Qed.
+#[global] Hint Resolve padded_monotone_ : paco.
+#[global] Hint Resolve padded_monotone_ : itree_spec.
+#[global] Hint Resolve pad_is_padded : itree_spec.
+
+Theorem pad_eutt {E : Type -> Type} {R : Type} : forall t : itree E R, t ≈ pad t.
+Proof with eauto with itree_spec.
+  ginit. gcofix CIH. intros.
+  unfold pad.
+  destruct (observe t) eqn : Ht; symmetry in Ht; apply simpobs in Ht.
+  - rewrite Ht.
+    gstep. red; simpl. constructor; auto.
+  - rewrite Ht.
+    gstep. red; simpl.
+    constructor.
+    gfinal. eauto.
+  - rewrite Ht. gstep. red. cbn.
+    constructor. intros. red.
+    rewrite tau_euttge.
+    gfinal. eauto.
+Qed.
+
+Global Instance pad_Proper {b1 b2 : bool} {E : Type -> Type} {R : Type} : Proper (eqit eq b1 b2 ==> eqit eq b1 b2) (@pad E R).
+Proof.
+  pcofix CIH.
+  intros t1 t2 Ht12. pstep. red. unfold pad.
+  punfold Ht12. red in Ht12. hinduction Ht12 before r;
+    intros; cbn; eauto.
+  - constructor. auto.
+  - constructor. pclearbot. right. eapply CIH; eauto.
+  - constructor. left. pstep. constructor. pclearbot. right.
+    eapply CIH; eauto. apply REL.
+  - constructor; auto.
+  - constructor; auto.
+Qed.
+
+Theorem pad_bind {E : Type -> Type} {R S: Type} : forall (t : itree E R) (k : R -> itree E S),
+    pad (ITree.bind t k) ≅ ITree.bind (pad t) (fun x => pad (k x)).
+Proof.
+  ginit. gcofix CIH. intros t k.
+  destruct (observe t) eqn : Heq; symmetry in Heq; apply simpobs in Heq.
+  - rewrite Heq. rewrite pad_ret. repeat rewrite bind_ret_l.
+    apply Reflexive_eqit_gen. auto.
+  - repeat rewrite Heq. rewrite pad_tau. repeat rewrite bind_tau. gstep.
+    red; cbn.
+    constructor.
+    gfinal. eauto.
+  - repeat rewrite Heq. rewrite pad_vis. repeat rewrite bind_vis. rewrite pad_vis.
+    gstep. constructor. intros. unfold id. gstep. red; cbn. constructor. gfinal. left. eapply CIH.
+Qed.
+
+Theorem pad_iter E R S (body : R -> itree E (R + S)):
+  forall r, pad (ITree.iter body r) ≅ ITree.iter (fun r => pad (body r)) r.
+Proof.
+  ginit. gcofix CIH.
+  intros. setoid_rewrite unfold_iter. rewrite pad_bind.
+  guclo eqit_clo_bind. econstructor.
+  reflexivity. intros. subst. destruct u2.
+  - rewrite pad_tau. gstep. constructor. gfinal. left. eauto.
+  - rewrite pad_ret. gstep. constructor. auto.
+Qed.
