src/ITreeSpec/RecFixSpecTotal.v
@@ -1,0 +1,95 @@
+From Stdlib Require Export
+  Morphisms
+  Setoid
+  Program.Equality
+  Lists.List
+  Logic.EqdepFacts
+  Eqdep EqdepFacts.
+
+Require Import  ExtLib.Structures.Monad.
+
+From ITree Require Import
+  Basics.HeterogeneousRelations
+  Core.ITreeDefinition
+  Eq.Eqit.
+
+From ITreeSpec Require Import
+  ITreeSpecDefinition
+  ITreeSpecFacts
+  ITreeSpecCombinatorFacts
+  MRecSpec
+  RecSpecFix.
+
+Open Scope entree_scope.
+Import Monad.
+Import MonadNotation.
+Local Open Scope monad_scope.
+From Paco Require Import paco.
+Fixpoint trepeat {E R: Type} `{EncodingType E} (n : nat) (t : entree E R) :=
+  match n with
+  | 0 => ret tt
+  | S n => t;; trepeat n t end.
+
+Section total_spec_fix.
+Context {A B : Type} `{QuantType A} `{QuantType B}.
+Context {E : Type} `{EncodingType E}.
+
+Context (Pre : A -> Prop) (Post : A -> B -> Prop).
+
+
+Definition total_spec' (a : A) : entree_spec E B :=
+  assume_spec (Pre a);;
+  b <- exists_spec B;;
+  assert_spec (Post a b);;
+  ret b.
+  
+
+Context (Rdec : Rel A A).
+Context (Hwf : well_founded Rdec).
+
+Definition total_spec_fix : A -> entree_spec E B :=
+  rec_fix_spec 
+    (fun rec a =>
+       assume_spec (Pre a);;
+       n <- exists_spec nat;;
+       trepeat n (
+         a' <- exists_spec A;;
+         assert_spec (Pre a' /\ Rdec a' a);;
+         rec a');;
+       b <- exists_spec B;;
+       assert_spec (Post a b);;
+       ret b
+    ).
+Theorem total_spec_fix_refines_total_spec' (a : A) : strict_refines (total_spec_fix a) (total_spec' a).
+Proof.
+  revert a. eapply well_founded_ind; eauto.
+  intros a Hind. unfold total_spec_fix, total_spec'.
+  quantr. intros. quantl. auto.
+  match goal with |- padded_refines eq PostRelEq eq (interp_mrec_spec ?b _ ) _ => set b as body end.
+  quantl. intros n. induction n.
+  - cbn. quantl. intros b. quantr. exists b. quantl. intros. quantr. auto.
+    apply padded_refines_ret. auto.
+  - cbn. do 2 rewrite interp_mrec_spec_bind. repeat apply padded_refines_bind_bind_l.
+    match goal with |- padded_refines eq PostRelEq eq _ ?t => assert (t ≅ Ret tt;; t) end.
+    cbn. 
+    (* some rewriting fails here for some reason *)
+    { pstep. red. cbn. rewrite itree_eta' at 1. rewrite itree_eta'. pstep_reverse.
+      apply Reflexive_eqit. auto. }
+    rewrite H3. eapply padded_refines_bind with (RR := fun _ _ => True).
+    + quantl. intros. quantl. intros [Hpre Hdec].
+      eapply padded_refines_weaken_l with (phi2 := total_spec' a0;; Ret tt).
+      * cbn. apply padded_refines_bind_bind_l.
+        quantl. auto. apply padded_refines_bind_bind_l.
+        quantl. intros. apply padded_refines_bind_bind_l. quantl.
+        intros. apply padded_refines_ret. auto.
+      * specialize (Hind a0 Hdec).
+        unfold call_spec. setoid_rewrite interp_mrec_spec_inl. rewrite tau_eutt.
+        rewrite interp_mrec_spec_bind. eapply padded_refines_bind; intros; try apply padded_refines_ret; eauto.
+    + intros b0 [] _. eapply padded_refines_weaken_l; try eapply IHn.
+      setoid_rewrite interp_mrec_spec_bind. 
+      eapply padded_refines_bind; intros; subst; try reflexivity.
+      quantl. intros. cbn.  eapply interp_mrec_spec_exists_specr. Unshelve. 2: eauto. 
+      quantl. intros. subst. quantr. auto. apply padded_refines_ret. auto.
+Qed.
+
+End total_spec_fix.
