src/ITreeSpec/TpEnc.v
@@ -1,0 +1,188 @@
+From Coq Require Import
+     Program
+     Setoid
+     Morphisms
+     Relations
+     Logic.FinFun
+.
+
+From Paco Require Import paco.
+
+From ITree Require Import
+     Basics.Basics
+     Basics.Utils
+     Basics.HeterogeneousRelations
+     Eq.Paco2.
+
+From EnTree Require Import
+     Basics.HeterogeneousRelations
+     Core.EnTreeDefinition
+     Core.SubEvent
+.
+
+Local Open Scope entree_scope.
+
+Set Printing Universes.
+
+Inductive TpEnc : Type@{entree_u} :=
+  | TpEnc_nat : TpEnc
+  | TpEnc_unit : TpEnc
+  | TpEnc_pair : TpEnc -> TpEnc -> TpEnc
+  | TpEnc_sum : TpEnc -> TpEnc -> TpEnc
+  | TpEnc_fun : TpEnc -> TpEnc -> TpEnc
+  | TpEnc_prop : Prop -> TpEnc
+  | TpEnc_list : TpEnc -> TpEnc
+  | TpEnc_Vec : nat -> TpEnc -> TpEnc.
+Check TpEnc : Type@{Set + 1}.
+
+
+Variant SpecEvent (E : Type@{entree_u}) : Type@{entree_u}:=
+  | Spec_vis (e : E)
+  | Spec_forall (tp : TpEnc)
+  | Spec_exists (tp : TpEnc).
+Arguments Spec_vis {_}.
+Arguments Spec_forall {_}.
+Arguments Spec_exists {_}.
+
+Fixpoint TpEnc_enc (tp : TpEnc) : Type@{entree_u} :=
+  match tp with
+  | TpEnc_nat => nat
+  | TpEnc_unit => unit
+  | TpEnc_pair tp1 tp2 => (TpEnc_enc tp1) * (TpEnc_enc tp2)
+  | TpEnc_sum tp1 tp2 => (TpEnc_enc tp1) + (TpEnc_enc tp2)
+  | TpEnc_fun tp1 tp2 => (TpEnc_enc tp1) -> (TpEnc_enc tp2)
+  | TpEnc_prop P => P
+  | TpEnc_list tp => list (TpEnc_enc tp)
+  | TpEnc_Vec n tp => False
+  end.
+
+#[global] Instance TpEnc_enc_inst : EncodedType TpEnc := TpEnc_enc.
+
+#[global] Instance encoded_SpecEvent E `{EncodedType E} : EncodedType (SpecEvent E) :=
+  fun s => 
+    match s with
+    | Spec_vis e => encodes e
+    | Spec_forall tp => encodes tp
+    | Spec_exists tp => encodes tp 
+end.
+
+Class QIndex (T : Type) :=
+  {
+    enc : TpEnc;
+    index : encodes enc -> T;
+    index_surj : Surjective index
+  }.
+
+#[global] Instance SpecEventReSum E1 E2 `{ReSum E1 E2} : ReSum E1 (SpecEvent E2) :=
+  fun e => Spec_vis (resum e).
+#[global] Instance SpecEventReSumRet E1 E2 {EncE1 : EncodedType E1} {EncE2 : EncodedType E2} {Res : ReSum E1 E2}
+ {ResRet : ReSumRet E1 E2} : ReSumRet E1 (SpecEvent E2) := fun e x => @resum_ret _ _ _ _ _ ResRet e x.
+
+Definition entree_spec E `{EncodedType E} R := entree (SpecEvent E) R.
+Notation entree_spec' E R := (entree' (SpecEvent E) R).
+
+Create HintDb entree_spec.
+
+Section refines.
+
+Context {E1 E2 : Type} `{EncodedType E1} `{EncodedType E2} {R1 R2 : Type}.
+
+Context (RPre : E1 -> E2 -> Prop) (RPost : forall (e1 : E1) (e2 : E2), encodes e1 -> encodes e2 -> Prop) (RR : R1 -> R2 -> Prop).
+
+Inductive refinesF (sim : entree_spec E1 R1 -> entree_spec E2 R2 -> Prop) : entree_spec' E1 R1 -> entree_spec' E2 R2 -> Prop := 
+  | refinesF_Ret r1 r2 : RR r1 r2 -> refinesF sim (RetF r1) (RetF r2)
+  | refinesF_Tau t1 t2 : sim t1 t2 -> refinesF sim (TauF t1) (TauF t2)
+  | refinesF_Vis e1 e2 k1 k2 : RPre e1 e2 -> (forall a b, RPost e1 e2 a b -> sim (k1 a) (k2 b) ) ->
+                               refinesF sim (VisF (Spec_vis e1) k1) (VisF (Spec_vis e2) k2)
+  | refinesF_TauL t1 ot2 : refinesF sim (observe t1) ot2 -> refinesF sim (TauF t1) ot2
+  | refinesF_TauR ot1 t2 : refinesF sim ot1 (observe t2) -> refinesF sim ot1 (TauF t2)
+
+  | refinesF_forallR A ot1 k : (forall a, refinesF sim ot1 (observe (k a)) ) -> refinesF sim ot1 (VisF (Spec_forall A) k)
+  | refinesF_existsR A ot1 k a : refinesF sim ot1 (observe (k a)) -> refinesF sim ot1 (VisF (Spec_exists A) k)
+  | refinesF_forallL A ot2 k a : refinesF sim (observe (k a)) ot2 -> refinesF sim (VisF (Spec_forall A) k ) ot2
+  | refinesF_existsL A ot2 k : (forall a, refinesF sim (observe (k a)) ot2) -> refinesF sim (VisF (Spec_exists A) k) ot2
+.
+
+Hint Constructors refinesF : entree_spec.
+
+Definition refines_ sim : entree_spec E1 R1 -> entree_spec E2 R2 -> Prop :=
+  fun t1 t2 => refinesF sim (observe t1) (observe t2).
+
+Lemma monotone_refinesF ot1 ot2 sim sim' (LE : sim <2= sim')
+      (IN : refinesF sim ot1 ot2) : refinesF sim' ot1 ot2.
+Proof with eauto with entree_spec.
+  induction IN...
+Qed.
+
+Lemma monotone_refines_: monotone2 refines_.
+Proof. red. intros. eapply monotone_refinesF; eauto. Qed.
+
+Hint Resolve monotone_refines_ : paco.
+
+Definition refines := paco2 refines_ bot2.
+
+End refines.
+
+(* what is *)
+Definition forall_spec {E} `{EncodedType E} (A : Type) `{QIndex A} : entree_spec E A :=
+  Vis (Spec_forall enc) (fun x : encodes (Spec_forall enc) => Ret (index x)).
+
+Lemma forall_spec_correctr {E1 E2} `{EncodedType E1} `{EncodedType E2} 
+      (A : Type) `{QIndex A} R1 R2  RPre RPost RR
+      (k : A -> entree_spec E2 R1) (t : entree_spec E1 R2) :
+  (forall a : A, refines RPre RPost RR t (k a)) ->
+  refines RPre RPost RR t (EnTree.bind (forall_spec A) k).
+Proof.
+  intros. pstep. red. cbn. constructor. cbn. intros. simpl.
+  pstep_reverse. auto with entree_spec. apply monotone_refines_.
+  apply H2.
+Qed.
+
+Lemma forall_spec_correctl {E1 E2} `{EncodedType E1} `{EncodedType E2} 
+      (A : Type) `{QIndex A} R1 R2  RPre RPost RR
+      (k : A -> entree_spec E2 R1) (t : entree_spec E1 R2) :
+  (exists a : A, refines RPre RPost RR (k a) t) ->
+  refines RPre RPost RR (EnTree.bind (forall_spec A) k) t.
+Proof.
+  intros. destruct H2 as [a Ha]. pstep. red.
+  specialize (index_surj a) as [x Hx]. econstructor.
+  Unshelve. 2 : exact x. rewrite Hx. simpl. pstep_reverse.
+  apply monotone_refines_.
+Qed.
+
+Definition exists_spec {E} `{EncodedType E} (A : Type) `{QIndex A} : entree_spec E A :=
+  Vis (Spec_exists enc) (fun x : encodes (Spec_exists enc) => Ret (index x)).
+
+Lemma exists_spec_correctr {E1 E2} `{EncodedType E1} `{EncodedType E2} 
+      (A : Type) `{QIndex A} R1 R2  RPre RPost RR
+      (k : A -> entree_spec E2 R1) (t : entree_spec E1 R2) :
+  (exists a : A, refines RPre RPost RR t (k a)) ->
+  refines RPre RPost RR t (EnTree.bind (exists_spec A) k).
+Proof.
+  intros. destruct H2 as [a Ha]. pstep. red.
+  specialize (index_surj a) as [x Hx]. econstructor.
+  Unshelve. 2 : exact x. rewrite Hx. simpl. pstep_reverse.
+  apply monotone_refines_.
+Qed.
+
+Lemma exists_spec_correctl {E1 E2} `{EncodedType E1} `{EncodedType E2} 
+      (A : Type) `{QIndex A} R1 R2  RPre RPost RR
+      (k : A -> entree_spec E2 R1) (t : entree_spec E1 R2) :
+  (forall a : A, refines RPre RPost RR t (k a)) ->
+  refines RPre RPost RR t (EnTree.bind (forall_spec A) k).
+Proof.
+  intros. pstep. red. cbn. constructor. cbn. intros. simpl.
+  pstep_reverse. auto with entree_spec. apply monotone_refines_.
+  apply H2.
+Qed.
+
+(*
+Definition assume_spec {E} `{EncodedType E} (P : Prop) : entree_spec E unit :=
+  Vis (Spec_forall P) (fun _ => Ret tt).
+Definition assert_spec {E} `{EncodedType E} (P : Prop) : entree_spec E unit :=
+  Vis (Spec_exists P) (fun _ => Ret tt).
+Definition forall_spec {E} `{EncodedType E} (A : Set) : entree_spec E A :=
+  Vis (Spec_forall A) (fun a => Ret a).
+Definition exists_spec {E} `{EncodedType E} (A : Set) : entree_spec E A :=
+  Vis (Spec_exists A) (fun a => Ret a).
+*)
